@prefix rdfs: <http://www.w3.org/2000/01/rdf-schema#>.
@prefix owl: <http://www.w3.org/2002/07/owl#>.
@prefix xsd: <http://www.w3.org/2001/XMLSchema#>.
@prefix skos: <http://www.w3.org/2004/02/skos/core#>.
@prefix dct: <http://purl.org/dc/terms/>.
@prefix human: <http://e-editiones.ch/ontology/human#>.
@prefix language: <http://e-editiones.ch/ontology/language#>.
@prefix teach: <http://e-editiones.ch/ontology/teaching#>.
@prefix document: <http://e-editiones.ch/ontology/document#>.
@prefix text: <http://e-editiones.ch/ontology/text#>.
@prefix image: <http://e-editiones.ch/ontology/image#>.
@prefix text-expression: <http://e-editiones.ch/ontology/text-expression#>.
@prefix text-structure: <http://e-editiones.ch/ontology/text-structure#>.
@prefix prosodic-structure: <http://e-editiones.ch/ontology/prosodic-structure#>.
@prefix textedit: <http://e-editiones.ch/ontology/text-editing#>.
@prefix scholarly-editing: <http://e-editiones.ch/ontology/scholarly-editing#>.
@prefix publish: <http://e-editiones.ch/ontology/publishing#>.
@prefix literature: <http://e-editiones.ch/ontology/literature#>.

@base <http://e-editiones.ch/ontology/delille>.
@prefix delille: <http://e-editiones.ch/ontology/delille#>.

<http://e-editiones.ch/ontology/delille>
	a owl:Ontology;
	dct:license <http://creativecommons.org/licenses/by/3.0/>;
	dct:title "An ontology about Jacques Delille's poetry citation"@en;
	dct:description """Formal description of specific concepts in the scientific edition about citations of the poem 'L'Homme des champs' of Jacques Delille, 22 June 1738 – 1 May 1813."""@en;
	dct:creator "Hans Cools, MD, knowledge engineer, ontologist, software developer, University of Basel, Switzerland"@en;
	dct:contributor
		"Dr. Roberta Padlina, tool coordinator and software developer, University of Basel, Switzerland"@en,
		"Prof. Dr. Hugues Marchal, Departement of Languages and Literatures, Faculty of Philosophy and History, University of Basel"@en;
	dct:publisher "University of Basel, Switzerland"@en;
	owl:versionInfo "2020-06-11"^^xsd:date.

#
# CLASSES
#

delille:VersePoem
	rdfs:isDefinedBy <http://e-editiones.ch/ontology/delille#>;
	a rdfs:Class;
	rdfs:label "Jacques Delille verse poem"@en, "Versgedicht Jacques Delilles"@de;
	rdfs:comment """Verse poem authored by Jacques Delille."""@en;
	rdfs:subClassOf literature:VersePoem, publish:TextExpression.
#	hasAuthor Delille

delille:TranslatedVersePoem
	rdfs:isDefinedBy <http://e-editiones.ch/ontology/delille#>;
	a rdfs:Class;
	rdfs:label "translated Jacques Delille verse poem"@en, "übersetzter Versgedicht Jacques Delilles"@de;
	rdfs:comment """Translated Jacques Delille verse poem."""@en;
	rdfs:subClassOf delille:VersePoem, language:PersonTranslation, text:Translation.

delille:NonVersePoem
	rdfs:isDefinedBy <http://e-editiones.ch/ontology/delille#>;
	a rdfs:Class;
	rdfs:label "Jacques Delille non-verse poem"@en, "Non-Versgedicht Jacques Delilles"@de;
	rdfs:comment """Expression other than a verse poem, authored by Jacques Delille."""@en;
	rdfs:subClassOf publish:TextExpression.
#	hasAuthor Delille

delille:EditedVersePoem
	rdfs:isDefinedBy <http://e-editiones.ch/ontology/delille#>;
	a rdfs:Class;
	rdfs:label "edited Jacques Delille verse poem"@en, "ediertes Versgedicht Jacques Delilles"@de;
	rdfs:comment """Verse poem authored by Jacques Delille and edited."""@en;
	rdfs:subClassOf delille:VersePoem, textedit:Edition.

delille:Canto
	rdfs:isDefinedBy <http://e-editiones.ch/ontology/delille#>;
	a rdfs:Class;
	rdfs:label "Jacques Delille canto"@en, "Canto Jacques Delilles"@de, "chant de Jacques Delille"@fr, "canto di Jacques Delille"@it;
	rdfs:comment """Group of strophes in a verse poem authored by Jacques Delille."""@en;
	rdfs:subClassOf prosodic-structure:VerseSection, text-expression:ExpressionPart.

delille:CitingExpression
	rdfs:isDefinedBy <http://e-editiones.ch/ontology/delille#>;
	a rdfs:Class;
	rdfs:label "citing text expression"@en, "zitierende Textexpression"@de; #, ""@fr, ""@it;
	rdfs:comment """Text expression citing one or more verses of a poem authored by Jacques Delille."""@en;
	rdfs:subClassOf publish:TextExpression.

delille:Dictionary
	rdfs:isDefinedBy <http://e-editiones.ch/ontology/delille#>;
	a rdfs:Class;
	rdfs:label "citing dictionary"@en, "zitierendes Wörterbuch"@de; #, ""@fr, ""@it;
	rdfs:comment """Dictionary citing one or more verses of a poem authored by Jacques Delille."""@en;
	rdfs:subClassOf text-expression:Dictionary, delille:CitingExpression.

delille:Manual
	rdfs:isDefinedBy <http://e-editiones.ch/ontology/delille#>;
	a rdfs:Class;
	rdfs:label "teaching manual"@en, "Lehrbuch"@de, "manuel scolaire"@fr, "manuale di testo"@it;
	rdfs:comment """Teaching manual as in the scientific edition about Jacques Delille's poetry citation."""@en;
	rdfs:subClassOf teach:Manual.

delille:Anthology
	rdfs:isDefinedBy <http://e-editiones.ch/ontology/delille#>;
	a rdfs:Class;
	rdfs:label "anthology"@en, "Anthologie"@de, "anthologie"@fr, "antologia"@it;
	rdfs:comment """Anthology as in the scientific edition about Jacques Delille's poetry citation."""@en;
	rdfs:subClassOf literature:Anthology.

delille:AnthologyOrManual
	rdfs:isDefinedBy <http://e-editiones.ch/ontology/delille#>;
	a rdfs:Class;
	rdfs:label "citing anthology or teaching manual"@en, "zitierende/s Anthologie oder Lehrbuch"@de; #, ""@fr, ""@it;
	rdfs:comment """Anthology or teaching manual citing one or more verses of a poem authored by Jacques Delille."""@en;
	rdfs:subClassOf delille:CitingExpression;
	owl:disjointUnionOf (delille:Anthology delille:Manual).

delille:LiteraryExpression
	rdfs:isDefinedBy <http://e-editiones.ch/ontology/delille#>;
	a rdfs:Class;
	rdfs:label "citing literary publication expression"@en, "zitierende literarische Publikationsexpression"@de; #, ""@fr, ""@it;
	rdfs:comment """Literary publication expression citing one or more verses of a poem authored by Jacques Delille."""@en;
	rdfs:subClassOf literature:Expression, delille:CitingExpression.

delille:PoemOrVersePlay
	rdfs:isDefinedBy <http://e-editiones.ch/ontology/delille#>;
	a rdfs:Class;
	rdfs:label "citing poem or verse play"@en, "zitierendes Gedicht oder Vers-Theaterstück"@de, "poème ou pièce de théâtre en vers citante"@fr; #, ""@it;
	rdfs:comment """Poem or verse play citing one or more verses of a poem authored by Jacques Delille."""@en;
	rdfs:subClassOf delille:LiteraryExpression.

delille:Novel
	rdfs:isDefinedBy <http://e-editiones.ch/ontology/delille#>;
	a rdfs:Class;
	rdfs:label "citing novel"@en, "zitierender Roman"@de; #, "récit fictionnel"@fr, ""@it;
	rdfs:comment """Novel citing one or more verses of a poem authored by Jacques Delille."""@en;
	rdfs:subClassOf literature:Novel, delille:LiteraryExpression.

delille:EssayOrPanoramicLiteraryOrPhilosophicOrHumanitiesExpression
	rdfs:isDefinedBy <http://e-editiones.ch/ontology/delille#>;
	a rdfs:Class;
	rdfs:label "citing essay, or panoramic literary, philosophic or Humanities expression"@en, "zitierendes Essay, oder panoramisch literarisch, philosophisch oder geisteswissenschaftliche Expression"@de, "essai citant , ou expression littéraire panoramique et pittoresque, philosophique ou scientifique humaines"@fr; #, ""@it;
	rdfs:comment """Essay, or panoramic literary, philosophic or Humanities publication expression citing one or more verses of a poem authored by Jacques Delille."""@en;
	rdfs:subClassOf delille:LiteraryExpression.

delille:LiteraryNonfictionExpression
	rdfs:isDefinedBy <http://e-editiones.ch/ontology/delille#>;
	a rdfs:Class;
	rdfs:label "citing literary nonfiction expression"@en, "zitierende sachliche literarische Expression"@de, "expression littéraire non-fiction citante"@fr; #, ""@it;
	rdfs:comment """Literary nonfiction expression, e.g. historical, citing one or more verses of a poem authored by Jacques Delille, being a memoir, biography, history, anecdote, or correspondence."""@en;
	rdfs:subClassOf delille:LiteraryExpression, literature:NonfictionExpression.

delille:LiteraryScientificExpression
	rdfs:isDefinedBy <http://e-editiones.ch/ontology/delille#>;
	a rdfs:Class;
	rdfs:label "citing literary scientific expression"@en, "zitierende Literaturwissenschaftliche Expression"@de, "expression scientifique littéraire citante"@fr; #, ""@it;
	rdfs:comment """Literary scientific publication expression in esthetics, poetry and literary history, citing one or more verses of a poem authored by Jacques Delille."""@en;
	rdfs:subClassOf delille:LiteraryExpression, text-expression:ScientificExpression, delille:CitingExpression.

delille:ScientificOrVulgarizedExpression
	rdfs:isDefinedBy <http://e-editiones.ch/ontology/delille#>;
	a rdfs:Class;
	rdfs:label "citing scientific or vulgarized publication expression"@en, "zitierende wissenschaftliche oder vulgarisierte Publikation-Expression"@de;
	rdfs:comment """Natural scientific or vulgarized publication expression citing one or more verses of a poem authored by Jacques Delille."""@en;
	rdfs:subClassOf text-expression:ScientificExpression, delille:CitingExpression.

delille:Catalogue
	rdfs:isDefinedBy <http://e-editiones.ch/ontology/delille#>;
	a rdfs:Class;
	rdfs:label "citing catalogue"@en, "zitierende Katalog"@de;
	rdfs:comment """Catalogue citing one or more verses of a poem authored by Jacques Delille."""@en;
	rdfs:subClassOf document:Catalogue, delille:CitingExpression.

delille:Article
	rdfs:isDefinedBy <http://e-editiones.ch/ontology/delille#>;
	a rdfs:Class;
	rdfs:label "citing article"@en, "zitierender Artikel"@de;
	rdfs:comment """Publication article citing one or more verses of a poem authored by Jacques Delille."""@en;
	rdfs:subClassOf publish:Article, delille:CitingExpression.

delille:NonOriginalEngraving
	rdfs:isDefinedBy <http://e-editiones.ch/ontology/delille#>;
	a rdfs:Class;
	rdfs:label "non-original engraving expression"@en,"nicht-originale Gravurexpression"@de;
	rdfs:comment """Image that is not an original engraving, as part of a Delille citing text expression. This image can be a painting, drawing, or engraving different from the original."""@en;
	rdfs:subClassOf image:Expression.

delille:Argument
	rdfs:isDefinedBy <http://e-editiones.ch/ontology/delille#>;
	a rdfs:Class;
	rdfs:label "argument"@en, "Argument"@de;
	rdfs:comment """Argument of a commentary on a citation of a verse of a poem authored by Jacques Delille."""@en;
	rdfs:subClassOf literature:Argument, publish:TextExpression.

delille:NonArtist-ManOfLetters-Vulgarizer
	rdfs:isDefinedBy <http://e-editiones.ch/ontology/delille#>;
	a rdfs:Class;
	rdfs:label "non-artist-man of letters-vulgarizer"@en, "Non-KünstlerIn-Literat-VulgarisatorIn"@de;
	rdfs:comment """Role of a person which is not artist, man of letters, or vulgarizer."""@en;
	rdfs:subClassOf human:PersonRole;
	owl:disjointWith human:Artist, text-expression:ManOfLetters, text-expression:Vulgarizer.

delille:ScholarlyEdition
	rdfs:isDefinedBy <http://e-editiones.ch/ontology/delille#>;
	a rdfs:Class;
	rdfs:label "Jacques Delille verse poem scholarly edition"@en, "wissenschaftliche Edition eines Versgedichtes Jacques Delilles"@de;
	rdfs:comment """Scholarly edition of a verse poem authored by Jacques Delille."""@en;
	rdfs:subClassOf scholarly-editing:Edition, publish:TextExpression.

delille:Commentary
	rdfs:isDefinedBy <http://e-editiones.ch/ontology/delille#>;
	a rdfs:Class;
	rdfs:label "commentary"@en, "Kommentar"@de;
	rdfs:comment """Commentary on a citation of a verse of a poem authored by Jacques Delille."""@en;
	rdfs:subClassOf text-expression:Commentary, text-expression:ScientificExpression, publish:TextExpression.

#
# PROPERTIES
#

delille:hasExternalResource
	rdfs:isDefinedBy <http://e-editiones.ch/ontology/delille#>;
	a owl:ObjectProperty;
	rdfs:label "has external resource"@en, "hat externe Ressource"@de;
	rdfs:comment """Relating a Delille-project resource to an external, i.e. non-Delille-project resource."""@en;
	rdfs:domain rdfs:Resource;
	rdfs:range rdfs:Resource.

delille:hasPunctuatedCitedVerseNumberSequenceLiteral
	rdfs:isDefinedBy <http://e-editiones.ch/ontology/delille#>;
	a owl:DatatypeProperty;
	rdfs:label "has punctuated cited verse number sequence literal"@en, "hat interpunktierte citierter Versnummersequenzliterale"@de;
	rdfs:comment """Relating a text expression, citing one or more verses of a poem authored by Jacques Delille, to its punctuated cited verse number sequence literal."""@en;
	skos:note """Used in the conclusion of an N3-rule invoking in the premise a backward N3-rule to replace in a sequence of non-negative integers inner consecutive NNIs with a hyphen and separate non-consecutive NNIs with a comma."""@en;
	rdfs:domain delille:CitingExpression;
	rdfs:range rdfs:Literal.

delille:verseHasNumberOfCitations
	rdfs:isDefinedBy <http://e-editiones.ch/ontology/delille#>;
	a owl:DatatypeProperty;
	rdfs:label "verse has number of citations"@en, "Vers hat Anzahl von Zitaten"@de;
	rdfs:comment """Relating a verse of 'L'Homme Des Champs' to the number of expressions wherein cited."""@en;
	skos:note """Used in an N3-rule to count for a verse the number of citations."""@en;
	rdfs:domain prosodic-structure:RhymingVerse;
	rdfs:range xsd:nonNegativeInteger.

delille:verseHasHighestNumberOfCitations
	rdfs:isDefinedBy <http://e-editiones.ch/ontology/delille#>;
	a owl:DatatypeProperty;
	rdfs:label "verse has highest number of citations"@en, "Vers hat höchste Anzahl von Zitaten"@de;
	rdfs:comment """Relating a verse of 'L'Homme Des Champs' to the highest number of citations of all verses."""@en;
	skos:note """Used in an N3-rule to count for a verse the highest number of citations."""@en;
	rdfs:domain prosodic-structure:RhymingVerse;
	rdfs:range xsd:nonNegativeInteger.

delille:verseHasLowestNumberOfCitations
	rdfs:isDefinedBy <http://e-editiones.ch/ontology/delille#>;
	a owl:DatatypeProperty;
	rdfs:label "verse has lowest number of citations"@en, "Vers hat geringste Anzahl von Zitaten"@de;
	rdfs:comment """Relating a verse of 'L'Homme Des Champs' to the lowest number of citations of all verses."""@en;
	skos:note """Used in an N3-rule to count for a verse the lowest number of citations."""@en;
	rdfs:domain prosodic-structure:RhymingVerse;
	rdfs:range xsd:nonNegativeInteger.

delille:verseHasNumberOfCiters
	rdfs:isDefinedBy <http://e-editiones.ch/ontology/delille#>;
	a owl:DatatypeProperty;
	rdfs:label "verse has number of citers"@en, "Vers hat Anzahl der ZitiererInnen"@de;
	rdfs:comment """Relating a verse of 'L'Homme Des Champs' to the number of citers it has."""@en;
	skos:note """Used in an N3-rule to count for a verse the number of citers."""@en;
	rdfs:domain prosodic-structure:RhymingVerse;
	rdfs:range xsd:nonNegativeInteger.

delille:hasCitingAgeNumeral
	rdfs:isDefinedBy <http://e-editiones.ch/ontology/delille#>;
	a owl:DatatypeProperty;
	rdfs:label "has citing age numeral"@en, "hat Zitierungsalternumerale"@de;
	rdfs:comment """Relating a person who cited a verse of 'L'Homme Des Champs' to the person's age at citing."""@en;
	skos:note """Used in an N3-rule to calculate for a person the age at citing."""@en;
	rdfs:domain [rdfs:subClassOf human:Person, [a owl:Restriction; owl:onProperty human:personHasRole; owl:someValuesFrom text:PersonCiter]];
	rdfs:range xsd:positiveInteger.

delille:hasCitingAgeRangeLiteral
	rdfs:isDefinedBy <http://e-editiones.ch/ontology/delille#>;
	a owl:DatatypeProperty;
	rdfs:label "has citing age range literal"@en, "hat Zitierungsaltersbereichliterale"@de;
	rdfs:comment """Relating a person who cited a verse of 'L'Homme Des Champs' to the person's age range at citing."""@en;
	skos:note """Used in an N3-rule to calculate for a person the age range at citing."""@en;
	rdfs:domain [rdfs:subClassOf human:Person, [a owl:Restriction; owl:onProperty human:personHasRole; owl:someValuesFrom text:PersonCiter]];
	rdfs:range rdfs:Literal.

delille:verseHasNumberOfCiterAgeRangeLiterals
	rdfs:isDefinedBy <http://e-editiones.ch/ontology/delille#>;
	a owl:DatatypeProperty;
	rdfs:label " verse has number of citer age range literals"@en, "Vers hat Anzahl der ZitiererInsaltersbereichliterale"@de;
	rdfs:comment """Relating a verse of 'L'Homme Des Champs' to the number of ranges of the ages of the persons who cited that verse."""@en;
	skos:note """Used in an N3-rule to count for a verse the number of ranges of the ages of the persons who cited that verse."""@en;
	rdfs:domain prosodic-structure:RhymingVerse;
	rdfs:range xsd:nonNegativeInteger.

delille:hasClassSpecificCitedVerse
	rdfs:isDefinedBy <http://e-editiones.ch/ontology/delille#>;
	a owl:ObjectProperty;
	rdfs:label "has class-specific cited verse"@en;
	rdfs:comment """Relating a text expression to a verse of 'L'Homme des champs' it cites class-specifically, i.e. not cited in instances of another citing expression class."""@en;
	skos:note """The verse can also be cited in another expression instance of the same class."""@en;
	skos:note """Used in the conclusion of an N3-rule to retrieve an expression citing a verse specific for the expression class, with the cited verse."""@en;
	rdfs:domain delille:CitingExpression;
	rdfs:range prosodic-structure:RhymingVerse.

delille:hasPunctuatedClassSpecificCitedVerseNumberSequenceLiteral
	rdfs:isDefinedBy <http://e-editiones.ch/ontology/delille#>;
	a owl:DatatypeProperty;
	rdfs:label "has punctuated class-specific cited verse number sequence literal"@en, "hat interpunktierte klassenspezifische citierter Versnummersequenzliterale"@de;
	rdfs:comment """Relating a text expression, citing class-specifically one or more verses of a poem authored by Jacques Delille, to its punctuated cited verse number sequence literal."""@en;
	skos:note """Used in the conclusion of an N3-rule invoking in the premise a backward N3-rule to replace in a sequence of non-negative integers inner consecutive NNIs with a hyphen and separate non-consecutive NNIs with a comma."""@en;
	rdfs:domain delille:CitingExpression;
	rdfs:range rdfs:Literal.

delille:hasUniqueCitedVerse
	rdfs:isDefinedBy <http://e-editiones.ch/ontology/delille#>;
	a owl:ObjectProperty;
	rdfs:label "has unique cited verse"@en;
	rdfs:comment """Relating a text expression to a verse of 'L'Homme des champs' it uniquely cites."""@en;
	skos:note """Used in the conclusion of an N3-rule to retrieve an expression uniquely citing a verse, with the cited verse."""@en;
	rdfs:domain delille:CitingExpression;
	rdfs:range prosodic-structure:RhymingVerse.

delille:hasPunctuatedUniquelyCitedVerseNumberSequenceLiteral
	rdfs:isDefinedBy <http://e-editiones.ch/ontology/delille#>;
	a owl:DatatypeProperty;
	rdfs:label "has punctuated unique cited verse number sequence literal"@en, "hat interpunktierte einmalige citierter Versnummersequenzliterale"@de;
	rdfs:comment """Relating a text expression, citing uniquely one or more verses of a poem authored by Jacques Delille, to its punctuated cited verse number sequence literal."""@en;
	skos:note """Used in the conclusion of an N3-rule invoking in the premise a backward N3-rule to replace in a sequence of non-negative integers inner consecutive NNIs with a hyphen and separate non-consecutive NNIs with a comma."""@en;
	rdfs:domain delille:CitingExpression;
	rdfs:range rdfs:Literal.

delille:verseHasNumberOfEarlyAnthologyOrManualAndDictionaryCitations
	rdfs:isDefinedBy <http://e-editiones.ch/ontology/delille#>;
	a owl:DatatypeProperty;
	rdfs:label "verse has number of early anthology or manual and dictionary citations"@en, "Vers hat frühe Anthologie- oder Lehrbuch- und Wörterbuch-Zitate"@de;
	rdfs:comment """Relating a verse of 'L'homme des champs' to the number of early anthologies or manuals, and dictionaries citing the verse."""@en;
	skos:note """Early means before the middle time point of the whole publication period of all expressions citing the verse."""@en;
	rdfs:domain [
		rdfs:subClassOf
			prosodic-structure:RhymingVerse, [
			a owl:Restriction; owl:onProperty text:isCitedIn; owl:someValuesFrom [owl:unionOf (delille:AnthologyOrManual delille:Dictionary)]]];
	rdfs:range xsd:nonNegativeInteger.

delille:verseHasNumberOfLateNonAnthologyOrManualAndDictionaryCitations
	rdfs:isDefinedBy <http://e-editiones.ch/ontology/delille#>;
	a owl:DatatypeProperty;
	rdfs:label "verse has number of late non-anthology or -manual and -dictionary citations"@en, "Vers hat späte Non-Anthologie- oder -Lehrbuch- und -Wörterbuch-Zitate"@de;
	rdfs:comment """Relating a verse of 'L'homme des champs' to the number of late text expressions, not being an anthology or manual, or dictionary, citing the verse."""@en;
	rdfs:domain [
		rdfs:subClassOf
			prosodic-structure:RhymingVerse, [
			a owl:Restriction; owl:onProperty text:isCitedIn; owl:someValuesFrom [owl:unionOf (delille:LiteraryExpression delille:LiteraryScientificExpression delille:ScientificOrVulgarizedExpression delille:Catalogue delille:Article)]]];
	rdfs:range xsd:nonNegativeInteger.

delille:verseHasNumberOfLateAnthologyOrManualAndDictionaryCitations
	rdfs:isDefinedBy <http://e-editiones.ch/ontology/delille#>;
	a owl:DatatypeProperty;
	rdfs:label "verse has number of late anthology or manual and dictionary citations"@en, "Vers hat späte Anthologie- oder Lehrbuch- und Wörterbuch-Zitate"@de;
	rdfs:comment """Relating a verse of 'L'homme des champs' to the number of late anthologies or manuals, and dictionaries citing the verse."""@en;
	rdfs:domain [
		rdfs:subClassOf
			prosodic-structure:RhymingVerse, [
			a owl:Restriction; owl:onProperty text:isCitedIn; owl:someValuesFrom [owl:unionOf (delille:AnthologyOrManual delille:Dictionary)]]];
	rdfs:range xsd:nonNegativeInteger.

delille:verseHasNumberOfEarlyNonAnthologyOrManualAndDictionaryCitations
	rdfs:isDefinedBy <http://e-editiones.ch/ontology/delille#>;
	a owl:DatatypeProperty;
	rdfs:label "verse has number of early non-anthology or -manual and -dictionary citations"@en, "Vers hat frühe Non-Anthologie- oder -Lehrbuch- oder -Wörterbuch-Zitate"@de;
	rdfs:comment """Relating a verse of 'L'homme des champs' to the number of early text expressions, not being an anthology or manual, or dictionary, citing the verse."""@en;
	rdfs:domain [
		rdfs:subClassOf
			prosodic-structure:RhymingVerse, [
			a owl:Restriction; owl:onProperty text:isCitedIn; owl:someValuesFrom [owl:unionOf (delille:LiteraryExpression delille:LiteraryScientificExpression delille:ScientificOrVulgarizedExpression delille:Catalogue delille:Article)]]];
	rdfs:range xsd:nonNegativeInteger.