@prefix rdfs: <http://www.w3.org/2000/01/rdf-schema#>.
@prefix owl: <http://www.w3.org/2002/07/owl#>.
@prefix xsd: <http://www.w3.org/2001/XMLSchema#>.
@prefix skos: <http://www.w3.org/2004/02/skos/core#>.
@prefix dct: <http://purl.org/dc/terms/>.
@prefix human: <http://e-editiones.ch/ontology/human#>.
@prefix cathord: <http://e-editiones.ch/ontology/catholic-order#>.
@prefix text: <http://e-editiones.ch/ontology/text#>.
@prefix text-expression: <http://e-editiones.ch/ontology/text-expression#>.
@prefix textedit: <http://e-editiones.ch/ontology/text-editing#>.
@prefix scholarly-editing: <http://e-editiones.ch/ontology/scholarly-editing#>.
@prefix infocar: <http://e-editiones.ch/ontology/information-carrier#>.

@base <http://e-editiones.ch/ontology/dietrich>.
@prefix dietrich: <http://e-editiones.ch/ontology/dietrich#>.

<http://e-editiones.ch/ontology/dietrich>
	a owl:Ontology;
	dct:license <http://creativecommons.org/licenses/by/3.0/>;
	dct:title "An ontology about father Joseph Dietrich's monastery diary"@en;
	dct:description """Formal description of specific concepts in the scientific study "Das Kloster-Tagebuch des Einsiedler Paters Joseph Dietrich, 1670-1704"."""@en;
	dct:creator "Hans Cools, MD, knowledge engineer, ontologist, software developer, University of Basel, Switzerland"@en;
	dct:contributor "Reinhard Priber, tool coordinator and software developer, University of Bern, Switzerland"@en;
	dct:publisher "Universities of Basel, Bern, and Zürich, Switzerland"@en;
	owl:versionInfo "2020-06-11"^^xsd:date.

#
# CLASSES
#

dietrich:DiaryEntry
	rdfs:isDefinedBy <http://e-editiones.ch/ontology/dietrich#>;
	a rdfs:Class;
	rdfs:label "diary entry by father Joseph Dietrich"@en, "Tagebucheintrag des Paters Joseph Dietrich"@de;
	rdfs:comment """Diary entry authored by father Joseph Dietrich."""@en;
	rdfs:subClassOf text:HandwrittenText, text-expression:DiaryEntry.

dietrich:DiaryVolume
	rdfs:isDefinedBy <http://e-editiones.ch/ontology/dietrich#>;
	a rdfs:Class;
	rdfs:label "diary volume by father Joseph Dietrich"@en, "Tagebuch-Band des Paters Joseph Dietrich"@de;
	rdfs:comment """Diary volume written and authored by father Joseph Dietrich."""@en;
	rdfs:subClassOf infocar:Manuscript, infocar:Diary, infocar:Volume.

#
# PROPERTIES
#

dietrich:hasExternalResource
	rdfs:isDefinedBy <http://e-editiones.ch/ontology/dietrich#>;
	a owl:ObjectProperty;
	rdfs:label "has external resource"@en, "hat externe Ressource"@de;
	rdfs:comment """Relating a Dietrich-project resource to an external, i.e. non-Dietrich-project resource."""@en;
	rdfs:domain rdfs:Resource;
	rdfs:range rdfs:Resource.

dietrich:personHasEinsiedlerProfessIdentifier
	rdfs:isDefinedBy <http://e-editiones.ch/ontology/dietrich#>;
	a owl:DatatypeProperty;
	rdfs:label "person has Einsiedler profess identifier"@en, "Person hat Einsiedler-Eintrittidentifikator"@de;
	rdfs:comment """Relating a catholic order person to an identifier for being professed into the order of the monastery of Einsiedeln."""@en;
	rdfs:domain cathord:Person;
	rdfs:range rdfs:Literal.

dietrich:personHasStGallerProfessIdentifier
	rdfs:isDefinedBy <http://e-editiones.ch/ontology/dietrich#>;
	a owl:DatatypeProperty;
	rdfs:label "person has St. Galler profess identifier"@en, "Person hat St. Galler-Eintrittidentifikator"@de;
	rdfs:comment """Relating a catholic order person to an identifier for being professed into the order of the monastery of St. Gallen."""@en;
	rdfs:domain cathord:Person;
	rdfs:range rdfs:Literal.

dietrich:personHasPfaeferserProfessIdentifier
	rdfs:isDefinedBy <http://e-editiones.ch/ontology/dietrich#>;
	a owl:DatatypeProperty;
	rdfs:label "person has Pfäferser profess identifier"@en, "Person hat St. Pfäferser-Eintrittidentifikator"@de;
	rdfs:comment """Relating a catholic order person to an identifier for being professed into the order of the monastery of Pfäfers."""@en;
	rdfs:domain cathord:Person;
	rdfs:range rdfs:Literal.

dietrich:personHasNonEinsiedler-StGaller-PfaeferserProfessIdentifier
	rdfs:isDefinedBy <http://e-editiones.ch/ontology/dietrich#>;
	a owl:DatatypeProperty;
	rdfs:label "person has non-Einsiedler-StGaller-Pfaeferser profess identifier"@en, "Person hat non-Einsiedler-StGaller-Pfaeferser-Eintrittidentifikator"@de;
	rdfs:comment """Relating a catholic order person to an identifier for being professed into the order of the monastery other than the one of Einsiedeln, St. Gallen, and Pfäfers."""@en;
	rdfs:domain cathord:Person;
	rdfs:range rdfs:Literal.

dietrich:personHasEinsiedlerAbbot
	rdfs:isDefinedBy <http://e-editiones.ch/ontology/dietrich#>;
	a owl:ObjectProperty;
	rdfs:label "person has Einsiedler abbot"@en, "Person hat Einsiedler-Abt"@de;
	rdfs:comment """Relating a catholic order person to the person being the abbot of the monastery of Einsiedeln."""@en;
	rdfs:domain cathord:Person;
	rdfs:range cathord:Person, [a owl:Restriction; owl:onProperty human:personHasRole; owl:someValuesFrom cathord:Abbot].