@prefix rdfs: <http://www.w3.org/2000/01/rdf-schema#>.
@prefix owl: <http://www.w3.org/2002/07/owl#>.
@prefix xsd: <http://www.w3.org/2001/XMLSchema#>.
@prefix skos: <http://www.w3.org/2004/02/skos/core#>.
@prefix dct: <http://purl.org/dc/terms/>.
@prefix text: <http://www.e-editiones.ch/ontology/text#>.
@prefix text-expression: <http://www.e-editiones.ch/ontology/text-expression#>.
@prefix textedit: <http://www.e-editiones.ch/ontology/text-editing#>.
@prefix scholarly-editing: <http://www.e-editiones.ch/ontology/scholarly-editing#>.
@prefix infocar: <http://www.e-editiones.ch/ontology/information-carrier#>.
@prefix letter-corresponding: <http://www.e-editiones.ch/ontology/letter-corresponding#>.

# @base <http://www.e-editiones.ch/ontology/lavater>.
@prefix lavater: <http://www.e-editiones.ch/ontology/lavater#>.

<http://www.e-editiones.ch/ontology/lavater>
	a owl:Ontology;
	dct:license <http://creativecommons.org/licenses/by/3.0/>;
	dct:title "An ontology about Johann Caspar Lavater's correspondence"@en;
	dct:description """Formal description of specific concepts in the critical edition of correspondence of Johann Caspar Lavater, 15 November 1741 - 2 January 1801."""@en;
	dct:creator "Hans Cools, MD, knowledge engineer, ontologist, software developer, Basel University, Switzerland"@en;
	dct:contributor "Reto Baumgartner, tool coordinator and software developer, University of Zürich, Switzerland"@en;
	dct:publisher "Universities of Basel, Bern, and Zürich, Switzerland"@en.

#
# CLASSES
#

lavater:LetterExpression
	rdfs:isDefinedBy <http://www.e-editiones.ch/ontology/lavater#>;
	a rdfs:Class;
	rdfs:label "Johann Caspar Lavater letter expression"@en, "Brief-Expression Johann Caspar Lavaters"@de;
	rdfs:comment """Letter expression either authored by or written to by Johann Caspar Lavater."""@en;
	rdfs:subClassOf letter-corresponding:Expression, text:HandwrittenText.

lavater:Letter
	rdfs:isDefinedBy <http://www.e-editiones.ch/ontology/lavater#>;
	a rdfs:Class;
	rdfs:label "Johann Caspar Lavater letter"@en, "Johann Caspar Lavater-Brief"@de, "lettre de Johann Caspar Lavater"@fr, "lettera di Johann Caspar Lavater"@it;
	rdfs:comment """Letter send by or to Johann Caspar Lavater."""@en;
	rdfs:subClassOf letter-corresponding:Letter, infocar:ConvoluteElement, infocar:ArchiveElement.

lavater:Page
	rdfs:isDefinedBy <http://www.e-editiones.ch/ontology/lavater#>;
	a rdfs:Class;
	rdfs:label "Johann Caspar Lavater letter page"@en, "Seite eines Briefes Johann Caspar Lavaters"@de;
	rdfs:comment """Page of a letter of Johann Caspar Lavater."""@en;
	rdfs:subClassOf infocar:Page.
#	hasRepresentation

lavater:LetterConvolute
	rdfs:isDefinedBy <http://www.e-editiones.ch/ontology/lavater#>;
	a rdfs:Class;
	rdfs:label "Johann Caspar Lavater letter convolute"@en,"Briefekonvolut Johann Caspar Lavaters"@de;
	rdfs:comment """Convolute of letters send by and to Johann Caspar Lavater."""@en;
	rdfs:subClassOf infocar:Convolute, infocar:ArchiveElement.

lavater:EditedLetter
	rdfs:isDefinedBy <http://www.e-editiones.ch/ontology/lavater#>;
	a rdfs:Class;
	rdfs:label "edited Johann Caspar Lavater letter expression"@en, "edierter Brief-Expression Johann Caspar Lavaters"@de;
	rdfs:comment """Letter expression either authored or received by Johann Caspar Lavater, and critically edited."""@en;
	rdfs:subClassOf scholarly-editing:CriticalEdition.
