@prefix rdfs: <http://www.w3.org/2000/01/rdf-schema#>.
@prefix owl: <http://www.w3.org/2002/07/owl#>.
@prefix xsd: <http://www.w3.org/2001/XMLSchema#>.
@prefix skos: <http://www.w3.org/2004/02/skos/core#>.
@prefix dct: <http://purl.org/dc/terms/>.
@prefix text: <http://www.e-editiones.ch/ontology/text#>.
@prefix text-expression: <http://www.e-editiones.ch/ontology/text-expression#>.
@prefix textedit: <http://www.e-editiones.ch/ontology/text-editing#>.
@prefix scholarly-editing: <http://www.e-editiones.ch/ontology/scholarly-editing#>.
@prefix infocar: <http://www.e-editiones.ch/ontology/information-carrier#>.
@prefix publish: <http://www.e-editiones.ch/ontology/publishing#>.
@prefix letter-corresponding: <http://www.e-editiones.ch/ontology/letter-corresponding#>.

# @base <http://www.e-editiones.ch/ontology/meyer>.
@prefix meyer: <http://www.e-editiones.ch/ontology/meyer#>.

<http://www.e-editiones.ch/ontology/meyer>
	a owl:Ontology;
	dct:license <http://creativecommons.org/licenses/by/3.0/>;
	dct:title "An ontology about Conrad Ferdinand Meyer's correspondence"@en;
	dct:description """Formal description of specific concepts in the critical edition of the correspondence of Conrad Ferdinand Meyer, 11 October 1825 – 28 November 1898."""@en;
	dct:creator "Hans Cools, MD, knowledge engineer, ontologist, software developer, Basel University, Switzerland"@en;
	dct:contributor "Reto Baumgartner, tool coordinator and software developer, University of Zürich, Switzerland"@en;
	dct:publisher "Universities of Basel, Bern, and Zürich, Switzerland"@en.

#
# CLASSES
#

meyer:LetterExpression
	rdfs:isDefinedBy <http://www.e-editiones.ch/ontology/meyer#>;
	a rdfs:Class;
	rdfs:label "Conrad Ferdinand Meyer letter expression"@en, "Briefexpression Conrad Ferdinand Meyers"@de;
	rdfs:comment """Letter expression authored by Conrad Ferdinand Meyer or another person."""@en;
	rdfs:subClassOf letter-corresponding:Expression, text:HandwrittenText.

meyer:DraftLetterExpression
	rdfs:isDefinedBy <http://www.e-editiones.ch/ontology/meyer#>;
	a rdfs:Class;
	rdfs:label "Conrad Ferdinand Meyer letter expression draft"@en, "Briefexpressionentwurf Conrad Ferdinand Meyers"@de;
	rdfs:comment """Draft of a letter expression authored by Conrad Ferdinand Meyer or another person."""@en;
	rdfs:subClassOf text-expression:Draft.

meyer:CopiedLetterExpression
	rdfs:isDefinedBy <http://www.e-editiones.ch/ontology/meyer#>;
	a rdfs:Class;
	rdfs:label "Conrad Ferdinand Meyer copied letter expression"@en, "kopierte Briefexpression Conrad Ferdinand Meyers"@de;
	rdfs:comment """Copied text of a letter expression authored by Conrad Ferdinand Meyer or another person, and being a witness of the original."""@en;
	rdfs:subClassOf scholarly-editing:Witness.

meyer:TranscribedLetterExpression
	rdfs:isDefinedBy <http://www.e-editiones.ch/ontology/meyer#>;
	a rdfs:Class;
	rdfs:label "Conrad Ferdinand Meyer transcribed letter expression"@en, "transkribierte Briefexpression Conrad Ferdinand Meyers"@de;
	rdfs:comment """Transcribed text of a letter expression authored by Conrad Ferdinand Meyer or another person."""@en;
	rdfs:subClassOf meyer:CopiedLetterExpression, text:TranscribedText.

meyer:PrintedLetterExpression
	rdfs:isDefinedBy <http://www.e-editiones.ch/ontology/meyer#>;
	a rdfs:Class;
	rdfs:label "Conrad Ferdinand Meyer printed letter expression"@en, "gedruckte Briefexpression Conrad Ferdinand Meyers"@de;
	rdfs:comment """Printed text of a letter expression authored by Conrad Ferdinand Meyer or another person."""@en;
	rdfs:subClassOf meyer:CopiedLetterExpression, text:PrintedText.

meyer:PhotocopiedLetterExpression
	rdfs:isDefinedBy <http://www.e-editiones.ch/ontology/meyer#>;
	a rdfs:Class;
	rdfs:label "Conrad Ferdinand Meyer photocopied letter expression"@en, "fotokopierte Briefexpression Conrad Ferdinand Meyers"@de;
	rdfs:comment """Photocopied text of a letter expression authored by Conrad Ferdinand Meyer or another person."""@en;
	rdfs:subClassOf meyer:CopiedLetterExpression, text:PhotocopiedText.

meyer:Letter
	rdfs:isDefinedBy <http://www.e-editiones.ch/ontology/meyer#>;
	a rdfs:Class;
	rdfs:label "Conrad Ferdinand Meyer letter"@en, "Conrad Ferdinand Meyer-Brief"@de, "lettre de Conrad Ferdinand Meyer"@fr, "lettera di Conrad Ferdinand Meyer"@it;
	rdfs:comment """Letter send by or to Conrad Ferdinand Meyer."""@en;
	rdfs:subClassOf letter-corresponding:Letter, infocar:ArchiveElement.

meyer:PostcardLetter
	rdfs:isDefinedBy <http://www.e-editiones.ch/ontology/meyer#>;
	a rdfs:Class;
	rdfs:label "Conrad Ferdinand Meyer postcard letter"@en, "Conrad Ferdinand Meyer-Postkartebrief"@de, "lettre carte postale de Conrad Ferdinand Meyer"@fr, "lettera cartolina di Conrad Ferdinand Meyer"@it;
	rdfs:comment """Letter written on a postcard send by or to Conrad Ferdinand Meyer."""@en;
	rdfs:subClassOf infocar:Postcard, meyer:Letter.

meyer:DraftLetter
	rdfs:isDefinedBy <http://www.e-editiones.ch/ontology/meyer#>;
	a rdfs:Class;
	rdfs:label "Conrad Ferdinand Meyer draft letter"@en, "Conrad Ferdinand Meyer-briefentwurf"@de;
	rdfs:comment """Draft of a letter to be sent by or to Conrad Ferdinand Meyer."""@en;
	rdfs:subClassOf infocar:Draft, infocar:ArchiveElement.

meyer:Copy
	rdfs:isDefinedBy <http://www.e-editiones.ch/ontology/meyer#>;
	a rdfs:Class;
	rdfs:label "Conrad Ferdinand Meyer letter copy"@en, "Conrad Ferdinand Meyer-Briefkopie"@de; #, "lettre de Conrad Ferdinand Meyer"@fr, "lettera di Conrad Ferdinand Meyer"@it;
	rdfs:comment """Copy of a letter send by or to Conrad Ferdinand Meyer."""@en;
	rdfs:subClassOf infocar:TextCopy, infocar:ArchiveElement.

meyer:Transcript
	rdfs:isDefinedBy <http://www.e-editiones.ch/ontology/meyer#>;
	a rdfs:Class;
	rdfs:label "Conrad Ferdinand Meyer letter transcript"@en, "Conrad Ferdinand Meyer-Brieftranskript"@de; #, "lettre de Conrad Ferdinand Meyer"@fr, "lettera di Conrad Ferdinand Meyer"@it;
	rdfs:comment """Transcribed copy of a letter send by or to Conrad Ferdinand Meyer."""@en;
	rdfs:subClassOf infocar:ManualTranscript, meyer:Copy.

meyer:Print
	rdfs:isDefinedBy <http://www.e-editiones.ch/ontology/meyer#>;
	a rdfs:Class;
	rdfs:label "Conrad Ferdinand Meyer letter print"@en, "Conrad Ferdinand Meyer-Briefdruck"@de; #, "lettre de Conrad Ferdinand Meyer"@fr, "lettera di Conrad Ferdinand Meyer"@it;
	rdfs:comment """Printed copy of a letter send by or to Conrad Ferdinand Meyer."""@en;
	rdfs:subClassOf infocar:Print, meyer:Copy.

meyer:FirstPrint
	rdfs:isDefinedBy <http://www.e-editiones.ch/ontology/meyer#>;
	a rdfs:Class;
	rdfs:label "Conrad Ferdinand Meyer letter first print"@en, "Conrad Ferdinand Meyer-Erstebriefdruck"@de; #, "lettre de Conrad Ferdinand Meyer"@fr, "lettera di Conrad Ferdinand Meyer"@it;
	rdfs:comment """First printed copy of a letter send by or to Conrad Ferdinand Meyer."""@en;
	rdfs:subClassOf infocar:FirstPrint, meyer:Print.

meyer:Photocopy
	rdfs:isDefinedBy <http://www.e-editiones.ch/ontology/meyer#>;
	a rdfs:Class;
	rdfs:label "Conrad Ferdinand Meyer letter photocopy"@en, "Conrad Ferdinand Meyer-Brieffotokopie"@de; #, "lettre de Conrad Ferdinand Meyer"@fr, "lettera di Conrad Ferdinand Meyer"@it;
	rdfs:comment """Photocopy of a letter send by or to Conrad Ferdinand Meyer."""@en;
	rdfs:subClassOf infocar:Photocopy, meyer:Copy.

meyer:Page
	rdfs:isDefinedBy <http://www.e-editiones.ch/ontology/meyer#>;
	a rdfs:Class;
	rdfs:label "Conrad Ferdinand Meyer letter page"@en, "Seite eines Briefes Conrad Ferdinand Meyers"@de;
	rdfs:comment """Page of a letter of Conrad Ferdinand Meyer."""@en;
	rdfs:subClassOf infocar:Page.

meyer:LetterConvolute
	rdfs:isDefinedBy <http://www.e-editiones.ch/ontology/meyer#>;
	a rdfs:Class;
	rdfs:label "Conrad Ferdinand Meyer letter convolute"@en,"Briefekonvolut Conrad Ferdinand Meyers"@de;
	rdfs:comment """Convolute of letters send by and to Conrad Ferdinand Meyer."""@en;
	rdfs:subClassOf infocar:Convolute, infocar:ArchiveElement.

meyer:CriticalEdition
	rdfs:isDefinedBy <http://www.e-editiones.ch/ontology/meyer#>;
	a rdfs:Class;
	rdfs:label "Conrad Ferdinand Meyer critical edition"@en, "Conrad Ferdinand Meyers kritische Edition"@de;
	rdfs:comment """Critically edited letter or draft authored by Conrad Ferdinand Meyer or another person, or of a copy thereof."""@en;
	rdfs:subClassOf scholarly-editing:CriticalEdition, publish:Expression.

#
# PROPERTIES
#