@prefix rdfs: <http://www.w3.org/2000/01/rdf-schema#>.
@prefix owl: <http://www.w3.org/2002/07/owl#>.
@prefix xsd: <http://www.w3.org/2001/XMLSchema#>.
@prefix skos: <http://www.w3.org/2004/02/skos/core#>.
@prefix dct: <http://purl.org/dc/terms/>.
@prefix human: <http://www.knora.org/ontology/0000/human#>.
@prefix philo: <http://www.knora.org/ontology/0000/philosophy#>.
@prefix knora-base: <http://www.knora.org/ontology/knora-base#>.

@base <http://www.knora.org/ontology/0000/philosophies>.
@prefix philos: <http://www.knora.org/ontology/0000/philosophies#>.

<http://www.knora.org/ontology/0000/philosophies>
	a owl:Ontology;
	dct:title "An ontology about philosophies"@en;
	dct:description """Formal description of philosophies, general subclasses, related classes, properties, and instances."""@en;
	dct:creator "Hans Cools, MD, knowledge engineer, ontologist, software developer, NIE-INE, Basel University, Switzerland"@en;
	dct:contributor "Prof. Dr. Ueli Zahnd, Faculty of Theology, University of Basel, Switzerland"@en, "Gabriel Müller, Faculty of Theology, University of Basel, Switzerland"@en;

	knora-base:attachedToProject <http://www.knora.org/ontology/knora-base#DefaultSharedOntologiesProject>. # <http://rdfh.ch/projects/0052>.

#
# INSTANCES
#

philos:Albertism
	a owl:Class;
	#rdfs:isDefinedBy <http://www.knora.org/ontology/0000/philosophies#>;
	rdfs:label "Albertism"@en;
	rdfs:comment """Theological ideas of Albertus Magnus, 13th-century German Scholastic philosopher."""@en; #*
	rdfs:subClassOf philo:Philosophy. # :Theology

philos:Humanism
	a owl:Class;
	#rdfs:isDefinedBy <http://www.knora.org/ontology/0000/philosophies#>;
	rdfs:label "Humanism"@en;
	rdfs:comment """."""@en; #*
	rdfs:subClassOf philo:Philosophy.

philos:Nominalism #** existing?
	a owl:Class;
	#rdfs:isDefinedBy <http://www.knora.org/ontology/0000/philosophies#>;
	rdfs:label "Nominalism"@en;
	rdfs:comment """Phylosophy stating that only individual things exist, denying the existence of universals and abstract objects."""@en;
	rdfs:subClassOf philo:Metaphysics.

philos:Scotism
	a owl:Class;
	#rdfs:isDefinedBy <http://www.knora.org/ontology/0000/philosophies#>;
	rdfs:label "Scotism"@en;
	rdfs:comment """."""@en; #*
	rdfs:subClassOf philo:Philosophy.

philos:Thomism
	a owl:Class;
	#rdfs:isDefinedBy <http://www.knora.org/ontology/0000/philosophies#>;
	rdfs:label "Thomism"@en;
	rdfs:comment """Phylosophy base on the work of Thomas Aquinas (1225 - 1274-O3-O7)."""@en;
	rdfs:subClassOf philo:Philosophy. # :Theology

#* Averroes?
#* Augustinus? - Augustinianism - Augustine of Hippo

#
# PROPERTIES
#

philos:adheringToThought
	a owl:ObjectProperty;
	rdfs:label "adhering to philosophy"@en, "ist Anhänger von Philosophie"@de;
	rdfs:comment """Relating a person to a philosophy the person adheres to."""@en;
	rdfs:domain human:Person;
	rdfs:range philo:Philosophy;
	rdfs:subPropertyOf human:adheringToThought;
	knora-base:subjectClassConstraint human:Person;
	knora-base:objectClassConstraint philo:Philosophy.

philos:adheringToThoughtValue
	a owl:ObjectProperty;
	rdfs:label "adhering to philosophy - statement"@en, "ist Anhänger von Philosophie - Festlegung"@de;
	rdfs:comment """Relating a person to a reification statement of the relation between the person and a philosophy the person adheres to."""@en;
	rdfs:subPropertyOf human:adheringToThoughtValue;
	knora-base:subjectClassConstraint human:Person;
	knora-base:objectClassConstraint knora-base:LinkValue.