@prefix rdfs: <http://www.w3.org/2000/01/rdf-schema#>.
@prefix owl: <http://www.w3.org/2002/07/owl#>.
@prefix xsd: <http://www.w3.org/2001/XMLSchema#>.
@prefix skos: <http://www.w3.org/2004/02/skos/core#>.
@prefix dct: <http://purl.org/dc/terms/>.
@prefix cidoc: <http://www.cidoc-crm.org/cidoc-crm/>.
@prefix human: <http://www.knora.org/ontology/0048/human#>.
@prefix concept: <http://www.knora.org/ontology/0044/concept#>.
@prefix language: <http://www.knora.org/ontology/004F/language#>.
@prefix text: <http://www.knora.org/ontology/0059/text#>.
@prefix text-structure: <http://www.knora.org/ontology/005B/text-structure#>.
@prefix textedit: <http://www.knora.org/ontology/005A/text-editing#>.
@prefix ling: <http://www.knora.org/ontology/005D/linguistics#>.
@prefix logic: <http://www.knora.org/ontology/005E/logic#>.
@prefix knora-base: <http://www.knora.org/ontology/knora-base#>.

@base <http://www.knora.org/ontology/0057/scholasticism>.
@prefix schola: <http://www.knora.org/ontology/0057/scholasticism#>.

<http://www.knora.org/ontology/0057/scholasticism>
	a owl:Ontology;
	dct:title "An ontology about Scholasticism"@en;
	dct:description """Formal description of elements in Scholasticism."""@en;
	dct:creator "Hans Cools, MD, knowledge engineer, ontologist, software developer, NIE, University of Basel, Switzerland"@en;
	dct:contributor "Prof. Dr. Ueli Zahnd, Faculty of Theology, University of Basel, Switzerland"@en, "Gabriel Müller, Faculty of Theology, University of Basel, Switzerland"@en;
	dct:publisher "Basel University, Switzerland"@en;

	knora-base:attachedToProject <http://rdfh.ch/projects/0057>.

#
# CLASSES
#

schola:Scholasticism
	a owl:Class;
	rdfs:label "scholasticism"@en, "Scholastik"@de;
	rdfs:comment """Method of critical thought dominating theological and philosophical study in Western Christianity and teaching by academics or scholastics (schoolmen) of universities in Europe from about 1100 to 1700."""@en;
	rdfs:subClassOf concept:ThoughtMethod. #*

schola:Scholastic
	a owl:Class;
	rdfs:label "scholastic"@en, "ScholastikerIn"@de;
	rdfs:comment """An adherent of Scholasticism."""@en;
	skos:note """There are no female scholastics because women were not allowed to universities."""@en; # Can this be stated that absolute?
	rdfs:subClassOf human:Person, [
#		a owl:Restriction; owl:onProperty schola:hasRole; owl:someValuesFrom schola:Role], [
		a owl:Restriction; owl:onProperty schola:hasRole; owl:minCardinality "0"^^xsd:nonNegativeInteger], [
		a owl:Restriction; owl:onProperty schola:hasRoleValue; owl:minCardinality "0"^^xsd:nonNegativeInteger] #, [
#		a owl:Restriction; owl:onProperty schola:hasReportatorRole; owl:minCardinality "0"^^xsd:nonNegativeInteger], [
#		a owl:Restriction; owl:onProperty schola:hasReportatorRoleValue; owl:minCardinality "0"^^xsd:nonNegativeInteger]
		.

#* schola:Translator: SCO text:Translator: handwriting?

schola:Role
	a owl:Class;
	rdfs:label "scholastic role"@en;
	rdfs:comment """Role a scholastic has."""@en;
	rdfs:subClassOf human:Role.

schola:Reportator
	a owl:Class;
	rdfs:label "reportator"@la, "reportator"@en, "Reportator"@de;
	rdfs:comment """Role of a scholastic student registering the content of a lesson."""@en; #* also secretary of lecturer, RP
	rdfs:subClassOf schola:Role.

# schola:Expression
#	a owl:Class;
#	rdfs:label "scholastic expression"@en, "scholastischer Expression"@de;
#	rdfs:comment """Expression created by a scholastic."""@en;
#	rdfs:subClassOf concept:Expression.

schola:Commentary
	a owl:Class;
	rdfs:label "commentarius scholasticus"@la, "scholastic commentary"@en, "scholastischer Kommentar"@de;
	rdfs:comment """Commentary made by a scholastic."""@en;
	rdfs:subClassOf text:Commentary, [
#*		a owl:Restriction; owl:onProperty schola:commentaryHasProcedure; owl:minCardinality "0"^^xsd:nonNegativeInteger], [
#*		a owl:Restriction; owl:onProperty schola:commentaryHasProcedureValue; owl:minCardinality "0"^^xsd:nonNegativeInteger], [
		a owl:Restriction; owl:onProperty schola:commentaryHasForm; owl:minCardinality "0"^^xsd:nonNegativeInteger], [
		a owl:Restriction; owl:onProperty schola:commentaryHasFormValue; owl:minCardinality "0"^^xsd:nonNegativeInteger], [
		a owl:Restriction; owl:onProperty schola:commentaryHasGloss; owl:minCardinality "0"^^xsd:nonNegativeInteger], [
		a owl:Restriction; owl:onProperty schola:commentaryHasGlossValue; owl:minCardinality "0"^^xsd:nonNegativeInteger], [
		a owl:Restriction; owl:onProperty schola:commentaryHasVerse; owl:minCardinality "0"^^xsd:nonNegativeInteger], [
		a owl:Restriction; owl:onProperty schola:commentaryHasVerseValue; owl:minCardinality "0"^^xsd:nonNegativeInteger], [
		a owl:Restriction; owl:onProperty schola:commentaryHasTable; owl:minCardinality "0"^^xsd:nonNegativeInteger], [
		a owl:Restriction; owl:onProperty schola:commentaryHasTableValue; owl:minCardinality "0"^^xsd:nonNegativeInteger], [
		a owl:Restriction; owl:onProperty schola:commentaryHasAbbreviation; owl:minCardinality "0"^^xsd:nonNegativeInteger], [ #* concerns whole expression ?
		a owl:Restriction; owl:onProperty schola:commentaryHasAbbreviationValue; owl:minCardinality "0"^^xsd:nonNegativeInteger], [
		a owl:Restriction; owl:onProperty schola:commentaryHasParaphrase; owl:minCardinality "0"^^xsd:nonNegativeInteger], [ #* concerns whole expression
		a owl:Restriction; owl:onProperty schola:commentaryHasParaphraseValue; owl:minCardinality "0"^^xsd:nonNegativeInteger], [
		a owl:Restriction; owl:onProperty schola:commentaryHasLiteralExposition; owl:minCardinality "0"^^xsd:nonNegativeInteger], [ #* concerns whole expression
		a owl:Restriction; owl:onProperty schola:commentaryHasLiteralExpositionValue; owl:minCardinality "0"^^xsd:nonNegativeInteger].

schola:SentenceCommentary
	a owl:Class;
	rdfs:label "commentarius scholasticus"@la, "scholastic sentence commentary"@en, "scholastischer Satz-Kommentar"@de; #*
	rdfs:comment """Commentary with sentence structure, made by a scholastic."""@en;
	rdfs:subClassOf schola:Commentary, text:SentenceExpression, [
		a owl:Restriction; owl:onProperty schola:commentaryHasQuestion; owl:minCardinality "0"^^xsd:nonNegativeInteger], [
		a owl:Restriction; owl:onProperty schola:commentaryHasQuestionValue; owl:minCardinality "0"^^xsd:nonNegativeInteger], [
		a owl:Restriction; owl:onProperty schola:commentaryHasConclusion; owl:minCardinality "0"^^xsd:nonNegativeInteger], [
		a owl:Restriction; owl:onProperty schola:commentaryHasConclusionValue; owl:minCardinality "0"^^xsd:nonNegativeInteger], [
		a owl:Restriction; owl:onProperty schola:commentaryHasSyllogism; owl:minCardinality "0"^^xsd:nonNegativeInteger], [
		a owl:Restriction; owl:onProperty schola:commentaryHasSyllogismValue; owl:minCardinality "0"^^xsd:nonNegativeInteger].

# schola:CommentingProcedure #* RLP: stage?
#	a owl:Class;
#	rdfs:label "scholastic commenting procedure"@en, "scholastische Kommentierungvorgehensweise"@de;
#	rdfs:comment """Scholastic procedure to comment."""@en;
#	rdfs:subClassOf event:Procedure. # event:Stage

schola:Lectura # actually a result of a creating procedure of which the commentary is the subject
	a owl:Class;
	rdfs:label "lectura"@la;
	rdfs:comment """Scholastic commentary on a text expression, as presented by its author in a lecture."""@en;
	rdfs:subClassOf schola:Commentary.

schola:LecturaRevisa #* RLP: = Ordinatio? ; after Lectura
	a owl:Class;
	rdfs:label "lectura revisa"@la;
	rdfs:comment """Scholastic commentary on a text expression, as revised by its author after its presentation in a lecture."""@en;
	rdfs:subClassOf schola:Commentary.

schola:Reportatio #* after LecturaRevisa
	a owl:Class;
	rdfs:label "reportatio"@la, "reportatio"@en, "Reportatio"@de;
	rdfs:comment """Scholastic commentary on a text expression, as recorded by a *student* in a lecture."""@en; #* RLP: "listener", "auditor" instead of "student"?
	rdfs:subClassOf schola:Commentary, [
		a owl:Restriction; owl:onProperty schola:hasReportator; owl:minCardinality "0"^^xsd:nonNegativeInteger], [
		a owl:Restriction; owl:onProperty schola:hasReportatorValue; owl:minCardinality "0"^^xsd:nonNegativeInteger].

schola:ReportatioApprobata #* after Reportatio
	a owl:Class;
	rdfs:label "reportatio approbata"@la;
	rdfs:comment """Scholastic commentary on a text expression as student recordings approved by the master."""@en;
	rdfs:subClassOf schola:Commentary.

schola:Ordinatio #* after ReportatioApprobata
	a owl:Class;
	rdfs:label "ordinatio"@la;
	rdfs:comment """Scholastic commentary on a text expression as composed for publication."""@en;
	rdfs:subClassOf schola:Commentary.

#
# PROPERTIES
#

schola:hasRole
	a owl:ObjectProperty;
	rdfs:label "has role"@en, "hat Rolle"@de;
	rdfs:comment """Relating a scholastic to a role he has."""@en;
	rdfs:domain schola:Scholastic;
	rdfs:range schola:Role;
	rdfs:subPropertyOf human:hasRole;
	knora-base:subjectClassConstraint schola:Scholastic;
	knora-base:objectClassConstraint schola:Role.

schola:hasRoleValue
	a owl:ObjectProperty;
	rdfs:label "has role - statement"@en, "hat Rolle - Festlegung"@de;
	rdfs:comment """Relating a scholastic to a statement as reification of the relation between the scholastic and a role he has."""@en;
	rdfs:subPropertyOf human:hasRoleValue;
	knora-base:subjectClassConstraint schola:Scholastic;
	knora-base:objectClassConstraint knora-base:LinkValue.

# schola:hasReportatorRole
#	a owl:ObjectProperty;
#	rdfs:label "has reportator role"@en, "hat Reportator Rolle"@de;
#	rdfs:comment """Relating a scholastic to a reportator role he has."""@en;
#	rdfs:domain schola:Scholastic;
#	rdfs:range schola:Reportator;  
#	rdfs:subPropertyOf schola:hasRole;
#	knora-base:subjectClassConstraint schola:Scholastic;
#	knora-base:objectClassConstraint schola:Reportator.

# schola:hasReportatorRoleValue
#	a owl:ObjectProperty;
#	rdfs:label "has reportator role - statement"@en, "hat Reportator Rolle - Festlegung"@de;
#	rdfs:comment """Relating a scholastic to a statement as reification of the relation between the scholastic and a reportator role he has."""@en;
#	rdfs:subPropertyOf schola:hasRoleValue;
#	knora-base:subjectClassConstraint schola:Scholastic;
#	knora-base:objectClassConstraint knora-base:LinkValue.

 schola:hasReportator
	a owl:ObjectProperty;
	rdfs:label "has reportator"@en, "hat Reportator"@de;
	rdfs:comment """Relating a scholastic comment of a lecture to a scholastic who reported it."""@en;
	rdfs:domain schola:Reportatio;
#	rdfs:range [rdfs:subClassOf schola:Scholastic, [a owl:Restriction; owl:onProperty schola:hasRole; owl:someValuesFrom schola:Reportator];
	rdfs:subPropertyOf knora-base:hasLinkTo;
	knora-base:subjectClassConstraint schola:Reportatio;
	knora-base:objectClassConstraint schola:Scholastic.

schola:hasReportatorValue
	a owl:ObjectProperty;
	rdfs:label "has reportator - statement"@en, "hat Reportator - Festlegung"@de;
	rdfs:comment """Relating a scholastic lecture to a statement as reification of the relation between the lecture and a scholastic who reported it."""@en;
	rdfs:subPropertyOf knora-base:hasLinkToValue;
	knora-base:subjectClassConstraint schola:Reportatio;
	knora-base:objectClassConstraint knora-base:LinkValue.

schola:commentaryHasForm
	a owl:ObjectProperty;
	rdfs:label "commentary has form"@en, "Kommentar hat Form"@de;
	rdfs:comment """Relating a scholastic commentary to a form it has."""@en;
	rdfs:domain schola:Commentary;
	rdfs:range text:Text;
	rdfs:subPropertyOf knora-base:hasLinkTo;
	knora-base:subjectClassConstraint schola:Commentary;
	knora-base:objectClassConstraint text:Text.

schola:commentaryHasFormValue
	a owl:ObjectProperty;
	rdfs:label "commentary has form - statement"@en, "Kommentar hat Form - Festlegung"@de;
	rdfs:comment """Relating a scholastic commentary to a statement as reification of the relation between the commentary and a form it has."""@en;
	rdfs:subPropertyOf knora-base:hasLinkToValue;
	knora-base:subjectClassConstraint schola:Commentary;
	knora-base:objectClassConstraint knora-base:LinkValue.

schola:commentaryHasGloss
	a owl:ObjectProperty;
	rdfs:label "commentary has gloss"@en, "Kommentar hat Glosse"@de;
	rdfs:comment """Relating a scholastic commentary to a gloss it contains."""@en;
	rdfs:domain schola:Commentary;
	rdfs:range text-structure:Gloss;
	rdfs:subPropertyOf schola:commentaryHasForm, text-structure:hasGloss;
	knora-base:subjectClassConstraint schola:Commentary;
	knora-base:objectClassConstraint text-structure:Gloss.

schola:commentaryHasGlossValue
	a owl:ObjectProperty;
	rdfs:label "commentary has gloss - statement"@en, "Kommentar hat Glosse - Festlegung"@de;
	rdfs:comment """Relating a scholastic commentary to a statement as reification of the relation between the commentary and a gloss it contains."""@en;
	rdfs:subPropertyOf schola:commentaryHasFormValue, text-structure:hasGlossValue;
	knora-base:subjectClassConstraint schola:Commentary;
	knora-base:objectClassConstraint knora-base:LinkValue.

schola:commentaryHasQuestion
	a owl:ObjectProperty;
	rdfs:label "commentary has question"@en, "Kommentar hat Frage"@de;
	rdfs:comment """Relating a scholastic commentary to a question it contains."""@en;
	rdfs:domain schola:SentenceCommentary;
	rdfs:range ling:Question;
	rdfs:subPropertyOf schola:commentaryHasForm, text-structure:hasSentence;
	knora-base:subjectClassConstraint schola:SentenceCommentary;
	knora-base:objectClassConstraint ling:Question.

schola:commentaryHasQuestionValue
	a owl:ObjectProperty;
	rdfs:label "commentary has question - statement"@en, "Kommentar hat Frage - Festlegung"@de;
	rdfs:comment """Relating a scholastic commentary to a statement as reification of the relation between the commentary and a question it contains."""@en;
	rdfs:subPropertyOf schola:commentaryHasFormValue, text-structure:hasSentenceValue;
	knora-base:subjectClassConstraint schola:SentenceCommentary;
	knora-base:objectClassConstraint knora-base:LinkValue.

schola:commentaryHasConclusion
	a owl:ObjectProperty;
	rdfs:label "commentary has conclusion"@en, "Kommentar hat Konklusion"@de;
	rdfs:comment """Relating a scholastic commentary to a conclusion it contains."""@en;
	rdfs:domain schola:SentenceCommentary;
	rdfs:range logic:Conclusion;
	rdfs:subPropertyOf schola:commentaryHasForm, text-structure:hasSentence;
	knora-base:subjectClassConstraint schola:SentenceCommentary;
	knora-base:objectClassConstraint logic:Conclusion.

schola:commentaryHasConclusionValue
	a owl:ObjectProperty;
	rdfs:label "commentary has conclusion - statement"@en, "Kommentar hat Konklusion - Festlegung"@de;
	rdfs:comment """Relating a scholastic commentary to a statement as reification of the relation between the commentary and a conclusion it contains."""@en;
	rdfs:subPropertyOf schola:commentaryHasFormValue, text-structure:hasSentenceValue;
	knora-base:subjectClassConstraint schola:SentenceCommentary;
	knora-base:objectClassConstraint knora-base:LinkValue.

schola:commentaryHasSyllogism
	a owl:ObjectProperty;
	rdfs:label "commentary has syllogism"@en, "Kommentar hat Syllogismus"@de;
	rdfs:comment """Relating a scholastic commentary to a syllogism it contains."""@en;
	rdfs:domain schola:SentenceCommentary;
	rdfs:range logic:Syllogism;
	rdfs:subPropertyOf schola:commentaryHasForm, text-structure:hasParagraph;
	knora-base:subjectClassConstraint schola:SentenceCommentary;
	knora-base:objectClassConstraint logic:Syllogism.

schola:commentaryHasSyllogismValue
	a owl:ObjectProperty;
	rdfs:label "commentary has syllogism - statement"@en, "Kommentar hat Syllogismus - Festlegung"@de;
	rdfs:comment """Relating a scholastic commentary to a statement as reification of the relation between the commentary and a syllogism it contains."""@en;
	rdfs:subPropertyOf schola:commentaryHasFormValue, text-structure:hasParagraphValue;
	knora-base:subjectClassConstraint schola:SentenceCommentary;
	knora-base:objectClassConstraint knora-base:LinkValue.

schola:commentaryHasVerse
	a owl:ObjectProperty;
	rdfs:label "commentary has verse"@en, "Kommentar hat Vers"@de;
	rdfs:comment """Relating a scholastic commentary to a verse it contains."""@en;
	rdfs:domain schola:Commentary;
	rdfs:range text-structure:Verse;
	rdfs:subPropertyOf schola:commentaryHasForm, text-structure:hasStructure; #* :VerseExpression
	knora-base:subjectClassConstraint schola:Commentary;
	knora-base:objectClassConstraint text-structure:Verse.

schola:commentaryHasVerseValue
	a owl:ObjectProperty;
	rdfs:label "commentary has verse - statement"@en, "Kommentar hat Vers - Festlegung"@de;
	rdfs:comment """Relating a scholastic commentary to a statement as reification of the relation between the commentary and a verse it contains."""@en;
	rdfs:subPropertyOf schola:commentaryHasFormValue, text-structure:hasStructureValue;
	knora-base:subjectClassConstraint schola:Commentary;
	knora-base:objectClassConstraint knora-base:LinkValue.

schola:commentaryHasTable
	a owl:ObjectProperty;
	rdfs:label "commentary has table"@en, "Kommentar hat Tabelle"@de;
	rdfs:comment """Relating a scholastic commentary to a table it contains."""@en;
	rdfs:domain schola:Commentary;
	rdfs:range text-structure:Table;
	rdfs:subPropertyOf schola:commentaryHasForm, text-structure:hasStructure;
	knora-base:subjectClassConstraint schola:Commentary;
	knora-base:objectClassConstraint text-structure:Table.

schola:commentaryHasTableValue
	a owl:ObjectProperty;
	rdfs:label "commentary has table - statement"@en, "Kommentar hat Tabelle - Festlegung"@de;
	rdfs:comment """Relating a scholastic commentary to a statement as reification of the relation between the commentary and a table it contains."""@en;
	rdfs:subPropertyOf schola:commentaryHasFormValue, text-structure:hasStructureValue;
	knora-base:subjectClassConstraint schola:Commentary;
	knora-base:objectClassConstraint knora-base:LinkValue.

schola:commentaryHasAbbreviation
	a owl:ObjectProperty;
	rdfs:label "commentary has abbreviation"@en, "Kommentar hat Kurzfassung"@de;
	rdfs:comment """Relating a scholastic commentary to an abbreviation it contains."""@en;
	rdfs:domain schola:Commentary;
	rdfs:range textedit:Abbreviation;
	rdfs:subPropertyOf schola:commentaryHasForm;
	knora-base:subjectClassConstraint schola:Commentary;
	knora-base:objectClassConstraint textedit:Abbreviation.

schola:commentaryHasAbbreviationValue
	a owl:ObjectProperty;
	rdfs:label "commentary has abbreviation - statement"@en, "Kommentar hat Kurzfassung - Festlegung"@de;
	rdfs:comment """Relating a scholastic commentary to a statement as reification of the relation between the commentary and an abbreviation it contains."""@en;
	rdfs:subPropertyOf schola:commentaryHasFormValue;
	knora-base:subjectClassConstraint schola:Commentary;
	knora-base:objectClassConstraint knora-base:LinkValue.

schola:commentaryHasParaphrase
	a owl:ObjectProperty;
	rdfs:label "commentary has paraphrase"@en, "Kommentar hat Paraphrase"@de;
	rdfs:comment """Relating a scholastic commentary to a paraphrase it contains."""@en;
	rdfs:domain schola:Commentary;
	rdfs:range textedit:Paraphrase;
	rdfs:subPropertyOf schola:commentaryHasForm;
	knora-base:subjectClassConstraint schola:Commentary;
	knora-base:objectClassConstraint textedit:Paraphrase.

schola:commentaryHasParaphraseValue
	a owl:ObjectProperty;
	rdfs:label "commentary has paraphrase - statement"@en, "Kommentar hat Paraphrase - Festlegung"@de;
	rdfs:comment """Relating a scholastic commentary to a statement as reification of the relation between the commentary and a paraphrase it contains."""@en;
	rdfs:subPropertyOf schola:commentaryHasFormValue;
	knora-base:subjectClassConstraint schola:Commentary;
	knora-base:objectClassConstraint knora-base:LinkValue.

schola:commentaryHasLiteralExposition
	a owl:ObjectProperty;
	rdfs:label "commentary has literal exposition"@en, "Kommentar hat wörtliche Auslegung"@de;
	rdfs:comment """Relating a scholastic commentary to a literal exposition it contains."""@en;
	rdfs:domain schola:Commentary;
	rdfs:range textedit:LiteralExposition;
	rdfs:subPropertyOf schola:commentaryHasForm;
	knora-base:subjectClassConstraint schola:Commentary;
	knora-base:objectClassConstraint textedit:LiteralExposition.

schola:commentaryHasLiteralExpositionValue
	a owl:ObjectProperty;
	rdfs:label "commentary has literal exposition - statement"@en, "Kommentar hat wörtliche Auslegung - Festlegung"@de;
	rdfs:comment """Relating a scholastic commentary to a statement as reification of the relation between the commentary and a literal exposition it contains."""@en;
	rdfs:subPropertyOf schola:commentaryHasFormValue;
	knora-base:subjectClassConstraint schola:Commentary;
	knora-base:objectClassConstraint knora-base:LinkValue.