@prefix rdfs: <http://www.w3.org/2000/01/rdf-schema#>.
@prefix owl: <http://www.w3.org/2002/07/owl#>.
@prefix xsd: <http://www.w3.org/2001/XMLSchema#>.
@prefix skos: <http://www.w3.org/2004/02/skos/core#>.
@prefix dct: <http://purl.org/dc/terms/>.
@prefix foaf: <http://xmlns.com/foaf/0.1/>.
@prefix cidoc: <http://www.cidoc-crm.org/cidoc-crm/>.
@prefix frbroo: <http://iflastandards.info/ns/fr/frbr/frbroo/>.
@prefix event: <http://www.knora.org/ontology/0047/event#>.
@prefix human: <http://www.knora.org/ontology/0048/human#>.
@prefix org: <http://www.knora.org/ontology/0051/organization#>.
@prefix language: <http://www.knora.org/ontology/004F/language#>.
@prefix concept: <http://www.knora.org/ontology/0044/concept#>.
@prefix math: <http://www.knora.org/ontology/0061/mathematics#>.
@prefix document: <http://www.knora.org/ontology/005C/document#>.
@prefix text-structure: <http://www.knora.org/ontology/005B/text-structure#>.
@prefix textedit: <http://www.knora.org/ontology/005A/text-editing#>.
@prefix infocar: <http://www.knora.org/ontology/004C/information-carrier#>.
@prefix publish: <http://www.knora.org/ontology/0056/publishing#>.
@prefix litera: <http://www.knora.org/ontology/0050/literature#>.
@prefix knora-base: <http://www.knora.org/ontology/knora-base#>.

@base <http://www.knora.org/ontology/0059/text>.
@prefix text: <http://www.knora.org/ontology/0059/text#>.

<http://www.knora.org/ontology/0059/text>
	a owl:Ontology;
	dct:title "An ontology about text"@en;
	dct:description """Formal description of text in broadest sense, general subclasses, related classes, and properties."""@en;
	skos:note """Text editing is described in a seperate ontology"""@en;
	dct:creator "Hans Cools, MD, knowledge engineer, ontologist, software developer, NIE-INE, Basel University, Switzerland"@en;
	dct:contributor "Roberta Padlina, tool coordinator, software developer, NIE-INE, Basel University, Switzerland"@en;
	dct:publisher "Basel University, Switzerland"@en;
#	skos:note """Representation of an otherwise literal data element as object enabling relating it to other data"""@en.

	knora-base:attachedToProject <http://rdfh.ch/projects/0059>.

#
# CLASSES
#

text:Text
	a owl:Class;
	rdfs:label "text"@en, "Text"@de, "texte"@fr, "testo"@it;
	rdfs:comment """Human natural language expression serialized in writable form."""@en; # what can be learned by heart
	rdfs:subClassOf language:HumanNaturalLanguageExpression, [
		a owl:Restriction; owl:onProperty text:hasLineNumber; owl:minCardinality "0"^^xsd:nonNegativeInteger], [
		a owl:Restriction; owl:onProperty text:hasVersionIndicator; owl:minCardinality "0"^^xsd:nonNegativeInteger], [
		a owl:Restriction; owl:onProperty text:hasPageNumberDescription; owl:minCardinality "0"^^xsd:nonNegativeInteger], [
		a owl:Restriction; owl:onProperty text:hasReferenceText; owl:minCardinality "0"^^xsd:nonNegativeInteger], [
		a owl:Restriction; owl:onProperty text:hasReferenceTextValue; owl:minCardinality "0"^^xsd:nonNegativeInteger], [
		a owl:Restriction; owl:onProperty text:hasRevisor; owl:minCardinality "0"^^xsd:nonNegativeInteger], [
		a owl:Restriction; owl:onProperty text:hasRevisorValue; owl:minCardinality "0"^^xsd:nonNegativeInteger], [
		a owl:Restriction; owl:onProperty text:hasTranscriber; owl:minCardinality "0"^^xsd:nonNegativeInteger], [
		a owl:Restriction; owl:onProperty text:hasTranscriberValue; owl:minCardinality "0"^^xsd:nonNegativeInteger], [
		a owl:Restriction; owl:onProperty text:hasCiter; owl:minCardinality "0"^^xsd:nonNegativeInteger], [
		a owl:Restriction; owl:onProperty text:hasCiterValue; owl:minCardinality "0"^^xsd:nonNegativeInteger], [
		a owl:Restriction; owl:onProperty text:hasCitation; owl:minCardinality "0"^^xsd:nonNegativeInteger], [
		a owl:Restriction; owl:onProperty text:hasCitationValue; owl:minCardinality "0"^^xsd:nonNegativeInteger], [
		a owl:Restriction; owl:onProperty text:hasCitationReferenceIdentifier; owl:minCardinality "0"^^xsd:nonNegativeInteger], [
		a owl:Restriction; owl:onProperty text:hasCitationReferenceIdentifierValue; owl:minCardinality "0"^^xsd:nonNegativeInteger], [
		a owl:Restriction; owl:onProperty text:hasCitationReferenceNumber; owl:minCardinality "0"^^xsd:nonNegativeInteger], [
		a owl:Restriction; owl:onProperty text:hasCitationReferenceNumberValue; owl:minCardinality "0"^^xsd:nonNegativeInteger], [
		a owl:Restriction; owl:onProperty text:isCitedIn; owl:minCardinality "0"^^xsd:nonNegativeInteger], [
		a owl:Restriction; owl:onProperty text:isCitedInValue; owl:minCardinality "0"^^xsd:nonNegativeInteger], [
		a owl:Restriction; owl:onProperty text:hasEditor; owl:minCardinality "0"^^xsd:nonNegativeInteger], [
		a owl:Restriction; owl:onProperty text:hasEditorValue; owl:minCardinality "0"^^xsd:nonNegativeInteger], [
		a owl:Restriction; owl:onProperty textedit:hasEdition; owl:minCardinality "0"^^xsd:nonNegativeInteger], [
		a owl:Restriction; owl:onProperty textedit:hasEditionValue; owl:minCardinality "0"^^xsd:nonNegativeInteger], [
		a owl:Restriction; owl:onProperty textedit:hasTransliteration; owl:minCardinality "0"^^xsd:nonNegativeInteger], [
		a owl:Restriction; owl:onProperty textedit:hasTransliterationValue; owl:minCardinality "0"^^xsd:nonNegativeInteger], [
		a owl:Restriction; owl:onProperty textedit:hasGlossator; owl:minCardinality "0"^^xsd:nonNegativeInteger], [
		a owl:Restriction; owl:onProperty textedit:hasGlossatorValue; owl:minCardinality "0"^^xsd:nonNegativeInteger], [
		a owl:Restriction; owl:onProperty textedit:hasAbbreviator; owl:minCardinality "0"^^xsd:nonNegativeInteger], [
		a owl:Restriction; owl:onProperty textedit:hasAbbreviatorValue; owl:minCardinality "0"^^xsd:nonNegativeInteger], [
		a owl:Restriction; owl:onProperty textedit:hasRedactor; owl:minCardinality "0"^^xsd:nonNegativeInteger], [
		a owl:Restriction; owl:onProperty textedit:hasRedactorValue; owl:minCardinality "0"^^xsd:nonNegativeInteger], [
		a owl:Restriction; owl:onProperty textedit:hasSameEditionAs; owl:minCardinality "0"^^xsd:nonNegativeInteger], [
		a owl:Restriction; owl:onProperty textedit:hasSameEditionAsValue; owl:minCardinality "0"^^xsd:nonNegativeInteger], [
		a owl:Restriction; owl:onProperty infocar:isTextOnPage; owl:minCardinality "0"^^xsd:nonNegativeInteger], [
		a owl:Restriction; owl:onProperty infocar:isTextOnPageValue; owl:minCardinality "0"^^xsd:nonNegativeInteger].

text:WrittenText
	a owl:Class;
	rdfs:label "written text"@en, "geschriebener Text"@de, "texte écrit"@fr, "testo scritto"@it;
	rdfs:comment """Text written by any method, e.g. manually, with an analogue or digital typewriter, or on a computer, abstracted from its carrier."""@en;
	rdfs:subClassOf text:Text, [
		a owl:Restriction; owl:onProperty infocar:isWrittenWith; owl:minCardinality "0"^^xsd:nonNegativeInteger], [
		a owl:Restriction; owl:onProperty infocar:isWrittenWithValue; owl:minCardinality "0"^^xsd:nonNegativeInteger].

text:HandwrittenText
	a owl:Class;
	rdfs:label "handwritten text"@en, "handgeschriebener Text"@de, "texte manuscrit"@fr, "testo scritto a mano"@it;
	rdfs:comment """Text written by hand."""@en;
	rdfs:subClassOf text:WrittenText, [
		a owl:Restriction; owl:onProperty infocar:isInManuscript; owl:minCardinality "0"^^xsd:nonNegativeInteger], [
		a owl:Restriction; owl:onProperty infocar:isInManuscriptValue; owl:minCardinality "0"^^xsd:nonNegativeInteger].

text:TypewrittenText
	a owl:Class;
	rdfs:label "typewritten text"@en, "maschinengeschriebener Text"@de, "texte dactylographié"@fr, "testo dattiloscritto"@it;
	rdfs:comment """Text written with a typewriter."""@en;
	rdfs:subClassOf text:WrittenText, [
		a owl:Restriction; owl:onProperty infocar:isInTypescript; owl:minCardinality "0"^^xsd:nonNegativeInteger], [
		a owl:Restriction; owl:onProperty infocar:isInTypescriptValue; owl:minCardinality "0"^^xsd:nonNegativeInteger]. #, [
#		a owl:Restriction; owl:onProperty infocar:isWrittenWith; owl:allValuesFrom text:Typewriter].

text:TranscribedText
	a owl:Class;
	rdfs:label "transcribed text"@en, "transkribierter Text"@de, "texte transcrit"@fr, "testo trascritto"@it;
	rdfs:comment """Text copied by character by any method."""@en;
	rdfs:subClassOf text:WrittenText, [
		a owl:Restriction; owl:onProperty infocar:isInTranscript; owl:minCardinality "0"^^xsd:nonNegativeInteger], [
		a owl:Restriction; owl:onProperty infocar:isInTranscriptValue; owl:minCardinality "0"^^xsd:nonNegativeInteger].

# text:Print: printed text abstracted from its carrier

text:Expression
	a owl:Class;
	rdfs:label "text expression"@en, "Text-Expression"@de, "expression textuelle"@fr, "espressione testuale"@it;
	rdfs:comment """Text as expression conform FRBROO."""@en;
	rdfs:subClassOf document:Expression, text:Text, [
		a owl:Restriction; owl:onProperty text:hasAuthor; owl:minCardinality "0"^^xsd:nonNegativeInteger], [
		a owl:Restriction; owl:onProperty text:hasAuthorValue; owl:minCardinality "0"^^xsd:nonNegativeInteger], [
		a owl:Restriction; owl:onProperty text:hasScientificEditor; owl:minCardinality "0"^^xsd:nonNegativeInteger], [
		a owl:Restriction; owl:onProperty text:hasScientificEditorValue; owl:minCardinality "0"^^xsd:nonNegativeInteger], [
		a owl:Restriction; owl:onProperty text:hasCriticalEditor; owl:minCardinality "0"^^xsd:nonNegativeInteger], [
		a owl:Restriction; owl:onProperty text:hasCriticalEditorValue; owl:minCardinality "0"^^xsd:nonNegativeInteger], [
		a owl:Restriction; owl:onProperty textedit:hasDerivedTextExpression; owl:minCardinality "0"^^xsd:nonNegativeInteger], [
		a owl:Restriction; owl:onProperty textedit:hasDerivedTextExpressionValue; owl:minCardinality "0"^^xsd:nonNegativeInteger], [
		a owl:Restriction; owl:onProperty textedit:hasScientificEdition; owl:minCardinality "0"^^xsd:nonNegativeInteger], [
		a owl:Restriction; owl:onProperty textedit:hasScientificEditionValue; owl:minCardinality "0"^^xsd:nonNegativeInteger], [
		a owl:Restriction; owl:onProperty textedit:hasDiplomaticTranscription; owl:minCardinality "0"^^xsd:nonNegativeInteger], [
		a owl:Restriction; owl:onProperty textedit:hasDiplomaticTranscriptionValue; owl:minCardinality "0"^^xsd:nonNegativeInteger], [
		a owl:Restriction; owl:onProperty textedit:hasCriticalEdition; owl:minCardinality "0"^^xsd:nonNegativeInteger], [
		a owl:Restriction; owl:onProperty textedit:hasCriticalEditionValue; owl:minCardinality "0"^^xsd:nonNegativeInteger].

text:IndividualExpression
	a owl:Class;
	rdfs:label "individual text expression"@en, "individuelle Text-Expression"@de;
	rdfs:comment """Text as individual expression."""@en;
	rdfs:subClassOf text:Expression, document:IndividualExpression, [
		a owl:Restriction; owl:onProperty text:hasIncipit; owl:minCardinality "0"^^xsd:nonNegativeInteger], [
		a owl:Restriction; owl:onProperty text:hasExplicit; owl:minCardinality "0"^^xsd:nonNegativeInteger].

text:ExpressionPart
	a owl:Class;
	rdfs:label "text expression part"@en, "Text-Expressionsteil"@de;
	rdfs:comment """Part of an individual text expression, considered as incomplete."""@en;
	rdfs:subClassOf text:Expression, document:ExpressionPart, [
		a owl:Restriction; owl:onProperty text:isPartOfIndividualExpression; owl:minCardinality "0"^^xsd:nonNegativeInteger], [
		a owl:Restriction; owl:onProperty text:isPartOfIndividualExpressionValue; owl:minCardinality "0"^^xsd:nonNegativeInteger].

text:Author
	a owl:Class;
	rdfs:label "text author"@en, "Textautor"@de, "auteur du texte"@fr, "autore di testo"@it;
	rdfs:comment """Role of a person being responsible for a text expression."""@en;
	skos:note """Often an author is also the creator of a text expression."""@en;
	rdfs:subClassOf human:Author.

text:ManOfLetters
	a owl:Class;
	rdfs:label "man of letters"@en, "Literat"@de, "homme de lettres"@fr, "uomo di lettere"@it;
	rdfs:comment """Role of a man devoted to literary activity."""@en;
	rdfs:subClassOf human:PersonRole.

text:WomanOfLetters
	a owl:Class;
	rdfs:label "woman of letters"@en, "Literatin"@de, "femme de lettres"@fr, "donna di lettere"@it;
	rdfs:comment """Role of a woman devoted to literary activity."""@en;
	rdfs:subClassOf human:PersonRole.

text:Revisor
	a owl:Class;
	rdfs:label "revisor"@en, "Revisor"@de, "réviseur"@fr, "revisore"@it;
	rdfs:comment """Role of a person checking on certain aspects of a text."""@en;
	rdfs:subClassOf human:PersonRole.

text:Translator
	a owl:Class;
	rdfs:label "translator"@en, "ÜbersetzerIn"@de, "traduct-eur/rice"@fr, "tradutt-ore/rice"@it;
	rdfs:comment """Role of a person translating text by writing or printing."""@en;
	rdfs:subClassOf language:PersonTranslator.

text:Copyist # -> text:Transcriber
	a owl:Class;
	rdfs:label "copyist"@en, "Kopist"@de, "copiste"@fr, "copista"@it, "scribes"@la; # "scribe"@en, "Schreiber"@de;
	rdfs:comment """Role of a person copying text by writing."""@en;
	rdfs:subClassOf human:PersonCreator.

text:AgentCiter
	a owl:Class;
	rdfs:label "agent citer"@en, "Agent-Zitierer"@de;
	rdfs:comment """Role of a human agent, person or group, citing a text."""@en;
	rdfs:subClassOf human:AgentRole.

text:PersonCiter
	a owl:Class;
	rdfs:label "person citer"@en, "Person-ZitiererIn"@de;
	rdfs:comment """Citer as role of a person."""@en;
	rdfs:subClassOf text:AgentCiter, human:PersonRole.

text:OrganizationCiter
	a owl:Class;
	rdfs:label "organization citer"@en, "Organisation-Zitiererin"@de;
	rdfs:comment """Citer as role of an organization."""@en;
	rdfs:subClassOf text:AgentCiter, org:Role.

text:Citation
	a owl:Class;
	rdfs:label "citation"@en, "Zitat"@de, "citation"@fr, "citazione"@it;
	rdfs:comment """."""@en;
	rdfs:subClassOf text:Text, [
		a owl:Restriction; owl:onProperty text:citationHasIdentifier; owl:minCardinality "0"^^xsd:nonNegativeInteger], [
		a owl:Restriction; owl:onProperty text:citationHasIdentifierValue; owl:minCardinality "0"^^xsd:nonNegativeInteger], [
		a owl:Restriction; owl:onProperty text:citationHasNumber; owl:minCardinality "0"^^xsd:nonNegativeInteger], [
		a owl:Restriction; owl:onProperty text:citationHasNumberValue; owl:minCardinality "0"^^xsd:nonNegativeInteger], [
		a owl:Restriction; owl:onProperty text:citationIsPartOf; owl:minCardinality "0"^^xsd:nonNegativeInteger], [
		a owl:Restriction; owl:onProperty text:citationIsPartOfValue; owl:minCardinality "0"^^xsd:nonNegativeInteger].

text:CitationIdentifier
	a owl:Class;
	rdfs:label "citation identifier"@en, "Zitatidentifikator"@de;
	rdfs:comment """Identifier of a citation."""@en;
	rdfs:subClassOf concept:Identifier, document:Structure.

text:CitationNumber
	a owl:Class;
	rdfs:label "citation number"@en, "Zitatnummer"@de;
	rdfs:comment """Number of a citation."""@en;
	rdfs:subClassOf text:CitationIdentifier, math:Number.

text:CitationReferenceIdentifier
	a owl:Class;
	rdfs:label "citation reference identifier"@en, "Zitatreferenzidentifikator"@de;
	rdfs:comment """Identifier of a citation reference."""@en;
	rdfs:subClassOf concept:Identifier, document:Reference, [
		a owl:Restriction; owl:onProperty text:hasCitationIdentifier; owl:minCardinality "0"^^xsd:nonNegativeInteger], [
		a owl:Restriction; owl:onProperty text:hasCitationIdentifierValue; owl:minCardinality "0"^^xsd:nonNegativeInteger].

text:CitationReferenceNumber
	a owl:Class;
	rdfs:label "citation reference number"@en, "Zitatreferenznummer"@de;
	rdfs:comment """Number of a citation reference."""@en;
	rdfs:subClassOf text:CitationReferenceIdentifier, [
		a owl:Restriction; owl:onProperty text:hasCitationNumber; owl:minCardinality "0"^^xsd:nonNegativeInteger], [
		a owl:Restriction; owl:onProperty text:hasCitationNumberValue; owl:minCardinality "0"^^xsd:nonNegativeInteger].

text:SentenceExpression
	a owl:Class;
	rdfs:label "sentence expression"@en, "Satz-Expression"@de, "expression de phrases"@fr, "espressione di frase"@it;
	rdfs:comment """Text expression with sentence structure."""@en;
	rdfs:subClassOf text:Expression.

text:DiaryEntry
	a owl:Class;
	rdfs:label "diary entry"@en, "Tagebucheintrag"@de, "entrée du journal"@fr, "iscrizione del diario"@it;
	rdfs:comment """Periodical, usually daily description of a personal experience or observation written in a diary."""@en;
	rdfs:subClassOf text:IndividualExpression, [
		a owl:Restriction; owl:onProperty text:isEntryOfDiaryExpression; owl:minCardinality "0"^^xsd:nonNegativeInteger], [
		a owl:Restriction; owl:onProperty text:isEntryOfDiaryExpressionValue; owl:minCardinality "0"^^xsd:nonNegativeInteger], [
		a owl:Restriction; owl:onProperty infocar:entryIsInDiary; owl:minCardinality "0"^^xsd:nonNegativeInteger], [
		a owl:Restriction; owl:onProperty infocar:entryIsInDiaryValue; owl:minCardinality "0"^^xsd:nonNegativeInteger], [
		a owl:Restriction; owl:onProperty infocar:hasDiaryEnteringDate; owl:minCardinality "0"^^xsd:nonNegativeInteger].

text:DiaryExpression
	a owl:Class;
	rdfs:label "diary expression"@en, "Tagebuch-Expression"@de, "expression d'un journal"@fr, "expression del diario"@it;
	rdfs:comment """Text expression with a diary content and possibly structure."""@en;
	rdfs:subClassOf text:IndividualExpression, [
		a owl:Restriction; owl:onProperty infocar:isInDiary; owl:minCardinality "0"^^xsd:nonNegativeInteger], [
		a owl:Restriction; owl:onProperty infocar:isInDiaryValue; owl:minCardinality "0"^^xsd:nonNegativeInteger].

text:LetterExpression
	a owl:Class;
	rdfs:label "letter expression"@en, "Brief-Expression"@de;
	rdfs:comment """Text expression with a letter content and possibly structure."""@en;
	rdfs:subClassOf text:IndividualExpression, [
		a owl:Restriction; owl:onProperty infocar:isInLetter; owl:minCardinality "0"^^xsd:nonNegativeInteger], [
		a owl:Restriction; owl:onProperty infocar:isInLetterValue; owl:minCardinality "0"^^xsd:nonNegativeInteger].

text:Commentary
	a owl:Class;
	rdfs:label "commentary"@en, "Kommentar"@de;
	rdfs:comment """Text expression in the form of a series of comments as analysis, interpretation or explanation of something, especially another textual expression."""@en;
	rdfs:subClassOf text:IndividualExpression.

text:Draft
	a owl:Class;
	rdfs:label "draft"@en, "Entwurf"@de;
	rdfs:comment """Developmental text expression."""@en;
	rdfs:subClassOf human:CreationVersion.

text:Development
	a owl:Class;
	rdfs:label "text development"@en, "Text-Entwicklung"@de;
	rdfs:comment """Action wherein a person(s) creates text resulting in different manifestation, e.g. from notebook to manuscript to typescript to published print."""@en;
	rdfs:subClassOf human:Creating, [
		a owl:Restriction; owl:onProperty event:hasStage; owl:minCardinality "0"^^xsd:nonNegativeInteger], [
		a owl:Restriction; owl:onProperty event:hasStageValue; owl:minCardinality "0"^^xsd:nonNegativeInteger].

#* extrinsic feature: carrier, typescript, system of signs, diacritical eg. &
#* intrinsic: formal content

#*text:Witness
#	a owl:Class;
#	rdfs:label "witness"@en, "Textzeuge"@de;
#	rdfs:comment """Copy of an original text ."""@en; #* note: enabling its reconstruction, -> looking for features of originality
#	rdfs:subClassOf text:Transcription.

text:Biography
	a owl:Class;
	rdfs:label "biography"@en, "Biographie"@de; #*
	rdfs:comment """Text expression about a person's life."""@en;
	rdfs:subClassOf text:IndividualExpression.

#
# PROPERTIES
#

text:hasText
	a owl:ObjectProperty;
	rdfs:label "has text"@en, "hat Text"@de;
	rdfs:comment """Relating a resource to a text as a writable coherent set of signs representing semantics in a language."""@en;
	rdfs:domain rdfs:Resource;
	rdfs:range rdfs:Literal;
	rdfs:subPropertyOf knora-base:hasValue;
	knora-base:subjectClassConstraint knora-base:Resource;
	knora-base:objectClassConstraint knora-base:TextValue.

text:hasName
	a owl:ObjectProperty;
	rdfs:label "has name"@en, "hat Name"@de;
	rdfs:comment """Relating a resource to a name as a textual identifier of the resource."""@en;
	rdfs:subPropertyOf text:hasText; # rdfs:label, foaf:name
	knora-base:subjectClassConstraint knora-base:Resource;
	knora-base:objectClassConstraint knora-base:TextValue.

text:hasPreferredName
	a owl:ObjectProperty;
	rdfs:label "has preferred name"@en, "hat bevorzugter Name"@de;
	rdfs:comment """Relating a resource to a preferred name."""@en;
	rdfs:subPropertyOf text:hasName;
	knora-base:subjectClassConstraint knora-base:Resource;
	knora-base:objectClassConstraint knora-base:TextValue.

text:hasAlias
	a owl:ObjectProperty;
	rdfs:label "has alias"@en, "hat Alias"@de;
	rdfs:comment """Relating a resource to an alias as an alternative name of the resource."""@en;
	rdfs:subPropertyOf text:hasName;
	knora-base:subjectClassConstraint knora-base:Resource;
	knora-base:objectClassConstraint knora-base:TextValue.

# text:hasSynonym
#	a owl:ObjectProperty;
#	rdfs:label "has synonym"@en, "hat Synonym"@de;
#	rdfs:comment """Relating a class to a synonym of the name of the class."""@en;
#	rdfs:domain rdfs:Resource;
#	rdfs:range rdfs:Literal;
#	rdfs:subPropertyOf text:hasName;
#	knora-base:subjectClassConstraint knora-base:Resource;
#	knora-base:objectClassConstraint knora-base:TextValue.

text:hasIdentifier
	a owl:ObjectProperty;
	rdfs:label "has identifier"@en, "hat Kennzeichen"@de;
	rdfs:comment """Relating a resource to an identifier as a unique and permanent textual reference to the resource within a given context, and conforming to a formal identification system."""@en;
	rdfs:subPropertyOf text:hasText; #* cf. dcterms:identifier
	knora-base:subjectClassConstraint knora-base:Resource;
	knora-base:objectClassConstraint knora-base:TextValue.

text:hasTitle
	a owl:ObjectProperty;
	rdfs:label "has title"@en, "hat Titel"@de;
	rdfs:comment """Relating a resource to a title as a textual identifier of the resource."""@en;
	rdfs:subPropertyOf text:hasText;
	knora-base:subjectClassConstraint knora-base:Resource;
	knora-base:objectClassConstraint knora-base:TextValue.

text:hasComment
	a owl:ObjectProperty;
	rdfs:label "has comment"@en, "hat Kommentar"@de;
	rdfs:comment """Relating a resource to a comment as a textual statement about the resource."""@en;
	rdfs:subPropertyOf text:hasText;
	knora-base:subjectClassConstraint knora-base:Resource;
	knora-base:objectClassConstraint knora-base:TextValue.

text:hasDescription
	a owl:ObjectProperty;
	rdfs:label "has description"@en, "hat Beschreibung"@de;
	rdfs:comment """Relating a resource to a description as a textual statement about features of the resource."""@en;
	rdfs:subPropertyOf text:hasText;
	knora-base:subjectClassConstraint knora-base:Resource;
	knora-base:objectClassConstraint knora-base:TextValue.

text:hasDefinition
	a owl:ObjectProperty;
	rdfs:label "has definition"@en, "hat Definition"@de;
	rdfs:comment """Relating a resource to a definition as a textual statement about the essential features of the resource."""@en;
	rdfs:subPropertyOf text:hasDescription;
	knora-base:subjectClassConstraint knora-base:Resource;
	knora-base:objectClassConstraint knora-base:TextValue.

text:hasDetailDescription
	a owl:ObjectProperty;
	rdfs:label "has detail description"@en, "hat Detail-Beschreibung"@de;
	rdfs:comment """Relating a resource to a description of its detail. E.g. in the case of a text a detail can be a passage variant or an emendation"""@en;
	rdfs:subPropertyOf text:hasDescription;
	knora-base:subjectClassConstraint knora-base:Resource;
	knora-base:objectClassConstraint knora-base:TextValue.

text:hasSpecialDescription
	a owl:ObjectProperty;
	rdfs:label "has special description"@en, "hat Besonderes-Beschreibung"@de;
	rdfs:comment """Relating a resource to a description of (a) certain feature(s)."""@en;
	rdfs:subPropertyOf text:hasDescription;
	knora-base:subjectClassConstraint knora-base:Resource;
	knora-base:objectClassConstraint knora-base:TextValue.

text:hasLineNumber
	a owl:ObjectProperty;
	rdfs:label "has line number"@en, "hat Liniennummer"@de;
	rdfs:comment """Relating a text to the number of a line of the text expression."""@en;
	rdfs:domain text:Text;
	rdfs:range rdfs:Literal;	
	rdfs:subPropertyOf text:hasText;
	knora-base:subjectClassConstraint text:Text;
	knora-base:objectClassConstraint knora-base:TextValue.

text:hasVersionIndicator
	a owl:ObjectProperty;
	rdfs:label "has version indicator"@en, "hat Version-Indikator"@de;
	rdfs:comment """Relating a text to a textual element that indicates its version."""@en;
	rdfs:domain text:Text;
	rdfs:range rdfs:Literal;
	rdfs:subPropertyOf text:hasText;
	knora-base:subjectClassConstraint text:Text;
	knora-base:objectClassConstraint knora-base:TextValue.

#text:hasPageNumber
#	a owl:ObjectProperty;
#	rdfs:label "has page number"@en;
#	rdfs:comment """Relating a text to the number of a page it is on."""@en;
#	rdfs:subPropertyOf knora-base:hasValue;
#	knora-base:subjectClassConstraint text:Text; # owl:propertyChainAxiom (infocar:isTextOnPage infocar:pageHasNumber)
#	knora-base:objectClassConstraint knora-base:IntValue.

text:hasPageNumberDescription
	a owl:ObjectProperty;
	rdfs:label "text has page number description"@en, "Text hat Seitennummerbeschreibung"@de;
	rdfs:comment """Relating a text to a description of the number(s) of and possibly a location on (a) pages it is on; examples of the string of its value: "001-002", "01 recto", "O2 (bottom)"."""@en;
	rdfs:domain text:Text;
	rdfs:range rdfs:Literal;
	rdfs:subPropertyOf knora-base:hasValue;
	knora-base:subjectClassConstraint text:Text;
	knora-base:objectClassConstraint knora-base:TextValue.

text:hasReferenceText
	a owl:ObjectProperty;
	rdfs:label "has reference text"@en, "hat Bezugstext"@de;
	rdfs:comment "Relating a text to another one as its reference."@en;
	rdfs:subPropertyOf knora-base:hasLinkTo;
	knora-base:subjectClassConstraint text:Text;
	knora-base:objectClassConstraint text:Text.

text:hasReferenceTextValue
	a owl:ObjectProperty;
	rdfs:label "has reference text - statement"@en, "hat Bezugstext - Festlegung"@de;
	rdfs:comment "Relating a text to a reification statement of the relation between the text and another one as its reference."@en;
	rdfs:subPropertyOf knora-base:hasLinkToValue;
	knora-base:subjectClassConstraint text:Text;
	knora-base:objectClassConstraint knora-base:LinkValue.

text:hasRevisor
	a owl:ObjectProperty;
	rdfs:label "has revisor"@en, "hat Revisor"@de;
	rdfs:comment """Relating a text to a person who revised it."""@en;
	rdfs:domain text:Text;
#	rdfs:range [rdfs:subClassOf human:Person, [a owl:Restriction; owl:onProperty human:personHasRole; owl:someValuesFrom text:Revisor]];
	rdfs:subPropertyOf knora-base:hasLinkTo;
	knora-base:subjectClassConstraint text:Text;
	knora-base:objectClassConstraint human:Person.

text:hasRevisorValue
	a owl:ObjectProperty;
	rdfs:label "has revisor - statement"@en, "hat Revisor - Festlegung"@de;
	rdfs:comment """Relating a text to a reification statement of the relation between the text and a person who revised it."""@en;
	rdfs:subPropertyOf knora-base:hasLinkToValue;
	knora-base:subjectClassConstraint text:Text;
	knora-base:objectClassConstraint knora-base:LinkValue.

text:hasTranscriber
	a owl:ObjectProperty;
	rdfs:label "has transcriber"@en, "hat TranskribiererIn"@de;
	rdfs:comment """Relating a text to a person who transcribed it."""@en;
	rdfs:domain text:Text;
#	rdfs:range [rdfs:subClassOf human:Person, [a owl:Restriction; owl:onProperty human:personHasRole; owl:someValuesFrom text:Transcriber]];
	rdfs:subPropertyOf knora-base:hasLinkTo;
	knora-base:subjectClassConstraint text:Text;
	knora-base:objectClassConstraint human:Person.

text:hasTranscriberValue
	a owl:ObjectProperty;
	rdfs:label "has transcriber - statement"@en, "hat TranskribiererIn - Festlegung"@de;
	rdfs:comment """Relating a text to a reification statement of the relation between the text and a person who transcribed it."""@en;
	rdfs:subPropertyOf knora-base:hasLinkToValue;
	knora-base:subjectClassConstraint text:Text;
	knora-base:objectClassConstraint knora-base:LinkValue.

text:hasCiter
	a owl:ObjectProperty;
	rdfs:label "has citer"@en, "hat ZitiererIn"@de;
	rdfs:comment """Relating a text to a human agent - person or group - citing it."""@en;
	rdfs:domain text:Text;
#	rdfs:range [rdfs:subClassOf human:Agent, [a owl:Restriction; owl:onProperty human:agentHasRole; owl:someValuesFrom text:AgentCiter]];
	rdfs:subPropertyOf knora-base:hasLinkTo;
	knora-base:subjectClassConstraint text:Text;
	knora-base:objectClassConstraint human:Agent.

text:hasCiterValue
	a owl:ObjectProperty;
	rdfs:label "has citer - statement"@en, "hat ZitiererIn - Festlegung"@de;
	rdfs:comment """Relating a text to a reification statement of the relation between the text and a human agent - person or group - citing it."""@en;
	rdfs:subPropertyOf knora-base:hasLinkToValue;
	knora-base:subjectClassConstraint text:Text;
	knora-base:objectClassConstraint knora-base:LinkValue.

text:hasCitation
	a owl:ObjectProperty;
	rdfs:label "has citation"@en, "hat Zitat"@de;
	rdfs:comment "Relating a text to a citation thereof."@en;
	rdfs:domain text:Text;
	rdfs:range text:Citation;
	rdfs:subPropertyOf knora-base:hasLinkTo;
	knora-base:subjectClassConstraint text:Text;
	knora-base:objectClassConstraint text:Citation.

text:hasCitationValue
	a owl:ObjectProperty;
	rdfs:label "has citation - statement"@en, "hat Zitat - Festlegung"@de;
	rdfs:comment "Relating a text to a reification statement of the relation between the text and a citation thereof."@en;
	rdfs:subPropertyOf knora-base:hasLinkToValue;
	knora-base:subjectClassConstraint text:Text;
	knora-base:objectClassConstraint knora-base:LinkValue.

text:hasCitationReferenceIdentifier
	a owl:ObjectProperty;
	rdfs:label "has citation reference identifier"@en, "hat Zitatreferenzidentifikator"@de;
	rdfs:comment "Relating a text to a citation reference identifier thereof."@en;
	rdfs:domain text:Text;
	rdfs:range text:CitationReferenceIdentifier;
	rdfs:subPropertyOf knora-base:hasLinkTo;
	knora-base:subjectClassConstraint text:Text;
	knora-base:objectClassConstraint text:CitationReferenceIdentifier.

text:hasCitationReferenceIdentifierValue
	a owl:ObjectProperty;
	rdfs:label "has citation reference identifier - statement"@en, "hat Zitatreferenzidentifikator - Festlegung"@de;
	rdfs:comment "Relating a text to a reification statement of the relation between the text and a citation reference identifier thereof."@en;
	rdfs:subPropertyOf knora-base:hasLinkToValue;
	knora-base:subjectClassConstraint text:Text;
	knora-base:objectClassConstraint knora-base:LinkValue.

text:hasCitationReferenceNumber
	a owl:ObjectProperty;
	rdfs:label "has citation reference number"@en, "hat Zitatreferenznummer"@de;
	rdfs:comment "Relating a text to a citation reference number thereof."@en;
	rdfs:domain text:Text;
	rdfs:range text:CitationReferenceNumber;
	rdfs:subPropertyOf knora-base:hasLinkTo;
	knora-base:subjectClassConstraint text:Text;
	knora-base:objectClassConstraint text:CitationReferenceNumber.

text:hasCitationReferenceNumberValue
	a owl:ObjectProperty;
	rdfs:label "has citation reference number - statement"@en, "hat Zitatreferenznummer - Festlegung"@de;
	rdfs:comment "Relating a text to a reification statement of the relation between the text and a citation reference number thereof."@en;
	rdfs:subPropertyOf knora-base:hasLinkToValue;
	knora-base:subjectClassConstraint text:Text;
	knora-base:objectClassConstraint knora-base:LinkValue.

text:isCitedIn
	a owl:ObjectProperty;
	rdfs:label "is cited in"@en, "ist zitiert in"@de;
	rdfs:comment "Relating a text to an expression wherein it is cited."@en;
	rdfs:domain text:Text;
	rdfs:range document:Expression;
	rdfs:subPropertyOf knora-base:hasLinkTo;
	knora-base:subjectClassConstraint text:Text;
	knora-base:objectClassConstraint document:Expression.

text:isCitedInValue
	a owl:ObjectProperty;
	rdfs:label "is cited in - statement"@en, "ist zitiert in - Festlegung"@de;
	rdfs:comment "Relating a text to a reification statement of the relation between the text and an expression wherein it is cited."@en;
	rdfs:subPropertyOf knora-base:hasLinkToValue;
	knora-base:subjectClassConstraint text:Text;
	knora-base:objectClassConstraint knora-base:LinkValue.

text:hasEditor
	a owl:ObjectProperty;
	rdfs:label "text has editor"@en, "Text hat Editor"@de;
	rdfs:comment """Relating a text to a person who edited it."""@en;
	rdfs:domain text:Text;
#	rdfs:range [rdfs:subClassOf human:Person, [a owl:Restriction; owl:onProperty human:personHasRole; owl:someValuesFrom textedit:Editor]];
	rdfs:subPropertyOf knora-base:hasLinkTo;
	knora-base:subjectClassConstraint text:Text;
	knora-base:objectClassConstraint human:Person.

text:hasEditorValue
	a owl:ObjectProperty;
	rdfs:label "text has editor - statement"@en, "Text hat Editor - Festlegung"@de;
	rdfs:comment """Relating a text to a reification statement of the relation between the text and a person who edited it."""@en;
	rdfs:subPropertyOf knora-base:hasLinkToValue;
	knora-base:subjectClassConstraint text:Text;
	knora-base:objectClassConstraint knora-base:LinkValue.

text:hasAuthor
	a owl:ObjectProperty;
	rdfs:label "text has author"@en, "Text hat Autor"@de;
	rdfs:comment """Relating a text expression to a person who authored it."""@en;
	skos:note """A text can have more than one author."""@en;
	rdfs:domain text:Expression;
#	rdfs:range [rdfs:subClassOf human:Person, [a owl:Restriction; owl:onProperty human:personHasRole; owl:someValuesFrom text:Author]];
	rdfs:subPropertyOf human:hasAuthor;
	knora-base:subjectClassConstraint text:Expression;
	knora-base:objectClassConstraint human:Person.

text:hasAuthorValue
	a owl:ObjectProperty;
	rdfs:label "text has author - statement"@en, "Text hat Autor - Festlegung"@de;
	rdfs:comment """Relating a text expression to a reification statement of the relation between the text and a person who authored it."""@en;
	rdfs:subPropertyOf human:hasAuthorValue;
	knora-base:subjectClassConstraint text:Expression;
	knora-base:objectClassConstraint knora-base:LinkValue.

text:hasIncipit
	a owl:ObjectProperty;
	rdfs:label "has incipit"@en, "hat Incipit"@de;
	rdfs:comment """Relating an untitled individual text expression to a beginning part thereof to identify the text."""@en;
	rdfs:subPropertyOf text:hasText;
	knora-base:subjectClassConstraint text:IndividualExpression;
	knora-base:objectClassConstraint knora-base:TextValue.

text:hasExplicit
	a owl:ObjectProperty;
	rdfs:label "has explicit"@en, "hat Explicit"@de;
	rdfs:comment """Relating an untitled individual text expression to an end part thereof to identify the text."""@en;
	rdfs:subPropertyOf text:hasText;
	knora-base:subjectClassConstraint text:IndividualExpression;
	knora-base:objectClassConstraint knora-base:TextValue.

text:hasScientificEditor
	a owl:ObjectProperty;
	rdfs:label "text expression has scientific editor"@en, "Text-Expression hat wissenschaftliche Editor"@de;
	rdfs:comment "Relating a text expression to a person who edited it scientifically."@en;
	rdfs:domain text:Expression;
#	rdfs:range [rdfs:subClassOf human:Person, [a owl:Restriction; owl:onProperty human:personHasRole; owl:someValuesFrom textedit:ScientificEditor]];
	rdfs:subPropertyOf knora-base:hasLinkTo;
	knora-base:subjectClassConstraint text:Expression;
	knora-base:objectClassConstraint human:Person.

text:hasScientificEditorValue
	a owl:ObjectProperty;
	rdfs:label "text expression has scientific editor - statement"@en, "Text-Expression hat wissenschaftliche Editor - Festlegung"@de;
	rdfs:comment "Relating a text expression to a reification statement of the relation between the expression and person who edited it scientifically."@en;
	rdfs:subPropertyOf knora-base:hasLinkToValue;
	knora-base:subjectClassConstraint text:Expression;
	knora-base:objectClassConstraint knora-base:LinkValue.

text:hasCriticalEditor
	a owl:ObjectProperty;
	rdfs:label "text expression has critical editor"@en, "Text-Expression hat kritische Editor"@de;
	rdfs:comment "Relating a text expression to a person who edited it critically."@en;
	rdfs:domain text:Expression;
#	rdfs:range [rdfs:subClassOf human:Person, [a owl:Restriction; owl:onProperty human:personHasRole; owl:someValuesFrom textedit:CriticalEditor]];
	rdfs:subPropertyOf knora-base:hasLinkTo;
	knora-base:subjectClassConstraint text:Expression;
	knora-base:objectClassConstraint human:Person.

text:hasCriticalEditorValue
	a owl:ObjectProperty;
	rdfs:label "text expression has critical editor - statement"@en, "Text-Expression hat kritische Editor - Festlegung"@de;
	rdfs:comment "Relating a text expression to a reification statement of the relation between the expression and person who edited it critically."@en;
	rdfs:subPropertyOf knora-base:hasLinkToValue;
	knora-base:subjectClassConstraint text:Expression;
	knora-base:objectClassConstraint knora-base:LinkValue.

text:isPartOfIndividualExpression
	a owl:ObjectProperty;
	rdfs:label "is part of individual text expression"@en, "ist Teil einer individuellen Text-Expression"@de;
	rdfs:comment """Relating a text expression part to an individual expression it is part of."""@en;
	rdfs:domain text:ExpressionPart;
	rdfs:range text:IndividualExpression;
	rdfs:subPropertyOf concept:isPartOf;
	knora-base:subjectClassConstraint text:ExpressionPart;
	knora-base:objectClassConstraint text:IndividualExpression.

text:isPartOfIndividualExpressionValue
	a owl:ObjectProperty;
	rdfs:label "is part of individual text expression - statement"@en, "ist Teil einer individuellen Text-Expression - Festlegung"@de;
	rdfs:comment """Relating a text expression part to a reification statement of the relation between the part and an individual expression it is part of."""@en;
	rdfs:subPropertyOf concept:isPartOfValue;
	knora-base:subjectClassConstraint text:ExpressionPart;
	knora-base:objectClassConstraint knora-base:LinkValue.

text:citationHasIdentifier
	a owl:ObjectProperty;
	rdfs:label "citation has identifier"@en, "Zitat hat Identifikator"@de;
	rdfs:comment """Relating a citation to an identifier (as resource) it has."""@en;
	rdfs:domain text:Citation;
	rdfs:range text:CitationIdentifier;
	rdfs:subPropertyOf knora-base:hasLinkTo;
	knora-base:subjectClassConstraint text:Citation;
	knora-base:objectClassConstraint text:CitationIdentifier.

text:citationHasIdentifierValue
	a owl:ObjectProperty;
	rdfs:label "citation has identifier - statement"@en, "Zitat hat Identifikator - Festlegung"@de;
	rdfs:comment """Relating a citation to a reification statement of the relation between the citation and an identifier (as resource) it has."""@en;
	rdfs:subPropertyOf knora-base:hasLinkToValue;
	knora-base:subjectClassConstraint text:Citation;
	knora-base:objectClassConstraint knora-base:LinkValue.

text:citationHasNumber
	a owl:ObjectProperty;
	rdfs:label "citation has number"@en, "Zitat hat Nummer"@de;
	rdfs:comment """Relating a citation to a natural number (as resource) it has."""@en;
	rdfs:domain text:Citation;
	rdfs:range text:CitationNumber;
	rdfs:subPropertyOf text:citationHasIdentifier;
	knora-base:subjectClassConstraint text:Citation;
	knora-base:objectClassConstraint text:CitationNumber.

text:citationHasNumberValue
	a owl:ObjectProperty;
	rdfs:label "citation has number - statement"@en, "Zitat hat Nummer - Festlegung"@de;
	rdfs:comment """Relating a citation to a reification statement of the relation between the citation and a natural number (as resource) it has."""@en;
	rdfs:subPropertyOf text:citationHasIdentifierValue;
	knora-base:subjectClassConstraint text:Citation;
	knora-base:objectClassConstraint knora-base:LinkValue.

text:citationIsPartOf
	a owl:ObjectProperty;
	rdfs:label "citation is part of text expression"@en, "Zitat ist Teil einer Text-Expression"@de;
	rdfs:comment """Relating a citation to a text expression it is part of."""@en;
	rdfs:domain text:Citation;
	rdfs:range text:Expression;
	rdfs:subPropertyOf concept:isPartOf;
	knora-base:subjectClassConstraint text:Citation;
	knora-base:objectClassConstraint text:Expression.

text:citationIsPartOfValue
	a owl:ObjectProperty;
	rdfs:label "citation is part of text expression - statement"@en, "Zitat ist Teil einer Text-Expression - Festlegung"@de;
	rdfs:comment """Relating a citation to a reification statement of the relation between the citation and a text expression it is part of."""@en;
	rdfs:subPropertyOf concept:isPartOfValue;
	knora-base:subjectClassConstraint text:Citation;
	knora-base:objectClassConstraint knora-base:LinkValue.

text:hasCitationIdentifier
	a owl:ObjectProperty;
	rdfs:label "has citation identifier"@en, "hat Zitatidentifikator"@de;
	rdfs:comment """Relating a citation reference identifier (as resource) to its citation identifier (as resource)."""@en;
	rdfs:domain text:CitationReferenceIdentifier;
	rdfs:range text:CitationIdentifier;
	rdfs:subPropertyOf knora-base:hasLinkTo;
	knora-base:subjectClassConstraint text:CitationReferenceIdentifier;
	knora-base:objectClassConstraint text:CitationIdentifier.

text:hasCitationIdentifierValue
	a owl:ObjectProperty;
	rdfs:label "has citation identifier - statement"@en, "hat Zitatidentifikator - Festlegung"@de;
	rdfs:comment """Relating a citation reference identifier (as resource) to a reification statement of the relation between that identifier and its citation identifier (as resource)."""@en;
	rdfs:subPropertyOf knora-base:hasLinkToValue;
	knora-base:subjectClassConstraint text:CitationReferenceIdentifier;
	knora-base:objectClassConstraint knora-base:LinkValue.

text:hasCitationNumber
	a owl:ObjectProperty;
	rdfs:label "has citation number"@en, "hat Zitatnummer"@de;
	rdfs:comment """Relating a citation reference number (as resource) to its citation number (as resource)."""@en;
	rdfs:domain text:CitationReferenceNumber;
	rdfs:range text:CitationNumber;
	rdfs:subPropertyOf text:hasCitationIdentifier;
	knora-base:subjectClassConstraint text:CitationReferenceNumber;
	knora-base:objectClassConstraint text:CitationNumber.

text:hasCitationNumberValue
	a owl:ObjectProperty;
	rdfs:label "has citation reference number - statement"@en, "hat Zitatnummer - Festlegung"@de;
	rdfs:comment """Relating a citation reference number (as resource) to a reification statement of the relation between that number and its citation number (as resource)."""@en;
	rdfs:subPropertyOf text:hasCitationIdentifierValue;
	knora-base:subjectClassConstraint text:CitationReferenceNumber;
	knora-base:objectClassConstraint knora-base:LinkValue.

text:isEntryOfDiaryExpression
	a owl:ObjectProperty;
	rdfs:label "is entry of diary expression"@en, "ist Eingabe einer Tagebuch-Expression"@de;
	rdfs:comment """Relating a diary entry to its diary expression."""@en;
	rdfs:domain text:DiaryEntry;
	rdfs:range text:DiaryExpression;
	rdfs:subPropertyOf concept:isPartOf;
	knora-base:subjectClassConstraint text:DiaryEntry;
	knora-base:objectClassConstraint text:DiaryExpression.

text:isEntryOfDiaryExpressionValue
	a owl:ObjectProperty;
	rdfs:label "is entry of diary expression - statement"@en, "ist Eingabe einer Tagebuch-Expression - Festlegung"@de;
	rdfs:comment """Relating a diary entry to a reification statement of the relation between that entry and its diary expression."""@en;
	rdfs:subPropertyOf concept:isPartOfValue;
	knora-base:subjectClassConstraint text:DiaryEntry;
	knora-base:objectClassConstraint knora-base:LinkValue.