@prefix rdfs: <http://www.w3.org/2000/01/rdf-schema#>.
@prefix owl: <http://www.w3.org/2002/07/owl#>.
@prefix xsd: <http://www.w3.org/2001/XMLSchema#>.
@prefix skos: <http://www.w3.org/2004/02/skos/core#>.
@prefix dct: <http://purl.org/dc/terms/>.
@prefix foaf: <http://xmlns.com/foaf/0.1/>.
@prefix cidoc: <http://www.cidoc-crm.org/cidoc-crm/>.
@prefix rico: <https://www.ica.org/standards/RiC/ontology#>.
@prefix agent: <http://e-editiones.ch/ontology/agent#>.
@prefix event: <http://e-editiones.ch/ontology/event#>.
@prefix creating: <http://e-editiones.ch/ontology/creating#>.
@prefix concept: <http://e-editiones.ch/ontology/concept#>.
@prefix text: <http://e-editiones.ch/ontology/text#>.
@prefix text-structure: <http://e-editiones.ch/ontology/text-structure#>.
@prefix text-expression: <http://e-editiones.ch/ontology/text-expression#>.
@prefix document: <http://e-editiones.ch/ontology/document#>.
@prefix org: <http://e-editiones.ch/ontology/organization#>.
@prefix publishing: <http://e-editiones.ch/ontology/publishing#>.
@prefix information-carrier: <http://e-editiones.ch/ontology/information-carrier#>.

@base <http://e-editiones.ch/ontology/archive-record>.
@prefix archive-record: <http://e-editiones.ch/ontology/archive-record#>.

<http://e-editiones.ch/ontology/archive-record>
	a owl:Ontology;
	dct:license <http://creativecommons.org/licenses/by/3.0/>;
	dct:title "An ontology about archive record"@en;
	dct:description """Formal description of an archive record, general subclasses, related classes and properties."""@en;
	dct:creator "Rebekka Plüss, research assistant and software developer, University of Basel, Switzerland"@en;
	dct:contributor "Hans Cools, MD, knowledge engineer, ontologist, software developer, University of Basel, Switzerland"@en;
	dct:publisher "Universities of Basel, Bern, and Zürich, Switzerland"@en;
	owl:versionInfo "2020-10-26"^^xsd:date.

#
# CLASSES
#

archive-record:ArchiveRecord
	rdfs:isDefinedBy <http://e-editiones.ch/ontology/archive-record#>;
	a rdfs:Class;
	rdfs:label "archive record"@en, "Archiveinheit"@de;
	rdfs:comment """A record as an entry in an Archive Information System with catalogue data and its primary data on a information carrier belonging to it. This record can be of any level of detail, from an entire archive to a single document or only a part of it."""@en;
	rdfs:subClassOf rico:RecordResource, document:Document.

archive-record:Carrier
	rdfs:isDefinedBy <http://e-editiones.ch/ontology/archive-record#>;
	a rdfs:Class;
	rdfs:label "carrier"@en, "Träger"@de;
	rdfs:comment """The physical or electronical carrier of the archive record, the archival material type. This can be, f. e., a book, a paper file, a collection of them or an electronic carrier as file or folder on the archive server,..."""@en;
	rdfs:subClassOf rico:CarrierType, information-carrier:Carrier.

archive-record:Provenance
	rdfs:isDefinedBy <http://e-editiones.ch/ontology/archive-record#>;
	a rdfs:Class;
	rdfs:label "provenance"@en, "Provenienz"@de;
	rdfs:comment """The agent (f.e. organization, person), which created the archive record originally for its own purposes."""@en;
	rdfs:subClassOf agent:Agent, rico:Agent.

archive-record:Volume
	rdfs:isDefinedBy <http://e-editiones.ch/ontology/archive-record#>;
	a rdfs:Class;
	rdfs:label "volume"@en, "Band"@de;
	rdfs:comment """Volume as type of the carrier resp. the archival material type. It is also a special book: One book of a serie of books. One serie is a set of books which are mostly created for the same purpose by the same provenance."""@en;
	rdfs:subClassOf archive-record:Carrier, information-carrier:Volume, archive-record:Book.

archive-record:Book
	rdfs:isDefinedBy <http://e-editiones.ch/ontology/archive-record#>;
	a rdfs:Class;
	rdfs:label "book"@en, "Buch"@de;
	rdfs:comment """Book as type of the carrier resp. the archival material type."""@en;
	rdfs:subClassOf archive-record:Carrier, information-carrier:Book.

archive-record:PaperFile
	rdfs:isDefinedBy <http://e-editiones.ch/ontology/archive-record#>;
	a rdfs:Class;
	rdfs:label "paper file"@en, "Papierdossier"@de;
	rdfs:comment """Paper file as type of the carrier resp. the archival material type."""@en;
	rdfs:subClassOf archive-record:Carrier.

archive-record:CarrierReference
	rdfs:isDefinedBy <http://e-editiones.ch/ontology/archive-record#>;
	a rdfs:Class;
	rdfs:label "carrier reference"@en, "Trägerreferenz"@de;
	rdfs:comment """A reference to a part of a carrier. This could be, f.e., a page reference to a volume."""@en;
	rdfs:subClassOf document:ContentStructureReference.

archive-record:Identifier
	rdfs:isDefinedBy <http://e-editiones.ch/ontology/archive-record#>;
	a rdfs:Class;
	rdfs:label "identifier"@en, "Identifikator"@de;
	rdfs:comment """The identifying mark with which an archive record can be clearly identified and referenced. In the context of an archive information system, this is usually the signature."""@en;
	rdfs:subClassOf rico:Identifier.

archive-record:CatalogueEntryWebpage
	rdfs:isDefinedBy <http://e-editiones.ch/ontology/archive-record#>;
	a rdfs:Class;
	rdfs:label "catalogue entry webpage"@en, "Katalogeintrag-Webseite"@de;
	rdfs:comment """Webpage of the catalogue entry in an archive information system."""@en;
	rdfs:subClassOf publishing:WebpagePublication.

#
# PROPERTIES
#

archive-record:hasCarrier
	rdfs:isDefinedBy <http://e-editiones.ch/ontology/archive-record#>;
	a owl:ObjectProperty;
	rdfs:label "archive record has carrier"@en, "Archivdatensatz hat Träger";
	rdfs:comment """Relating a archive record to its physical or electronical carrier."""@en;
	rdfs:domain archive-record:ArchiveRecord;
	rdfs:range archive-record:Carrier;
	rdfs:subPropertyOf rico:hasCarrierType, information-carrier:isOnCarrier.

archive-record:hasCarrierReference
	rdfs:isDefinedBy <http://e-editiones.ch/ontology/archive-record#>;
	a owl:ObjectProperty;
	rdfs:label "archive record has carrier reference"@en, "Archivdatensatz hat Trägerreferenz";
	rdfs:comment """Relating a archive record to its reference in its physical or electronical carrier, f.e. archive record has carrier reference page in a volume."""@en;
	rdfs:domain archive-record:ArchiveRecord;
	rdfs:range archive-record:CarrierReference.

archive-record:isheldbyArchive
	rdfs:isDefinedBy <http://e-editiones.ch/ontology/archive-record#>;
	a owl:ObjectProperty;
	rdfs:label "archive record is held by archive"@en, "Archivdatensatz wird geführt von Archiv";
	rdfs:comment """Relating a archive record to its archive in which it is stored and recorded. The archive is responsible for the publishing and managing of an archive record."""@en;
	rdfs:domain archive-record:ArchiveRecord;
	rdfs:range org:Archive.

archive-record:hasProvenance
	rdfs:isDefinedBy <http://e-editiones.ch/ontology/archive-record#>;
	a owl:ObjectProperty;
	rdfs:label "archive record has provenance"@en, "Archivdatensatz hat Provenienz";
	rdfs:comment """Relating a archive record to the agent, which originally created the archive record for its own purposes."""@en;
	rdfs:domain archive-record:ArchiveRecord;
	rdfs:range archive-record:Provenance;
	rdfs:subPropertyOf rico:hasProvenance.

archive-record:hasWebpage
	rdfs:isDefinedBy <http://e-editiones.ch/ontology/archive-record#>;
	a owl:ObjectProperty;
	rdfs:label "archive record has webpage"@en, "Archivdatensatz hat Webseite";
	rdfs:comment """Relating a archive record to the webpage of the catalogue entry in an archive information system."""@en;
	rdfs:domain archive-record:ArchiveRecord;
	rdfs:range archive-record:CatalogueEntryWebpage;
	rdfs:subPropertyOf publishing:hasWebPublication.

archive-record:isRepresentedBy
	rdfs:isDefinedBy <http://e-editiones.ch/ontology/archive-record#>;
	a owl:ObjectProperty;
	rdfs:label "is represented by archive record"@en, "wird durch Archiveinheit dargestellt";
	rdfs:comment """Relating something in the world (an event, a thing...) to the archive record it is represented by."""@en;
	rdfs:domain rdfs:Resource;
	rdfs:range archive-record:ArchiveRecord;
	owl:inverseOf archive-record:represents. #°

archive-record:represents
	rdfs:isDefinedBy <http://e-editiones.ch/ontology/archive-record#>;
	a owl:ObjectProperty;
	rdfs:label "archive record represents"@en, "Archiveinheit stellt dar";
	rdfs:comment """Relating an archive record to what (an event, a thing...) it represents."""@en;
	rdfs:domain archive-record:ArchiveRecord;
	rdfs:range rdfs:Resource;
	owl:inverseOf archive-record:isRepresentedBy.


