@prefix rdfs: <http://www.w3.org/2000/01/rdf-schema#>.
@prefix owl: <http://www.w3.org/2002/07/owl#>.
@prefix xsd: <http://www.w3.org/2001/XMLSchema#>.
@prefix skos: <http://www.w3.org/2004/02/skos/core#>.
@prefix dct: <http://purl.org/dc/terms/>.
@prefix rico: <https://www.ica.org/standards/RiC/ontology#>.
@prefix agent: <http://e-editiones.ch/ontology/agent#>.
@prefix document: <http://e-editiones.ch/ontology/document#>.
@prefix organization: <http://e-editiones.ch/ontology/organization#>.
@prefix publishing: <http://e-editiones.ch/ontology/publishing#>.
@prefix information-carrier: <http://e-editiones.ch/ontology/information-carrier#>.

@base <http://e-editiones.ch/ontology/archive-record>.
@prefix archive-record: <http://e-editiones.ch/ontology/archive-record#>.

<http://e-editiones.ch/ontology/archive-record>
	a owl:Ontology;
	dct:license <http://creativecommons.org/licenses/by/3.0/>;
	dct:title "An ontology about archive record"@en;
	dct:description """Formal description of an archive record, general subclasses, related classes and properties."""@en;
	dct:creator "Rebekka Plüss, research assistant and software developer, University of Basel, Switzerland"@en;
	dct:contributor "Hans Cools, MD, knowledge engineer, ontologist, software developer, University of Basel, Switzerland"@en;
	dct:publisher "Universities of Basel, Bern, and Zürich, Switzerland"@en;
	owl:versionInfo "2020-10-26"^^xsd:date.

#
# CLASSES
#

archive-record:ArchiveRecord
	rdfs:isDefinedBy <http://e-editiones.ch/ontology/archive-record#>;
	a rdfs:Class;
	rdfs:label "archive record"@en, "Archiveinheit"@de;
	rdfs:comment """A record as an entry in an Archive Information System with catalogue data and its primary data on an information carrier belonging to it. This record can be of any level of detail, from an entire archive to a single document or only a part of it."""@en;
	rdfs:subClassOf rico:RecordResource, document:Document.

archive-record:Carrier
	rdfs:isDefinedBy <http://e-editiones.ch/ontology/archive-record#>;
	a rdfs:Class;
	rdfs:label "archive record carrier"@en, "Archiveinheitträger"@de;
	rdfs:comment """Carrier of an archive record, i.e. the archival material. This can be, f. e., a book, a paper file, a collection of them or an electronic carrier as file or folder on the archive server"""@en;
	rdfs:subClassOf rico:CarrierType, information-carrier:Carrier.

archive-record:Provenance
	rdfs:isDefinedBy <http://e-editiones.ch/ontology/archive-record#>;
	a rdfs:Class;
	rdfs:label "archive record provenance"@en, "Archiveinheitprovenienz"@de;
	rdfs:comment """Agent, i.e. organization or person, who created the archive record originally for own purpose."""@en;
	rdfs:subClassOf agent:Agent, rico:Agent.

archive-record:Book
	rdfs:isDefinedBy <http://e-editiones.ch/ontology/archive-record#>;
	a rdfs:Class;
	rdfs:label "archive record book"@en, "Archiveinheitbuch"@de;
	rdfs:comment """Archive record carrier as book."""@en;
	rdfs:subClassOf archive-record:Carrier, information-carrier:Book.

archive-record:Volume
	rdfs:isDefinedBy <http://e-editiones.ch/ontology/archive-record#>;
	a rdfs:Class;
	rdfs:label "archive record volume"@en, "Archiveinheitband"@de;
	rdfs:comment """Archive record book as volume. It is also a special book: One book of a serie of books. One serie is a set of books which are mostly created for the same purpose by the same provenance."""@en;
	rdfs:subClassOf information-carrier:Volume, archive-record:Book.

archive-record:PaperFile
	rdfs:isDefinedBy <http://e-editiones.ch/ontology/archive-record#>;
	a rdfs:Class;
	rdfs:label "archive record carrier as paper file"@en, "Archiveinheit-Papierdossier"@de;
	rdfs:comment """Archive record as paper file."""@en;
	rdfs:subClassOf archive-record:Carrier.

archive-record:CarrierReference
	rdfs:isDefinedBy <http://e-editiones.ch/ontology/archive-record#>;
	a rdfs:Class;
	rdfs:label "archive record carrier reference"@en, "Archiveinheitträgerreferenz"@de;
	rdfs:comment """A reference from an archive record to a part of a carrier, e.g. a reference to a page of a volume."""@en;
	rdfs:subClassOf document:ContentStructureReference. # text-structure:CompositionalContentStructure

archive-record:Identifier
	rdfs:isDefinedBy <http://e-editiones.ch/ontology/archive-record#>;
	a rdfs:Class;
	rdfs:label "archive record identifier"@en, "Archiveinheitidentifikator"@de;
	rdfs:comment """Identifier of an archive record. In the context of an archive information system, this is usually the signature."""@en;
	rdfs:subClassOf rico:Identifier.

archive-record:CatalogueEntryWebpage
	rdfs:isDefinedBy <http://e-editiones.ch/ontology/archive-record#>;
	a rdfs:Class;
	rdfs:label "catalogue entry webpage"@en, "Katalogeintrag-Webseite"@de;
	rdfs:comment """Webpage of the catalogue entry in an archive information system."""@en;
	rdfs:subClassOf publishing:WebpagePublication. # electronic-information:Webpage

#
# PROPERTIES
#

archive-record:hasCarrier
	rdfs:isDefinedBy <http://e-editiones.ch/ontology/archive-record#>;
	a owl:ObjectProperty;
	rdfs:label "archive record has carrier"@en, "Archivdatensatz hat Träger";
	rdfs:comment """Relating an archive record to its carrier."""@en;
	rdfs:domain archive-record:ArchiveRecord;
	rdfs:range archive-record:Carrier;
	rdfs:subPropertyOf rico:hasCarrierType, information-carrier:isOnCarrier.

archive-record:hasCarrierReference
	rdfs:isDefinedBy <http://e-editiones.ch/ontology/archive-record#>;
	a owl:ObjectProperty;
	rdfs:label "archive record has carrier reference"@en, "Archivdatensatz hat Trägerreferenz";
	rdfs:comment """Relating an archive record to its reference to a carrier part, f.e. a page in a volume."""@en;
	rdfs:domain archive-record:ArchiveRecord;
	rdfs:range archive-record:CarrierReference.

archive-record:isheldbyArchive
	rdfs:isDefinedBy <http://e-editiones.ch/ontology/archive-record#>;
	a owl:ObjectProperty;
	rdfs:label "archive record is held by archive"@en, "Archivdatensatz wird geführt von Archiv";
	rdfs:comment """Relating an archive record to its archive in which it is stored and recorded. The archive is responsible for the publishing and managing of an archive record."""@en;
	rdfs:domain archive-record:ArchiveRecord;
	rdfs:range organization:Archive.

archive-record:hasProvenance
	rdfs:isDefinedBy <http://e-editiones.ch/ontology/archive-record#>;
	a owl:ObjectProperty;
	rdfs:label "archive record has provenance"@en, "Archivdatensatz hat Provenienz";
	rdfs:comment """Relating an archive record to the agent, which originally created the archive record for its own purposes."""@en;
	rdfs:domain archive-record:ArchiveRecord;
	rdfs:range archive-record:Provenance;
	rdfs:subPropertyOf rico:hasProvenance.

archive-record:hasWebpage
	rdfs:isDefinedBy <http://e-editiones.ch/ontology/archive-record#>;
	a owl:ObjectProperty;
	rdfs:label "archive record has webpage"@en, "Archivdatensatz hat Webseite";
	rdfs:comment """Relating an archive record to the webpage of the catalogue entry in an archive information system."""@en;
	rdfs:domain archive-record:ArchiveRecord;
	rdfs:range archive-record:CatalogueEntryWebpage;
	rdfs:subPropertyOf publishing:hasWebPublication.

archive-record:isRepresentedBy
	rdfs:isDefinedBy <http://e-editiones.ch/ontology/archive-record#>;
	a owl:ObjectProperty;
	rdfs:label "is represented by archive record"@en, "wird durch Archiveinheit dargestellt";
	rdfs:comment """Relating something in the world (an event, a thing...) to the archive record it is represented by."""@en;
	rdfs:domain rdfs:Resource;
	rdfs:range archive-record:ArchiveRecord;
	owl:inverseOf archive-record:represents.

archive-record:represents
	rdfs:isDefinedBy <http://e-editiones.ch/ontology/archive-record#>;
	a owl:ObjectProperty;
	rdfs:label "archive record represents"@en, "Archiveinheit stellt dar";
	rdfs:comment """Relating an archive record to what (an event, a thing...) it represents."""@en;
	rdfs:domain archive-record:ArchiveRecord;
	rdfs:range rdfs:Resource;
	owl:inverseOf archive-record:isRepresentedBy.


