@prefix rdfs: <http://www.w3.org/2000/01/rdf-schema#>.
@prefix owl: <http://www.w3.org/2002/07/owl#>.
@prefix xsd: <http://www.w3.org/2001/XMLSchema#>.
@prefix skos: <http://www.w3.org/2004/02/skos/core#>.
@prefix dct: <http://purl.org/dc/terms/>.
@prefix foaf: <http://xmlns.com/foaf/0.1/>.
@prefix cidoc: <http://www.cidoc-crm.org/cidoc-crm/>.
@prefix rico: <https://www.ica.org/standards/RiC/ontology#>.
@prefix event: <http://e-editiones.ch/ontology/event#>.
@prefix creating: <http://e-editiones.ch/ontology/creating#>.
@prefix concept: <http://e-editiones.ch/ontology/concept#>.
@prefix text: <http://e-editiones.ch/ontology/text#>.
@prefix text-structure: <http://e-editiones.ch/ontology/text-structure#>.
@prefix text-expression: <http://e-editiones.ch/ontology/text-expression#>.
@prefix document: <http://e-editiones.ch/ontology/document#>.
@prefix org: <http://e-editiones.ch/ontology/organization#>.

@base <http://e-editiones.ch/ontology/archive-record>.
@prefix archive-record: <http://e-editiones.ch/ontology/archive-record#>.

<http://e-editiones.ch/ontology/archive-record>
	a owl:Ontology;
	dct:license <http://creativecommons.org/licenses/by/3.0/>;
	dct:title "An ontology about archive record"@en;
	dct:description """Formal description of an archive record, general subclasses, related classes and properties."""@en;
	dct:creator "Rebekka Plüss, research assistant and software developer, University of Basel, Switzerland"@en;
	dct:contributor "Hans Cools, MD, knowledge engineer, ontologist, software developer, University of Basel, Switzerland"@en;
	dct:publisher "Universities of Basel, Bern, and Zürich, Switzerland"@en;
	owl:versionInfo "2020-10-26"^^xsd:date.

#
# CLASSES
#

archive-record:ArchiveRecord
	rdfs:isDefinedBy <http://e-editiones.ch/ontology/archive-record#>;
	a rdfs:Class;
	rdfs:label "archive record"@en, "Archivalie"@de;
	rdfs:comment """A record as an entry in an Archive Information System. This record can be f.e. one or more fonds, one or more dossiers, one or more documents, one or more parts of a document,..."""@en;
	rdfs:subClassOf rico:Record, rico:Instantiation, creating:Creation, document:Document.

archive-record:Carrier
	rdfs:isDefinedBy <http://e-editiones.ch/ontology/archive-record#>;
	a rdfs:Class;
	rdfs:label "carrier"@en, "Träger"@de;
	rdfs:comment """The physical or electronical carrier of the archive record, the archival material type. This can be, f. e., a book, a paper file, a collection of them or an electronic carrier as file or folder on the archive server,..."""@en;
	rdfs:subClassOf rico:CarrierType.

archive-record:Volume
	rdfs:isDefinedBy <http://e-editiones.ch/ontology/archive-record#>;
	a rdfs:Class;
	rdfs:label "volume"@en, "Band"@de;
	rdfs:comment """Volume as type of the carrier resp. the archival material type."""@en;
	rdfs:subClassOf archive-record:Carrier.

archive-record:Book
	rdfs:isDefinedBy <http://e-editiones.ch/ontology/archive-record#>;
	a rdfs:Class;
	rdfs:label "book"@en, "Buch"@de;
	rdfs:comment """Book as type of the carrier resp. the archival material type."""@en;
	rdfs:subClassOf archive-record:Carrier.

archive-record:PaperFile
	rdfs:isDefinedBy <http://e-editiones.ch/ontology/archive-record#>;
	a rdfs:Class;
	rdfs:label "paper file"@en, "Papierdossier"@de;
	rdfs:comment """Paper file as type of the carrier resp. the archival material type."""@en;
	rdfs:subClassOf archive-record:Carrier.

archive-record:CarrierReference
	rdfs:isDefinedBy <http://e-editiones.ch/ontology/archive-record#>;
	a rdfs:Class;
	rdfs:label "carrier reference"@en, "Trägerreferenz"@de;
	rdfs:comment """A reference in a carrier. This could be, f.e., a page in a volume."""@en;
	rdfs:subClassOf document:Structure, concept:Identifier.


#
# PROPERTIES
#

archive-record:hasCarrier
	rdfs:isDefinedBy <http://e-editiones.ch/ontology/archive-record#>;
	a owl:ObjectProperty;
	rdfs:label "archive record has carrier"@en, "Archivalie hat Träger";
	rdfs:comment """Relating a archive record to its physical or electronical carrier."""@en;
	rdfs:domain archive-record:ArchiveRecord;
	rdfs:range archive-record:Carrier;
	rdfs:subPropertyOf rico:hasCarrierType.


archive-record:hasCarrierReference
	rdfs:isDefinedBy <http://e-editiones.ch/ontology/archive-record#>;
	a owl:ObjectProperty;
	rdfs:label "archive record has carrier reference"@en, "Archivalie hat Trägerreferenz";
	rdfs:comment """Relating a archive record to its reference in its physical or electronical carrier, f.e. archive record has carrier reference page in a volume."""@en;
	rdfs:domain archive-record:ArchiveRecord;
	rdfs:range archive-record:CarrierReference.


archive-record:isheldbyArchive
	rdfs:isDefinedBy <http://e-editiones.ch/ontology/archive-record#>;
	a owl:ObjectProperty;
	rdfs:label "archive record is held by archive"@en, "Archivalie wird geführt von Archiv";
	rdfs:comment """Relating a archive record to its archive in which it is stored, recorded. The archive is responsible for the publishing of the archive record."""@en;
	rdfs:domain archive-record:ArchiveRecord;
	rdfs:range org:Archive.

