@prefix rdf: <http://www.w3.org/1999/02/22-rdf-syntax-ns#>.
@prefix rdfs: <http://www.w3.org/2000/01/rdf-schema#>.
@prefix owl: <http://www.w3.org/2002/07/owl#>.
@prefix xsd: <http://www.w3.org/2001/XMLSchema#>.
@prefix skos: <http://www.w3.org/2004/02/skos/core#>.
@prefix dct: <http://purl.org/dc/terms/>.
@prefix event: <http://e-editiones.ch/ontology/event#>.
@prefix concept: <http://e-editiones.ch/ontology/concept#>.

@base <http://e-editiones.ch/ontology/calendar>.
@prefix calendar: <http://e-editiones.ch/ontology/calendar#>.

<http://e-editiones.ch/ontology/calendar>
	a owl:Ontology;
	dct:issued "2019-12-28T13:45:00+01:00"^^xsd:dateTime;
	dct:license <http://creativecommons.org/licenses/by/3.0/>;
	dct:title "calendar-ontology"@en;
	dct:description """Formal description of calendar, subclasses, related classes, and properties."""@en;
	dct:creator "Hans Cools, MD, knowledge engineer, ontologist, software developer, University of Basel, Switzerland"@en;
	dct:contributor "Rebekka Plüss, research assistant and software developer, University of Basel, Switzerland"@en;
	dct:publisher "Universities of Basel, Bern, and Zürich, Switzerland"@en;
	owl:versionInfo "2020-06-11"^^xsd:date.

#
# CLASSES
#

calendar:Calendar
	rdfs:isDefinedBy <http://e-editiones.ch/ontology/calendar#>;
	a rdfs:Class;
	rdfs:label "calendar"@en, "Kalender"@de, "calendrier"@fr, "calendario"@it;
	rdfs:comment """System of reckoning time in which the beginning, length, and divisions of a year are defined, sometimes along with multiyear cycles."""@en;
	rdfs:subClassOf concept:Information.

#
# INSTANCES
#

calendar:julianCalendar
	rdfs:isDefinedBy <http://e-editiones.ch/ontology/calendar#>;
	a calendar:Calendar;
	rdfs:label "Julian calendar"@en, "julianischer Kalender"@de, "calendrier julien"@fr, "calendario juliano"@it;
	rdfs:comment """Calendar introduced in 46 BC in Rome by Julius Caesar. It is based on a solar year of 365 days. There are 12 months of 30 or 31 days, except for February, which has 28 days with the exception of every leap year when it has 29 days. Every fourth year and centenary year is a leap year of 366 days. The beginning of a year is not fixed on January 1. It was replaced by the Gregorian calendar in 1582 AD."""@en;
	skos:note """Has 365.25 days/year. This number is used in temoral reasoning."""@en;
	skos:note """A year that is exactly divisible by four is a leap year, except for years that are exactly divisible by 100, but these centurial years are leap years if they are exactly divisible by 400. For example, the years 1700, 1800, and 1900 are not leap years, but the year 2000 is."""@en.

calendar:prolepticJulianCalendar
	rdfs:isDefinedBy <http://e-editiones.ch/ontology/calendar#>;
	a calendar:Calendar;
	rdfs:label "proleptic Julian calendar"@en, "proleptischer julianischer Kalender"@de, "calendrier julien proleptique"@fr, "calendario juliano proleptico"@it;
	rdfs:comment """Produced by extending the Julian calendar backward to dates preceding its use in stable form from 4 AD on."""@en;
	skos:note """There is no proleptic Julian year 0. Year 1 BC is followed by year 1 AD."""@en.

calendar:gregorianCalendar
	rdfs:isDefinedBy <http://e-editiones.ch/ontology/calendar#>;
	a calendar:Calendar;
	rdfs:label "Gregorian calendar"@en, "gregorianischer Kalender"@de, "calendrier grégorien"@fr, "calendario gregoriano"@it;
	rdfs:comment """Calendar introduced on 15 October 1582 AD by Pope Gregory XIII, and a correction of the Julian calendar. It is based on a solar year of 365 days. Every fourth year is a leap year of 366 days except for centenary years not evenly divisible by 400."""@en;
	skos:note """Has 365.2425 days or 365 days, 5 hours, 49 minutes and 12 seconds per year. This number is used in temoral reasoning."""@en.

calendar:prolepticGregorianCalendar
	rdfs:isDefinedBy <http://e-editiones.ch/ontology/calendar#>;
	a calendar:Calendar;
	rdfs:label "proleptic Gregorian calendar"@en, "proleptischer gregorianischer Kalender"@de, "calendrier grégorien proleptique"@fr, "calendario gregoriano proleptico"@it;
	rdfs:comment """Produced by extending the Gregorian calendar backward to dates preceding its introduction on 15 October 1582."""@en;
	skos:note """There is no proleptic Gregorian year 0. Year 1 BC is followed by year 1 AD."""@en.

calendar:julianDate
	rdfs:isDefinedBy <http://e-editiones.ch/ontology/calendar#>;
	a rdfs:Datatype;
	rdfs:label "Julian date datatype"@en, "Datentyp julianisches Datum"@de;
	rdfs:comment """Datatype to type a date in the Julian calendar."""@en.

calendar:prolepticJulianDate
	rdfs:isDefinedBy <http://e-editiones.ch/ontology/calendar#>;
	a rdfs:Datatype;
	rdfs:label "proleptic Julian date datatype"@en, "Datentyp proleptisches julianisches Datum"@de;
	rdfs:comment """Datatype to type a date in the proleptic Julian calendar."""@en.

calendar:julianDayNumber
	rdfs:isDefinedBy <http://e-editiones.ch/ontology/calendar#>;
	a rdfs:Datatype;
	rdfs:label "Julian Day Number datatype"@en, "Datentyp julianische Tagesnummer"@de;
	rdfs:comment """Datatype to type a Julian Day Number integer."""@en;
	rdfs:comment """The Julian Day Number (JDN) is the integer assigned to a whole solar day in the Julian day count starting from noon Universal time, with Julian Day Number 0 assigned to the day starting at noon on Monday, January 1, 4713 BC, proleptic Julian calendar (November 24, 4714 BC, in the proleptic Gregorian calendar), a date at which three multi-year cycles started (Indiction, Solar, and Lunar cycles) and which precedes any date in recorded human history."""@en;
	rdfs:subClassOf xsd:integer.

#
# PROPERTIES
#

calendar:hasMessageLiteral
	rdfs:isDefinedBy <http://e-editiones.ch/ontology/calendar#>;
	a owl:DatatypeProperty;
	rdfs:label "has message literal"@en, "hat Nachrichtliteral"@de;
	rdfs:comment """Relating something to a message literal about a calendar related time expression about that something."""@en;
	skos:note """Used in an N3-rule; e.g. checking on leap year: "Has leap year."; e.g. checking consistency of e.g. month number, in case > 12: "There are only 12 months in the Gregorian, Julian or proleptic Julian calendar." """@en;
	rdfs:domain rdfs:Resource;
	rdfs:range rdfs:Literal.

calendar:hasCalendar
	rdfs:isDefinedBy <http://e-editiones.ch/ontology/calendar#>;
	a owl:ObjectProperty;
	rdfs:label "has calendar"@en, "hat Kalender"@de;
	rdfs:comment """Relating an event to a calendar."""@en;
	rdfs:domain rdfs:Resource; # event:Event;
	rdfs:range calendar:Calendar.

calendar:dateLiteralToDate
	rdfs:isDefinedBy <http://e-editiones.ch/ontology/calendar#>;
	a owl:ObjectProperty;
	rdfs:label "date literal to date"@en, "Datumliteral zu Datum"@de;
	rdfs:comment """Relating a calendar date as a literal list to the list with a calendar-dependent date typed literal."""@en;
	skos:note """Used in the premise of an N3-rule to invoke the backward N3-rule converting a date literal list to the list with the calendar-dependent date typed literal and the Julian Day Number for temporal reasoning."""@en;
	rdfs:domain rdf:List;
	rdfs:range rdf:List.

calendar:yearLiteralToPeriod
	rdfs:isDefinedBy <http://e-editiones.ch/ontology/calendar#>;
	a owl:ObjectProperty;
	rdfs:label "year literal to period"@en, "Jahrliteral zu Zeitraum"@de;
	rdfs:comment """Relating a calendar year literal to the list with the calendar-dependent start and end date typed literal, and start and end Julian Day Number of the year."""@en;
	skos:note """Used in the premise of an N3-rule to invoke the backward N3-rule converting a year literal to the described list, making explicit the start and end of the year for interval calculus in temporal reasoning."""@en;
	rdfs:domain rdf:List;
	rdfs:range rdf:List.

calendar:yearMonthLiteralToPeriod
	rdfs:isDefinedBy <http://e-editiones.ch/ontology/calendar#>;
	a owl:ObjectProperty;
	rdfs:label "year month literal to period"@en, "Jahr- und Monatliteral zu Zeitraum"@de;
	rdfs:comment """Relating a calendar year-month literal list to the list with the calendar-dependent start and end date typed literal, and start and end Julian Day Number of the month."""@en;
	skos:note """Used in the premise of an N3-rule to invoke the backward N3-rule converting a year-month literal list to the described object list, making explicit the start and end of the month for interval calculus in temporal reasoning."""@en;
	rdfs:domain rdf:List;
	rdfs:range rdf:List.

calendar:yearLiteralToDecadePeriod
	rdfs:isDefinedBy <http://e-editiones.ch/ontology/calendar#>;
	a owl:ObjectProperty;
	rdfs:label "year literal to decade period"@en, "Jahrliteral zu Jahrzehnt"@de;
	rdfs:comment """Relating a list with a decade start year literal and its calendar to the list with the calendar-dependent start and end date typed literal, and start and end Julian Day Number of the decade."""@en;
	skos:note """Used in the premise of an N3-rule to invoke the backward N3-rule converting a decade start year literal to the described object list, making explicit the start and end of the decade for interval calculus in temporal reasoning."""@en;
	rdfs:domain rdf:List;
	rdfs:range rdf:List.

calendar:startYearLiteralToCenturyPeriod
	rdfs:isDefinedBy <http://e-editiones.ch/ontology/calendar#>;
	a owl:ObjectProperty;
	rdfs:label "start year literal to century period"@en, "Startjahrliteral zu Jahrhundert"@de;
	rdfs:comment """Relating a list with a century start year literal and its calendar to the list with the calendar-dependent start and end date typed literal, and start and end Julian Day Number of the century."""@en;
	skos:note """Used in the premise of an N3-rule to invoke the backward N3-rule converting a century start year literal to the described object list, making explicit the start and end of the century for interval calculus in temporal reasoning."""@en;
	skos:note """Used in case of an accuracy of a century for an event time indicator, e.g. Gregorian death year '14..'."""@en;
	rdfs:domain rdf:List;
	rdfs:range rdf:List.

calendar:endYearLiteralToCenturyPeriod
	rdfs:isDefinedBy <http://e-editiones.ch/ontology/calendar#>;
	a owl:ObjectProperty;
	rdfs:label "end year literal to century period"@en, "Endjahrliteral zu Jahrhundert"@de;
	rdfs:comment """Relating a list with a century end year literal and its calendar to the list with the calendar-dependent start and end date typed literal, and start and end Julian Day Number of the century."""@en;
	skos:note """Used in the premise of an N3-rule to invoke the backward N3-rule converting a century end year literal to the described object list, making explicit the start and end of the century for interval calculus in temporal reasoning."""@en;
	skos:note """Used in case of an accuracy of a century for an event time indicator, e.g. Gregorian death year '14..'."""@en;
	rdfs:domain rdf:List;
	rdfs:range rdf:List.

calendar:hasGregorianDate
	rdfs:isDefinedBy <http://e-editiones.ch/ontology/calendar#>;
	a owl:DatatypeProperty;
	rdfs:label "has Gregorian date"@en, "hat gregorianisches Datum"@de;
	rdfs:comment """Relating something to its Gregorian date."""@en;
	rdfs:domain rdfs:Resource;
	rdfs:range xsd:date.

calendar:hasGregorianStartDate
	rdfs:isDefinedBy <http://e-editiones.ch/ontology/calendar#>;
	a owl:DatatypeProperty;
	rdfs:label "has Gregorian start date"@en, "hat gregorianisches Startdatum"@de;
	rdfs:comment """Relating an event to its Gregorian start date."""@en;
	rdfs:domain event:Event;
	rdfs:range xsd:date.

calendar:hasGregorianEndDate
	rdfs:isDefinedBy <http://e-editiones.ch/ontology/calendar#>;
	a owl:DatatypeProperty;
	rdfs:label "has Gregorian end date"@en, "hat gregorianisches Enddatum"@de;
	rdfs:comment """Relating an event to its Gregorian end date."""@en;
	rdfs:domain event:Event;
	rdfs:range xsd:date.

calendar:gregorianListToDate
	rdfs:isDefinedBy <http://e-editiones.ch/ontology/calendar#>;
	a owl:DatatypeProperty;
	rdfs:label "Gregorian list to date"@en, "gregorianische Liste zu Datum"@de;
	rdfs:comment """Relating a Gregorian date as a list of literals to its date typed literal."""@en;
	skos:note """Used in the premise of the backward 'dateLiteralToDate', 'yearLiteralToPeriod', and 'yearMonthLiteralToPeriod' N3-rules for the Gregorian calendar to invoke its backward 'gregorianListToDate' N3-rule converting a Gregorian date literal list to its date typed literal."""@en;
	rdfs:domain rdf:List;
	rdfs:range xsd:date.

calendar:gregorianListToJulianDayNumber
	rdfs:isDefinedBy <http://e-editiones.ch/ontology/calendar#>;
	a owl:DatatypeProperty;
	rdfs:label "Gregorian list to Julian Day Number"@en, "gregorianische Liste zu julianische Tagesnummer"@de;
	rdfs:comment """Relating a Gregorian date as a list of literals to its Julian Day Number."""@en;
	skos:note """Used in the premise of the backward 'dateLiteralToDate', 'yearLiteralToPeriod', and 'yearMonthLiteralToPeriod' N3-rules for the Gregorian calendar to invoke its backward 'gregorianListToJulianDayNumber' N3-rule converting a Gregorian date literal list to its Julian Day Number."""@en;
	rdfs:domain rdf:List;
	rdfs:range calendar:julianDayNumber.

calendar:checkGregorianLeapYear
	rdfs:isDefinedBy <http://e-editiones.ch/ontology/calendar#>;
	a owl:DatatypeProperty;
	rdfs:label "check Gregorian leap year"@en, "gregorianisches Schaltjahr prüfen"@de;
	rdfs:comment """Relating a Gregorian date as a list of literals to the message about the year being leap or not."""@en;
	skos:note """Used in the premise of the backward 'dateLiteralToDate', 'yearLiteralToPeriod', and 'yearMonthLiteralToPeriod' N3-rules for the Gregorian calendar to invoke its backward 'checkGregorianLeapYear' N3-rules returning the literal message for the year being leap or not."""@en;
	rdfs:domain rdf:List;
	rdfs:range rdfs:Literal.

calendar:hasJulianDate
	rdfs:isDefinedBy <http://e-editiones.ch/ontology/calendar#>;
	a owl:DatatypeProperty;
	rdfs:label "has Julian date"@en, "hat julianisches Datum"@de;
	rdfs:comment """Relating something to its Julian date."""@en;
	rdfs:domain rdfs:Resource;
	rdfs:range calendar:julianDate.

calendar:hasJulianStartDate
	rdfs:isDefinedBy <http://e-editiones.ch/ontology/calendar#>;
	a owl:DatatypeProperty;
	rdfs:label "has Julian start date"@en, "hat julianisches Startdatum"@de;
	rdfs:comment """Relating something to its Julian start date."""@en;
	rdfs:domain event:Event;
	rdfs:range calendar:julianDate.

calendar:hasJulianEndDate
	rdfs:isDefinedBy <http://e-editiones.ch/ontology/calendar#>;
	a owl:DatatypeProperty;
	rdfs:label "has Julian end date"@en, "hat julianisches Enddatum"@de;
	rdfs:comment """Relating something to its Julian end date."""@en;
	rdfs:domain event:Event;
	rdfs:range calendar:julianDate.

calendar:julianListToDate
	rdfs:isDefinedBy <http://e-editiones.ch/ontology/calendar#>;
	a owl:DatatypeProperty;
	rdfs:label "Julian list to date"@en, "julianische Liste zu Datum"@de;
	rdfs:comment """Relating a Julian date as a list of literals to its date typed literal."""@en;
	skos:note """Used in the premise of the backward 'dateLiteralToDate' N3-rules for the Julian calendar to invoke its backward 'julianListToDate' N3-rule converting a Julian date literal list to its date typed literal."""@en;
	rdfs:domain rdf:List;
	rdfs:range calendar:julianDate.

calendar:julianListToJulianDayNumber
	rdfs:isDefinedBy <http://e-editiones.ch/ontology/calendar#>;
	a owl:DatatypeProperty;
	rdfs:label "Julian list to Julian Day Number"@en, "julianische Liste zu julianische Tagesnummer"@de;
	rdfs:comment """Relating a Julian date as a list of literals to its Julian Day Number."""@en;
	skos:note """Used in the premise of the backward 'dateLiteralToDate', 'yearLiteralToPeriod', and 'yearMonthLiteralToPeriod' N3-rules to invoke its backward 'julianListToJulianDayNumber' N3-rule converting a Julian date literal list to its Julian Day Number."""@en;
	rdfs:domain rdf:List;
	rdfs:range calendar:julianDayNumber.

calendar:julianSetListToDate
	rdfs:isDefinedBy <http://e-editiones.ch/ontology/calendar#>;
	a owl:DatatypeProperty;
	rdfs:label "Julian set date list to date"@en, "gesetzte julianische Datumliste zu Datum"@de;
	rdfs:comment """Relating a Julian date literal list with set month and day to its date typed literal."""@en;
	skos:note """Used in the premise of the backward 'yearLiteralToPeriod' and 'yearMonthLiteralToPeriod' N3-rules for the Julian calendar to invoke its backward 'julianSetListToDate' N3-rule converting a Julian date literal list to its date typed literal."""@en;
	rdfs:domain rdf:List;
	rdfs:range calendar:julianDate.

calendar:hasProlepticJulianDate
	rdfs:isDefinedBy <http://e-editiones.ch/ontology/calendar#>;
	a owl:DatatypeProperty;
	rdfs:label "has proleptic Julian date"@en, "hat proleptisch julianisches Datum"@de;
	rdfs:comment """Relating something to its proleptic Julian date."""@en;
	rdfs:domain rdfs:Resource;
	rdfs:range calendar:prolepticJulianDate.

calendar:hasProlepticJulianStartDate
	rdfs:isDefinedBy <http://e-editiones.ch/ontology/calendar#>;
	a owl:DatatypeProperty;
	rdfs:label "has proleptic Julian start date"@en, "hat proleptisch julianisches Startdatum"@de;
	rdfs:comment """Relating something to its proleptic Julian start date."""@en;
	rdfs:domain event:Event;
	rdfs:range calendar:prolepticJulianDate.

calendar:hasProlepticJulianEndDate
	rdfs:isDefinedBy <http://e-editiones.ch/ontology/calendar#>;
	a owl:DatatypeProperty;
	rdfs:label "has proleptic Julian end date"@en, "hat proleptisch julianisches Enddatum"@de;
	rdfs:comment """Relating something to its proleptic Julian end date."""@en;
	rdfs:domain event:Event;
	rdfs:range calendar:prolepticJulianDate.

calendar:prolepticJulianListToDate
	rdfs:isDefinedBy <http://e-editiones.ch/ontology/calendar#>;
	a owl:DatatypeProperty;
	rdfs:label "proleptic Julian list to date"@en, "proleptisch julianische Liste zu Datum"@de;
	rdfs:comment """Relating a proleptic Julian date as a list of literals to its date typed literal."""@en;
	skos:note """Used in the premise of the backward 'dateLiteralToDate' N3-rules for the proleptic Julian calendar to invoke its backward 'prolepticJulianListToDate' N3-rule converting a proleptic Julian date literal list to its date typed literal."""@en;
	rdfs:domain rdf:List;
	rdfs:range calendar:prolepticJulianDate.

calendar:prolepticJulianListToJulianDayNumber
	rdfs:isDefinedBy <http://e-editiones.ch/ontology/calendar#>;
	a owl:DatatypeProperty;
	rdfs:label "proleptic Julian list to Julian Day Number"@en, "proleptisch julianische Liste zu julianischer Tagesnummer"@de;
	rdfs:comment """Relating a proleptic Julian date as a list of literals to its Julian Day Number."""@en;
	skos:note """Used in the premise of the backward 'dateLiteralToDate', 'yearLiteralToPeriod', and 'yearMonthLiteralToPeriod' N3-rules to invoke its backward 'prolepticJulianListToJulianDayNumber' N3-rule converting a proleptic Julian date literal list to its Julian Day Number."""@en;
	rdfs:domain rdf:List;
	rdfs:range calendar:julianDayNumber.

calendar:prolepticJulianSetListToDate
	rdfs:isDefinedBy <http://e-editiones.ch/ontology/calendar#>;
	a owl:DatatypeProperty;
	rdfs:label "proleptic Julian set date list to date"@en, "gesetzte proleptisch julianische Datumliste zu Datum"@de;
	rdfs:comment """Relating a proleptic Julian date literal list with set month and day, to its date typed literal."""@en;
	skos:note """Used in the premise of the backward 'yearLiteralToPeriod' and 'yearMonthLiteralToPeriod' N3-rules for the proleptic Julian calendar to invoke its backward 'prolepticJulianSetListToDate' N3-rule converting a proleptic Julian date literal list to its date typed literal."""@en;
	rdfs:domain rdf:List;
	rdfs:range calendar:prolepticJulianDate.

calendar:hasJulianDayNumber
	rdfs:isDefinedBy <http://e-editiones.ch/ontology/calendar#>;
	a owl:DatatypeProperty;
	rdfs:label "has Julian Day Number"@en, "hat julianische Tagesnummer"@de;
	rdfs:comment """Relating something to its Julian Day Number."""@en;
	skos:note """Used in an N3-rule to convert a calendar date literal list to a Julian Day Number."""@en;
	rdfs:domain rdfs:Resource;
	rdfs:range calendar:julianDayNumber.

calendar:hasStartJulianDayNumber
	rdfs:isDefinedBy <http://e-editiones.ch/ontology/calendar#>;
	a owl:DatatypeProperty;
	rdfs:label "has start Julian Day Number"@en, "hat Start-julianische Tagesnummer"@de;
	rdfs:comment """Relating something to its start Julian Day Number."""@en;
	skos:note """Used in an N3-rule to convert a calendar start date literal list of a year or year-month period to a start Julian Day Number integer."""@en;
	rdfs:domain event:Event;
	rdfs:range calendar:julianDayNumber;
	rdfs:subPropertyOf calendar:hasJulianDayNumber.

calendar:hasEndJulianDayNumber
	rdfs:isDefinedBy <http://e-editiones.ch/ontology/calendar#>;
	a owl:DatatypeProperty;
	rdfs:label "has end Julian Day Number"@en, "hat End-julianische Tagesnummer"@de;
	rdfs:comment """Relating an event to its end Julian Day Number."""@en;
	skos:note """Used in an N3-rule to convert a calendar end date literal list of a year or year-month period to an end Julian Day Number integer."""@en;
	rdfs:domain event:Event;
	rdfs:range calendar:julianDayNumber;
	rdfs:subPropertyOf calendar:hasJulianDayNumber.

calendar:julianDayNumeralToGregorianDate
	rdfs:isDefinedBy <http://e-editiones.ch/ontology/calendar#>;
	a owl:DatatypeProperty;
	rdfs:label "Julian Day Numeral to Gregorian date"@en, "julianischer Tag-Numeral zu gregorianischem Datum"@de;
	rdfs:comment """Relating a Julian Day Numeral to its Gregorian date typed literal."""@en;
	skos:note """Used in the premise of an N3-rule to invoke the eponymous backward N3-rule to convert a Julian Day Numeral, i.e. not typed with calendar:julianDayNumber, to its Gregorian date typed literal."""@en;
	rdfs:domain xsd:nonNegativeInteger;
	rdfs:range xsd:date.
