@prefix rdf: <http://www.w3.org/1999/02/22-rdf-syntax-ns#>.
@prefix rdfs: <http://www.w3.org/2000/01/rdf-schema#>.
@prefix owl: <http://www.w3.org/2002/07/owl#>.
@prefix xsd: <http://www.w3.org/2001/XMLSchema#>.
@prefix skos: <http://www.w3.org/2004/02/skos/core#>.
@prefix dct: <http://purl.org/dc/terms/>.
@prefix foaf: <http://xmlns.com/foaf/0.1/>.
@prefix cidoc: <http://www.cidoc-crm.org/cidoc-crm/>.
@prefix frbroo: <http://iflastandards.info/ns/fr/frbr/frbroo/>.
@prefix event: <http://e-editiones.ch/ontology/event#>.
@prefix human: <http://e-editiones.ch/ontology/human#>.
@prefix creating: <http://e-editiones.ch/ontology/creating#>.
@prefix concept: <http://e-editiones.ch/ontology/concept#>.
@prefix math: <http://e-editiones.ch/ontology/mathematics#>.
@prefix ling: <http://e-editiones.ch/ontology/linguistics#>.
@prefix text: <http://e-editiones.ch/ontology/text#>.
@prefix text-structure: <http://e-editiones.ch/ontology/text-structure#>.
@prefix note-structure: <http://e-editiones.ch/ontology/note-structure#>.
@prefix text-expression: <http://e-editiones.ch/ontology/text-expression#>.
@prefix infocar: <http://e-editiones.ch/ontology/information-carrier#>.
@prefix publish: <http://e-editiones.ch/ontology/publishing#>.

@base <http://e-editiones.ch/ontology/document>.
@prefix document: <http://e-editiones.ch/ontology/document#>.

<http://e-editiones.ch/ontology/document>
	a owl:Ontology;
	dct:license <http://creativecommons.org/licenses/by/3.0/>;
	dct:title "An ontology about document"@en;
	dct:description """Formal description of document, general subclasses, related classes and properties."""@en;
	dct:creator "Hans Cools, MD, knowledge engineer, ontologist, software developer, University of Basel, Switzerland"@en;
	dct:contributor "Roberta Padlina, project coordinator and software developer, University of Basel, Switzerland"@en;
	dct:publisher "Universities of Basel, Bern, and Z체rich, Switzerland"@en;
	owl:versionInfo "2020-06-11"^^xsd:date.

#
# CLASSES
#

document:Document
	rdfs:isDefinedBy <http://e-editiones.ch/ontology/document#>;
	a rdfs:Class;
	rdfs:label "document"@en, "Dokument"@de;
	rdfs:comment """Identifiable, immaterial, contained information, e.g. a text, a graphic, an image, an audiogram, a videogram, abstracted from its information carrier."""@en;
	rdfs:subClassOf concept:Information, cidoc:E31_Document.

document:State
	rdfs:isDefinedBy <http://e-editiones.ch/ontology/document#>;
	a rdfs:Class;
	rdfs:label "document state"@en, "Zustand eines Dokumentes"@de;
	rdfs:comment """State of a document."""@en;
	rdfs:subClassOf event:State.

document:Set
	rdfs:isDefinedBy <http://e-editiones.ch/ontology/document#>;
	a rdfs:Class;
	rdfs:label "document set"@en, "Dokumentenreihe"@de;
	rdfs:comment """Set of documents."""@en;
	rdfs:subClassOf concept:Set.

document:Element
	rdfs:isDefinedBy <http://e-editiones.ch/ontology/document#>;
	a rdfs:Class;
	rdfs:label "document element"@en, "Dokumentelement"@de;
	rdfs:comment """Information as part of a document."""@en;
	rdfs:subClassOf concept:Information. #째 document:Document

document:Structure
	rdfs:isDefinedBy <http://e-editiones.ch/ontology/document#>;
	a rdfs:Class;
	rdfs:label "document structure"@en, "Dokumentstruktur"@de;
	rdfs:comment """Structural element of a document."""@en;
	rdfs:subClassOf document:Element.

document:Layout
	rdfs:isDefinedBy <http://e-editiones.ch/ontology/document#>;
	a rdfs:Class;
	rdfs:label "layout"@en, "Aufmachung"@de;
	rdfs:comment """Way in which the content of a page is set out."""@en;
	rdfs:subClassOf document:Element.

document:Space #째
	rdfs:isDefinedBy <http://e-editiones.ch/ontology/document#>;
	a rdfs:Class;
	rdfs:label "document space"@en, "Leerraum eines Dokumentes"@de;
	rdfs:comment """Empty space between document content structures, e.g. lines, columns, paragraphs, sections, strophes, images."""@en;
	rdfs:subClassOf document:Structure.

document:VerticalSpace
	rdfs:isDefinedBy <http://e-editiones.ch/ontology/document#>;
	a rdfs:Class;
	rdfs:label "vertical document space"@en, "vertikaler Leerraum eines Dokumentes"@de;
	rdfs:comment """Document space with vertical orientation, e.g. between columns."""@en;
	rdfs:subClassOf document:Space.

document:HorizontalSpace
	rdfs:isDefinedBy <http://e-editiones.ch/ontology/document#>;
	a rdfs:Class;
	rdfs:label "horizontal document space"@en, "horizontaler Leerraum eines Dokumentes"@de;
	rdfs:comment """Document space with horizontal orientation, e.g. between lines."""@en;
	rdfs:subClassOf document:Space.

#째 document:Reference

document:ContentStructure
	rdfs:isDefinedBy <http://e-editiones.ch/ontology/document#>;
	a rdfs:Class;
	rdfs:label "document content structure"@en, "Dokumentinhaltstruktur"@de;
	rdfs:comment """Content structure of a document."""@en;
	rdfs:subClassOf document:Structure.

document:ContentStructureIdentifier
	rdfs:isDefinedBy <http://e-editiones.ch/ontology/document#>;
	a rdfs:Class;
	rdfs:label "document content structure identifier"@en, "Dokumentinhaltstrukturidentifikator"@de;
	rdfs:comment """Identifier of a document content structure."""@en;
	rdfs:subClassOf document:Structure, concept:Identifier.

document:ContentStructureReference
	rdfs:isDefinedBy <http://e-editiones.ch/ontology/document#>;
	a rdfs:Class;
	rdfs:label "document content structure reference"@en, "Dokumentinhaltstrukturreferenz"@de;
	rdfs:comment """Reference as a document structure, referring from one document content structure to another via the identifier, e.g. a footnote reference from a text or image to the footnote identifier. The reference is linked to and has the same literal representation as the identifier of the content structure it refers to."""@en;
	rdfs:subClassOf document:Structure, concept:Identifier.

document:TextStructureReference
	rdfs:isDefinedBy <http://e-editiones.ch/ontology/document#>;
	a rdfs:Class;
	rdfs:label "text structure reference"@en, "Textstrukturreferenz"@de;
	rdfs:comment """Document content structure reference to a text structure, e.g. a footnote reference."""@en;
	rdfs:subClassOf document:ContentStructureReference.

document:FootnoteReference
	rdfs:isDefinedBy <http://e-editiones.ch/ontology/document#>;
	a rdfs:Class;
	rdfs:label "footnote reference"@en, "Fussnotereferenz"@de;
	rdfs:comment """Reference of a document content structure to a footnote via the footnote identifier."""@en;
	rdfs:subClassOf document:TextStructureReference.

document:EndnoteReference
	rdfs:isDefinedBy <http://e-editiones.ch/ontology/document#>;
	a rdfs:Class;
	rdfs:label "endnote reference"@en, "Endnotereferenz"@de;
	rdfs:comment """Reference of a document content structure to an endnote via the endnote identifier."""@en;
	rdfs:subClassOf document:TextStructureReference.

document:ExpressionReference
	rdfs:isDefinedBy <http://e-editiones.ch/ontology/document#>;
	a rdfs:Class;
	rdfs:label "document expression reference"@en, "Dokument-Expression-Referenz"@de;
	rdfs:comment """Document structure referring from a document content structure to a document expression identifier, e.g. a siglum."""@en;
	rdfs:subClassOf document:Structure, concept:Identifier.

document:Column
	rdfs:isDefinedBy <http://e-editiones.ch/ontology/document#>;
	a rdfs:Class;
	rdfs:label "column"@en, "Spalte"@de;
	rdfs:comment """Content structure displaying information, e.g. text lines and graphs, as a column as part of a page."""@en;
	rdfs:subClassOf document:ContentStructure.

document:Page
	rdfs:isDefinedBy <http://e-editiones.ch/ontology/document#>;
	a rdfs:Class;
	rdfs:label "document page"@en, "Dokumentseite"@de;
	rdfs:comment """Content structure with information, e.g. text lines and graphs, as a page as part of a document expression, on an information carrier page."""@en;
	rdfs:subClassOf document:ContentStructure.

document:PageIdentifier
	rdfs:isDefinedBy <http://e-editiones.ch/ontology/document#>;
	a rdfs:Class;
	rdfs:label "document page identifier"@en, "Dokumentseiteidentifikator"@de;
	rdfs:comment """Identifier of a document page."""@en;
	skos:note """The document page identifier is a reification."""@en;
	rdfs:subClassOf document:ContentStructureIdentifier.

document:PageOrdinalNumber
	rdfs:isDefinedBy <http://e-editiones.ch/ontology/document#>;
	a rdfs:Class;
	rdfs:label "document page ordinal number"@en, "Dokumentseiteordinalzahl"@de;
	rdfs:comment """Ordinal number of a document page."""@en;
	skos:note """The document page ordinal number is a reification."""@en;
	rdfs:subClassOf document:PageIdentifier, math:OrdinalNumber.

document:TitlePage
	rdfs:isDefinedBy <http://e-editiones.ch/ontology/document#>;
	a rdfs:Class;
	rdfs:label "title page"@en, "Titelblatt"@de;
	rdfs:comment """Document page contianing a title."""@en;
	rdfs:subClassOf document:Page.

document:Marginal
	rdfs:isDefinedBy <http://e-editiones.ch/ontology/document#>;
	a rdfs:Class;
	rdfs:label "marginal"@en, "Marginale"@de;
	rdfs:comment """Information besides a text in the margin of a carrier, e.g. a text, doodle, or illumination."""@en;
	rdfs:subClassOf document:ContentStructure.

document:Table
	rdfs:isDefinedBy <http://e-editiones.ch/ontology/document#>;
	a rdfs:Class;
	rdfs:label "table"@en, "Tabelle"@de;
	rdfs:comment """Two-dimensional structure composed of one or more fields or cell containing information and being part of a vertical column and a horizontal row, both with own identifier."""@en;
	rdfs:subClassOf document:ContentStructure.

document:Expression
	rdfs:isDefinedBy <http://e-editiones.ch/ontology/document#>;
	a rdfs:Class;
	rdfs:label "document expression"@en, "Dokument-Expression"@de;
	rdfs:comment """Document realisation of a work, based on FRBRoo, e.g. a text, story, poem, play, musical, song, joke, choreographic notation, movement pattern, sound pattern, image, multimedia object, or any combination of them, having an objectively recognisable structure."""@en;
	rdfs:subClassOf document:Document, frbroo:F2_Expression.

document:IndividualExpression
	rdfs:isDefinedBy <http://e-editiones.ch/ontology/document#>;
	a rdfs:Class;
	rdfs:label "individual document expression"@en, "individuelle Dokument-Expression"@de;
	rdfs:comment """Document realisation of an individual work."""@en;
	rdfs:subClassOf document:Expression, frbroo:F22_Self-Contained_Expression.

document:ExpressionPart
	rdfs:isDefinedBy <http://e-editiones.ch/ontology/document#>;
	a rdfs:Class;
	rdfs:label "document expression part"@en, "Dokument-Expressionsteil"@de;
	rdfs:comment """Part of an individual document expression, considered as incomplete."""@en;
	rdfs:subClassOf document:Expression, frbroo:F23_Expression_Fragment.

document:Draft
	rdfs:isDefinedBy <http://e-editiones.ch/ontology/document#>;
	a rdfs:Class;
	rdfs:label "document draft"@en, "Dokumententwurf"@de;
	rdfs:comment """Developmental document expression, subject to future modification, not having all envisioned features."""@en;
	rdfs:subClassOf document:Expression, creating:UnfinishedCreation.

document:PolyAuthorExpression
	rdfs:isDefinedBy <http://e-editiones.ch/ontology/document#>;
	a rdfs:Class;
	rdfs:label "poly-author document expression"@en, "Mehrautorentextdokument-Expression"@de;
	rdfs:comment """Document expression by different authors."""@en;
	rdfs:subClassOf document:Expression.

document:ExpressionIdentifier
	rdfs:isDefinedBy <http://e-editiones.ch/ontology/document#>;
	a rdfs:Class;
	rdfs:label "document expression identifier"@en, "Dokument-Expressionsidentifikator"@de;
	rdfs:comment """Identifier of a document expression."""@en;
	rdfs:subClassOf document:Structure, concept:Identifier.

document:BibliographicReference
	rdfs:isDefinedBy <http://e-editiones.ch/ontology/document#>;
	a rdfs:Class;
	rdfs:label "bibliographic reference"@en, "bibliographische Referenz"@de, "r챕f챕rence bibliographique"@fr, "riferimenti bibliografici"@it;
	rdfs:comment """All information, structured along certain composition rules, to identify a resource in any format (print, audiovisual, digital, etc.), published or unpublished. Used for example to refer from a part in a text expression to a part in another text expression. """@en;
	skos:note """There is not 1 canonical way to write a bibliographic reference"""@en;
	rdfs:seeAlso <https://products.abc-clio.com/ODLIS/odlis_b.aspx>;
	rdfs:subClassOf text-structure:ContentStructure.

document:CitationBibliographicReference
	rdfs:isDefinedBy <http://e-editiones.ch/ontology/document#>;
	a rdfs:Class;
	rdfs:label "citation bibliographic reference"@en, "bibliographische Referenz eines Zitats"@de; # , "r챕f챕rence bibliographique"@fr, "riferimenti bibliografici"@it;
	rdfs:comment """All information, structured along certain composition rules, to identify a text expression part as citation of a part of another text expression, the latter being published or not. """@en;
	skos:note """There is not 1 canonical way to write a citation bibliographic reference"""@en;
	rdfs:subClassOf text-structure:ContentStructure.

#째 document:Witness

document:CompleteWorks
	rdfs:isDefinedBy <http://e-editiones.ch/ontology/document#>;
	a rdfs:Class;
	rdfs:label "complete works"@en, "Gesamtwerk"@de;
	rdfs:comment """Set of individual document expressions of one author."""@en;
	rdfs:subClassOf document:Set.

document:Cycle
	rdfs:isDefinedBy <http://e-editiones.ch/ontology/document#>;
	a rdfs:Class;
	rdfs:label "expression cycle"@en, "Expression-Zyklus"@de;
	rdfs:comment """Set of individual document expressions belonging together, usually created around a certain theme, and intended to be experienced in a certain sequence."""@en;
	rdfs:subClassOf document:Set.

document:Catalogue
	rdfs:isDefinedBy <http://e-editiones.ch/ontology/document#>;
	a rdfs:Class;
	rdfs:label "catalogue"@en, "Katalog"@de, "catalogue"@fr;
	rdfs:comment """List of descriptions of things, mostly ordered, e.g. alphabetically; e.g. library's book catalogue, exhibition's works of art catalogue, mail-order company's items for sale catalogue."""@en;
	rdfs:subClassOf document:IndividualExpression.

document:Encoder
	rdfs:isDefinedBy <http://e-editiones.ch/ontology/document#>;
	a rdfs:Class;
	rdfs:label "encoder"@en, "KodiererIn"@de, "codeur"@fr, "codificatore"@it;
	rdfs:comment """Role of a person converting a document into code, e.g. from text to XML."""@en;
	rdfs:subClassOf creating:PersonCreator.

document:Code
	rdfs:isDefinedBy <http://e-editiones.ch/ontology/document#>;
	a rdfs:Class;
	rdfs:label "code document"@en,"Kode-Dokument"@de;
	rdfs:comment """Information as code, e.g. in any programming language."""@en;
	rdfs:subClassOf concept:Information.

document:HypertextDocument
	rdfs:isDefinedBy <http://e-editiones.ch/ontology/document#>;
	a rdfs:Class;
	rdfs:label "hypertext document"@en,"Hypertext-Dokument"@de;
	rdfs:comment """Document written in Hypertext Markup Language (HTML)."""@en;
	rdfs:subClassOf document:Code.

document:HypertextElement
	rdfs:isDefinedBy <http://e-editiones.ch/ontology/document#>;
	a rdfs:Class;
	rdfs:label "hypertext document element"@en, "Hypertext-Dokumentelement"@de;
	rdfs:comment """Information as part of a hypertext document."""@en;
	rdfs:subClassOf document:Element.

document:HypertextStructure
	rdfs:isDefinedBy <http://e-editiones.ch/ontology/document#>;
	a rdfs:Class;
	rdfs:label "hypertext document structure"@en, "Hypertext-Dokumentstruktur"@de;
	rdfs:comment """Structural element of a hypertext document."""@en;
	rdfs:subClassOf document:HypertextElement, document:Structure.

document:HypertextPage
	rdfs:isDefinedBy <http://e-editiones.ch/ontology/document#>;
	a rdfs:Class;
	rdfs:label "hypertext document page"@en, "Hypertext-Dokumentseite"@de;
	rdfs:comment """Page of a hypertext document."""@en;
	rdfs:subClassOf document:Page, document:HypertextStructure.

document:HypertextStartPage
	rdfs:isDefinedBy <http://e-editiones.ch/ontology/document#>;
	a rdfs:Class;
	rdfs:label "hypertext document start page"@en, "Hypertext-Dokumentstartseite"@de;
	rdfs:comment """Start page of a hypertext document."""@en;
	rdfs:subClassOf document:HypertextPage.

#
# DATATYPE INSTANCES
#

document:css
	rdfs:isDefinedBy <http://e-editiones.ch/ontology/document#>;
	a rdfs:Class, rdfs:Datatype;
	rdfs:label "CSS-datatype"@en;
	rdfs:comment """Datatype to type a literal expressed in the Cascading Style Sheets-language (CSS)."""@en;
	skos:note """Example: "color: #000000;"^^document:css"""@en.

#
# PROPERTIES
#

document:hasContentLiteral
	rdfs:isDefinedBy <http://e-editiones.ch/ontology/document#>;
	a owl:ObjectProperty;
	rdfs:label "document has content literal"@en, "Dokument hat Inhaltliterale"@de;
	rdfs:comment """Relating a document to its content literal."""@en;
	skos:note """Includes a code literal of a programming language, e.g. HTML."""@en;
	rdfs:domain document:Document;
	rdfs:range rdfs:Literal.

document:hasState
	rdfs:isDefinedBy <http://e-editiones.ch/ontology/document#>;
	a owl:ObjectProperty;
	rdfs:label "document has state"@en, "Dokument hat Zustand"@de;
	rdfs:comment """Relating a document to its state."""@en;
	rdfs:domain document:Document;
	rdfs:range document:State.

document:isElementOfDocument
	rdfs:isDefinedBy <http://e-editiones.ch/ontology/document#>;
	a owl:ObjectProperty;
	rdfs:label "is element of document"@en, "ist Element eines Dokumentes"@de;
	rdfs:comment """Relating a document element to a document it is part of."""@en;
	rdfs:domain document:Element;
	rdfs:range document:Document;
	rdfs:subPropertyOf concept:isPartOf.

document:isStructureOfDocument
	rdfs:isDefinedBy <http://e-editiones.ch/ontology/document#>;
	a owl:ObjectProperty;
	rdfs:label "is structure of document"@en, "ist Struktur eines Dokumentes"@de;
	rdfs:comment """Relating a document structure to a document it is part of."""@en;
	rdfs:domain document:Structure;
	rdfs:range document:Document;
	rdfs:subPropertyOf document:isElementOfDocument.

document:isSpaceOfDocument
	rdfs:isDefinedBy <http://e-editiones.ch/ontology/document#>;
	a owl:ObjectProperty;
	rdfs:label "is space of document"@en, "ist Leerraum eines Dokumentes"@de;
	rdfs:comment """Relating a space to the document it is part of."""@en;
	rdfs:domain document:Space;
	rdfs:range document:Document;
	rdfs:subPropertyOf document:isStructureOfDocument.

document:contentStructureHasIdentifier
	rdfs:isDefinedBy <http://e-editiones.ch/ontology/document#>;
	a owl:ObjectProperty;
	rdfs:label "document content structure has identifier"@en, "Dokumentinhaltstruktur hat Identifikator"@de;
	rdfs:comment """Relating a document content structure to its identifier."""@en;
	rdfs:domain document:ContentStructure;
	rdfs:range document:ContentStructureIdentifier;
	rdfs:subPropertyOf concept:hasIdentifier.

document:contentStructureHasReference
	rdfs:isDefinedBy <http://e-editiones.ch/ontology/document#>;
	a owl:ObjectProperty;
	rdfs:label "document content structure has reference"@en, "Dokumentinhaltstruktur hat Referenz"@de;
	rdfs:comment """Relating a document content structure to a reference it has."""@en;
	rdfs:domain document:ContentStructure;
	rdfs:range document:ContentStructureReference.

document:contentStructureHasTextReference
	rdfs:isDefinedBy <http://e-editiones.ch/ontology/document#>;
	a owl:ObjectProperty;
	rdfs:label "document content structure has text reference"@en, "Dokumentinhaltstruktur hat Textreferenz"@de;
	rdfs:comment """Relating a document content structure to a text reference it has."""@en;
	rdfs:domain document:ContentStructure;
	rdfs:range document:TextStructureReference;
	rdfs:subPropertyOf document:contentStructureHasReference.

document:contentStructureHasFootnoteReference
	rdfs:isDefinedBy <http://e-editiones.ch/ontology/document#>;
	a owl:ObjectProperty;
	rdfs:label "document content structure has footnote reference"@en, "Dokumentinhaltstruktur hat Fussnotereferenz"@de;
	rdfs:comment """Relating a document content structure to a footnote reference it has."""@en;
	rdfs:domain document:ContentStructure;
	rdfs:range document:FootnoteReference;
	rdfs:subPropertyOf document:contentStructureHasTextReference.

document:contentStructureHasEndnote
	rdfs:isDefinedBy <http://e-editiones.ch/ontology/document#>;
	a owl:ObjectProperty;
	rdfs:label "document content structure has endnote"@en, "Dokumentinhaltstruktur hat Endnote"@de;
	rdfs:comment """Relating a document content structure to an endnote it has."""@en;
	rdfs:domain document:ContentStructure;
	rdfs:range document:Endnote;
	owl:propertyChainAxiom (document:contentStructureHasEndnoteReference document:endnoteReferenceHasIdentifier note-structure:isIdentifierOfEndnote).

document:contentStructureHasEndnoteReference
	rdfs:isDefinedBy <http://e-editiones.ch/ontology/document#>;
	a owl:ObjectProperty;
	rdfs:label "document content structure has endnote reference"@en, "Dokumentinhaltstruktur hat Endnotereferenz"@de;
	rdfs:comment """Relating a document content structure to an endnote reference it has."""@en;
	rdfs:domain document:ContentStructure;
	rdfs:range document:EndnoteReference;
	rdfs:subPropertyOf document:contentStructureHasTextReference.

document:contentStructureHasExpressionReference
	rdfs:isDefinedBy <http://e-editiones.ch/ontology/document#>;
	a owl:ObjectProperty;
	rdfs:label "document content structure has expression reference"@en, "Dokumentinhaltstruktur hat Expression-Referenz"@de;
	rdfs:comment """Relating a document content structure to an expression reference it has."""@en;
	rdfs:domain document:ContentStructure;
	rdfs:range document:ExpressionReference.

document:contentStructureReferenceHasContentStructureIdentifier
	rdfs:isDefinedBy <http://e-editiones.ch/ontology/document#>;
	a owl:ObjectProperty;
	rdfs:label "document content structure reference has document content structure identifier"@en, "Dokumentinhaltstrukturreferenz hat Dokumentinhaltstrukturidentifikator"@de;
	rdfs:comment """Relating the reference of a document content structure to another document content structure, to the identifier of the latter."""@en;
	rdfs:domain document:ContentStructureReference;
	rdfs:range document:ContentStructureIdentifier.

document:textStructureReferenceHasTextStructureIdentifier
	rdfs:isDefinedBy <http://e-editiones.ch/ontology/document#>;
	a owl:ObjectProperty;
	rdfs:label "text structure reference has text structure identifier"@en, "Textstrukturreferenz hat Textstrukturidentifikator"@de;
	rdfs:comment """Relating a text structure reference of a document content structure to the identifier of the text structure. E.g. a document content structure has a footnote reference linked to the identifier of the footnote."""@en;
	rdfs:domain document:TextStructureReference;
	rdfs:range text-structure:Identifier;
	rdfs:subPropertyOf document:contentStructureReferenceHasContentStructureIdentifier.

document:footnoteReferenceHasFootnoteIdentifier
	rdfs:isDefinedBy <http://e-editiones.ch/ontology/document#>;
	a owl:ObjectProperty;
	rdfs:label "footnote reference has footnote identifier"@en, "Fussnotereferenz hat Fussnoteidentifikator"@de;
	rdfs:comment """Relating a footnote reference of a document content structure to the identifier of the footnote."""@en;
	rdfs:domain document:FootnoteReference;
	rdfs:range note-structure:FootnoteIdentifier;
	rdfs:subPropertyOf document:textStructureReferenceHasTextStructureIdentifier.

document:footnoteReferenceHasFootnoteNumber
	rdfs:isDefinedBy <http://e-editiones.ch/ontology/document#>;
	a owl:ObjectProperty;
	rdfs:label "footnote reference has footnote number"@en, "Fussnotereferenz hat Fussnotenummer"@de;
	rdfs:comment """Relating a footnote reference of a document content structure to the number of the footnote."""@en;
	rdfs:domain document:FootnoteReference;
	rdfs:range note-structure:FootnoteNumber;
	rdfs:subPropertyOf document:footnoteReferenceHasFootnoteIdentifier.

document:endnoteReferenceHasEndnoteIdentifier
	rdfs:isDefinedBy <http://e-editiones.ch/ontology/document#>;
	a owl:ObjectProperty;
	rdfs:label "endnote reference has endnote identifier"@en, "Endnotereferenz hat Endnoteidentifikator"@de;
	rdfs:comment """Relating an endnote reference of a document content structure to the identifier of the endnote."""@en;
	rdfs:domain document:EndnoteReference;
	rdfs:range note-structure:EndnoteIdentifier;
	rdfs:subPropertyOf document:textStructureReferenceHasTextStructureIdentifier.

document:endnoteReferenceHasEndnoteNumber
	rdfs:isDefinedBy <http://e-editiones.ch/ontology/document#>;
	a owl:ObjectProperty;
	rdfs:label "endnote reference has endnote number"@en, "Endnotereferenz hat Endnotenummer"@de;
	rdfs:comment """Relating an endnote reference of a document content structure to the number of the endnote."""@en;
	rdfs:domain document:EndnoteReference;
	rdfs:range note-structure:EndnoteNumber;
	rdfs:subPropertyOf document:endnoteReferenceHasEndnoteIdentifier.

document:isColumnOfPage
	rdfs:isDefinedBy <http://e-editiones.ch/ontology/document#>;
	a owl:ObjectProperty;
	rdfs:label "is column of document page"@en, "ist Spalte einer Dokumentseite"@de;
	rdfs:comment """Relating a column to a document page it is part of."""@en;
	rdfs:domain document:Column;
	rdfs:range document:Page;
	rdfs:subPropertyOf concept:isPartOf.

document:isPageOfExpression
	rdfs:isDefinedBy <http://e-editiones.ch/ontology/document#>;
	a owl:ObjectProperty;
	rdfs:label "is page of document expression"@en, "ist Seite einer Dokumentexpression"@de;
	rdfs:comment """Relating a document page to a document expression it is part of."""@en;
	rdfs:domain document:Page;
	rdfs:range document:Expression;
	rdfs:subPropertyOf concept:isPartOf.

document:pageHasIdentifier
	rdfs:isDefinedBy <http://e-editiones.ch/ontology/document#>;
	a owl:ObjectProperty;
	rdfs:label "document page has identifier"@en, "Dokumentseite hat Identifikator"@de;
	rdfs:comment """Relating a document page to its identifier."""@en;
	rdfs:domain document:Page;
	rdfs:range document:PageIdentifier;
	rdfs:subPropertyOf document:contentStructureHasIdentifier.

document:pageHasOrdinalNumber
	rdfs:isDefinedBy <http://e-editiones.ch/ontology/document#>;
	a owl:ObjectProperty;
	rdfs:label "document page has ordinal number"@en, "Dokumentseite hat Ordinalzahl"@de;
	rdfs:comment """Relating a document page to its ordinal number."""@en;
	rdfs:domain document:Page;
	rdfs:range document:PageOrdinalNumber;
	rdfs:subPropertyOf document:pageHasIdentifier.

document:pageHasOrdinalNumeral
	rdfs:isDefinedBy <http://e-editiones.ch/ontology/document#>;
	a owl:DatatypeProperty;
	rdfs:label "page has ordinal numeral"@en, "Seite hat Ordinalnumerale"@de;
	rdfs:comment """Relating a page to its ordinal numeral."""@en;
	rdfs:domain document:Page;
	rdfs:range xsd:nonNegativeInteger;
	rdfs:subPropertyOf math:hasOrdinalNumeral;
	owl:propertyChainAxiom (document:pageHasOrdinalNumber math:hasNumeral).

document:isTableOfColumn
	rdfs:isDefinedBy <http://e-editiones.ch/ontology/document#>;
	a owl:ObjectProperty;
	rdfs:label "is table of column"@en, "ist Tabelle einer Spalte"@de;
	rdfs:comment """Relating a table to a column it is part of."""@en;
	rdfs:domain document:Table;
	rdfs:range document:Column;
	rdfs:subPropertyOf concept:isPartOf.

document:expressionHasIdentifier
	rdfs:isDefinedBy <http://e-editiones.ch/ontology/document#>;
	a owl:ObjectProperty;
	rdfs:label "expression has identifier"@en, "Expression hat Identifikator"@de;
	rdfs:comment """Relating a document expression to its identifier."""@en;
	rdfs:domain document:Expression;
	rdfs:range document:ExpressionIdentifier;
	rdfs:subPropertyOf concept:hasIdentifier.

document:expressionHasTitleLiteral
	rdfs:isDefinedBy <http://e-editiones.ch/ontology/document#>;
	a owl:DatatypeProperty;
	rdfs:label "expression has title literal"@en, "Expression hat Titelliterale"@de;
	rdfs:comment """Relating an expression to its title literal."""@en;
	rdfs:domain document:Expression;
	rdfs:range rdfs:Literal;
	rdfs:subPropertyOf text:hasTitleLiteral.

document:expressionHasSubtitleLiteral
	rdfs:isDefinedBy <http://e-editiones.ch/ontology/document#>;
	a owl:DatatypeProperty;
	rdfs:label "expression has subtitle literal"@en, "Expression hat Untertitelliterale"@de;
	rdfs:comment """Relating an expression to a subtitle literal it has."""@en;
	rdfs:domain document:Expression;
	rdfs:range rdfs:Literal;
	rdfs:subPropertyOf text:hasSubtitleLiteral.

document:isExpressionOfCycle
	rdfs:isDefinedBy <http://e-editiones.ch/ontology/document#>;
	a owl:ObjectProperty;
	rdfs:label "is expression of cycle"@en, "ist Expression eines Zyklus"@de;
	rdfs:comment """Relating an individual expression to a cycle it is part of."""@en;
	rdfs:domain document:IndividualExpression;
	rdfs:range document:Cycle;
	rdfs:subPropertyOf concept:isPartOf.

document:isPartOfIndividualExpression
	rdfs:isDefinedBy <http://e-editiones.ch/ontology/document#>;
	a owl:ObjectProperty;
	rdfs:label "is part of individual expression"@en, "ist Teil einer individuellen Expression"@de;
	rdfs:comment """Relating an expression part to an individual expression it is part of."""@en;
	rdfs:domain document:ExpressionPart;
	rdfs:range document:IndividualExpression;
	rdfs:subPropertyOf concept:isPartOf.

document:expressionReferenceHasIdentifier
	rdfs:isDefinedBy <http://e-editiones.ch/ontology/document#>;
	a owl:ObjectProperty;
	rdfs:label "expression reference has identifier"@en, "Expression-Referenz hat Identifikator"@de;
	rdfs:comment """Relating a document expression reference to its identifier."""@en;
	rdfs:domain document:ExpressionReference;
	rdfs:range document:ExpressionIdentifier;
	rdfs:subPropertyOf concept:hasIdentifier.

document:hasBibliographicReference
	rdfs:isDefinedBy <http://e-editiones.ch/ontology/document#>;
	a owl:ObjectProperty;
	rdfs:label "has bibliographic reference"@en, "hat bibliographische Referenz"@de, "a une r챕f챕rence bibliographique"@fr, "ha riferimenti bibliografici"@it;
	rdfs:comment """Relating a document expression to a bibliographic reference it has."""@en;
	rdfs:domain document:Expression;
	rdfs:range document:BibliographicReference;
	rdfs:subPropertyOf concept:hasSymbolicEntity.

document:bibliographicReferenceHasLiteral
	rdfs:isDefinedBy <http://e-editiones.ch/ontology/document#>;
	a owl:DatatypeProperty;
	rdfs:label "bibliographic reference has literal"@en, "bibliographische Referenz hat Literale"@de, "r챕f챕rence bibliographique a un litt챕ral"@fr, "riferimento bibliografico ha un letterale"@it;
	rdfs:comment """Relating a bibliographic reference to its literal."""@en;
	rdfs:domain document:BibliographicReference;
	rdfs:range rdfs:Literal;
	rdfs:subPropertyOf concept:symbolicEntityHasLiteral.

document:hasBibliographicReferenceLiteral
	rdfs:isDefinedBy <http://e-editiones.ch/ontology/document#>;
	a owl:DatatypeProperty;
	rdfs:label "has bibliographic reference literal"@en, "hat bibliographische Referenzliterale"@de, "a un litt챕ral de r챕f챕rence bibliographique"@fr, "ha riferimenti bibliografici letterali"@it;
	rdfs:comment """Relating a document expression to the literal of a bibliographic reference it has."""@en;
	rdfs:domain document:Expression;
	rdfs:range rdfs:Literal;
	rdfs:subPropertyOf concept:hasLiteral;
	owl:propertyChainAxiom (document:hasBibliographicReference document:bibliographicReferenceHasLiteral).

document:hasCitationBibliographicReference
	rdfs:isDefinedBy <http://e-editiones.ch/ontology/document#>;
	a owl:ObjectProperty;
	rdfs:label "has citation bibliographic reference"@en, "hat bibliographische Referenz eines Zitats"@de; # , "a une r챕f챕rence bibliographique"@fr, "ha riferimenti bibliografici"@it;
	rdfs:comment """Relating a text expression to a bibliographic reference of a citation thereof."""@en;
	rdfs:domain text-expression:Expression;
	rdfs:range document:CitationBibliographicReference;
	rdfs:subPropertyOf concept:hasSymbolicEntity.

document:citationBibliographicReferenceHasLiteral
	rdfs:isDefinedBy <http://e-editiones.ch/ontology/document#>;
	a owl:DatatypeProperty;
	rdfs:label "citation bibliographic reference has literal"@en, "bibliographische Referenz eines Zitats hat Literal"@de; #, "r챕f챕rence bibliographique a un litt챕ral"@fr, "riferimento bibliografico ha un letterale"@it;
	rdfs:comment """Relating a citation bibliographic reference to its literal."""@en;
	rdfs:domain document:CitationBibliographicReference;
	rdfs:range rdfs:Literal;
	rdfs:subPropertyOf concept:symbolicEntityHasLiteral.

document:hasCitationBibliographicReferenceLiteral
	rdfs:isDefinedBy <http://e-editiones.ch/ontology/document#>;
	a owl:DatatypeProperty;
	rdfs:label "has citation bibliographic reference literal"@en, "hat bibliographische Referenzliterale eines Zitats"@de; # , "a un litt챕ral de r챕f챕rence bibliographique"@fr, "ha riferimenti bibliografici letterali"@it;
	rdfs:comment """Relating a text expression to the literal of a bibliographic reference of a citation thereof."""@en;
	rdfs:domain text-expression:Expression;
	rdfs:range rdfs:Literal;
	rdfs:subPropertyOf concept:hasLiteral.

