@prefix rdfs: <http://www.w3.org/2000/01/rdf-schema#>.
@prefix owl: <http://www.w3.org/2002/07/owl#>.
@prefix xsd: <http://www.w3.org/2001/XMLSchema#>.
@prefix skos: <http://www.w3.org/2004/02/skos/core#>.
@prefix dct: <http://purl.org/dc/terms/>.
@prefix foaf: <http://xmlns.com/foaf/0.1/>.
@prefix cidoc: <http://www.cidoc-crm.org/cidoc-crm/>.
@prefix physical-entity: <http://e-editiones.ch/ontology/physical-entity#>.
@prefix human: <http://e-editiones.ch/ontology/human#>.
@prefix concept: <http://e-editiones.ch/ontology/concept#>.
@prefix mathematics: <http://e-editiones.ch/ontology/mathematics#>.
@prefix organization: <http://e-editiones.ch/ontology/organization#>.
@prefix text: <http://e-editiones.ch/ontology/text#>.

@base <http://e-editiones.ch/ontology/human-geography>.
@prefix human-geography: <http://e-editiones.ch/ontology/human-geography#>.

<http://e-editiones.ch/ontology/human-geography>
	a owl:Ontology;
	dct:license <http://creativecommons.org/licenses/by/3.0/>;
	dct:title """Human Geography"""@en;
	dct:description """Formal description of human geography, general subclasses, related classes, and properties."""@en;
	dct:creator "Hans Cools, MD, knowledge engineer, ontologist, software developer, NIE-INE, University of Basel, Switzerland"@en;
	dct:contributor "Rebekka Plüss, research assistant and software developer, University of Basel, Switzerland"@en;
	dct:publisher "Universities of Basel, Bern, and Zürich, Switzerland"@en;
	owl:versionInfo "2020-06-11"^^xsd:date.

#
# CLASSES
#

human-geography:Nation
	rdfs:isDefinedBy <http://e-editiones.ch/ontology/human-geography#>;
	a rdfs:Class;
	rdfs:label "nation"@en, "Nation"@de;
	rdfs:comment """Stable political organization with a commonality e.g. ethnicity, language, culture, ."""@en;
	rdfs:subClassOf organization:PoliticalOrganization.

human-geography:Country
	rdfs:isDefinedBy <http://e-editiones.ch/ontology/human-geography#>;
	a rdfs:Class;
	rdfs:label "country"@en, "Land"@de;
	rdfs:comment """Place of a nation."""@en;
	rdfs:subClassOf physical-entity:EarthPlace.

human-geography:State
	rdfs:isDefinedBy <http://e-editiones.ch/ontology/human-geography#>;
	a rdfs:Class;
	rdfs:label "state"@en, "Staat"@de;
	rdfs:comment """Political organization with an own government."""@en;
	rdfs:subClassOf organization:PoliticalOrganization.

human-geography:NationState
	rdfs:isDefinedBy <http://e-editiones.ch/ontology/human-geography#>;
	a rdfs:Class;
	rdfs:label "nation state"@en, "Nationalstaat"@de;
	rdfs:comment """Political organization of a nation with an own government."""@en;
	rdfs:subClassOf human-geography:State.

human-geography:SovereignState
	rdfs:isDefinedBy <http://e-editiones.ch/ontology/human-geography#>;
	a rdfs:Class;
	rdfs:label "sovereign state"@en, "Souveränstaat"@de;
	rdfs:comment """Political organization of a sovereign state with an own government."""@en;
	rdfs:subClassOf human-geography:State.

human-geography:FederalState
	rdfs:isDefinedBy <http://e-editiones.ch/ontology/human-geography#>;
	a rdfs:Class;
	rdfs:label "federal state"@en, "Bundesstaat"@de;
	rdfs:comment """Political organization of a federal state with an own government."""@en;
	rdfs:subClassOf human-geography:State.

human-geography:Government
	rdfs:isDefinedBy <http://e-editiones.ch/ontology/human-geography#>;
	a rdfs:Class;
	rdfs:label "government"@en, "Regierung"@de;
	rdfs:comment """One or more persons in a politician role exercising authority over a particular territory."""@en;
	rdfs:subClassOf organization:PoliticalOrganization.

human-geography:Monarchy
	rdfs:isDefinedBy <http://e-editiones.ch/ontology/human-geography#>;
	a rdfs:Class;
	rdfs:label "monarchy"@en, "Monarchie"@de;
	rdfs:comment """State wherein one person or family governs."""@en;
	rdfs:subClassOf human-geography:State.

human-geography:Monarch
	rdfs:isDefinedBy <http://e-editiones.ch/ontology/human-geography#>;
	a rdfs:Class;
	rdfs:label "monarch"@en, "Monarch"@de, "monarque"@fr;
	rdfs:comment """Role of a person being a sovereign head of state in a monarchy."""@en;
	rdfs:subClassOf human:PersonRole.

human-geography:King
	rdfs:isDefinedBy <http://e-editiones.ch/ontology/human-geography#>;
	a rdfs:Class;
	rdfs:label "king"@en, "König"@de, "roi"@fr;
	rdfs:comment """Role of a man being the absolute ruler in a monarchy or husband of a woman being the absolute ruler in a monarchy."""@en;
	rdfs:subClassOf human:Monarch.

human-geography:Queen
	rdfs:isDefinedBy <http://e-editiones.ch/ontology/human-geography#>;
	a rdfs:Class;
	rdfs:label "queen"@en, "Königin"@de, "reine"@fr;
	rdfs:comment """Role of a woman being the absolute ruler in a monarchy or wife of a man being the absolute ruler in a monarchy."""@en;
	rdfs:subClassOf human:Monarch.

human-geography:Empire
	rdfs:isDefinedBy <http://e-editiones.ch/ontology/human-geography#>;
	a rdfs:Class;
	rdfs:label "empire"@en, "Imperium"@de;
	rdfs:comment """Group of nations with an overarching government."""@en;
	rdfs:subClassOf organization:PoliticalOrganization.

human-geography:Emperor
	rdfs:isDefinedBy <http://e-editiones.ch/ontology/human-geography#>;
	a rdfs:Class;
	rdfs:label "emperor"@en, "Kaiser"@de, "empereur"@fr;
	rdfs:comment """Role of a man being a sovereign head of an empire or husband of a woman being a sovereign head of an empire."""@en;
	rdfs:subClassOf human:PersonRole.

human-geography:Empress
	rdfs:isDefinedBy <http://e-editiones.ch/ontology/human-geography#>;
	a rdfs:Class;
	rdfs:label "empress"@en, "Kaiserin"@de, "impératrice"@fr;
	rdfs:comment """Role of a woman being a sovereign head of an empire or wife of a man being a sovereign head of an empire."""@en;
	rdfs:subClassOf human:PersonRole.

human-geography:Town
	rdfs:isDefinedBy <http://e-editiones.ch/ontology/human-geography#>;
	a rdfs:Class;
	rdfs:label "town"@en, "Ortschaft"@de;
	rdfs:comment """Smallest place with political boundaries and an own government."""@en;
	rdfs:subClassOf physical-entity:EarthPlace.

human-geography:Village
	rdfs:isDefinedBy <http://e-editiones.ch/ontology/human-geography#>;
	a rdfs:Class;
	rdfs:label "village"@en, "Dorf"@de;
	rdfs:comment """Small place with political boundaries but without an own government."""@en;
	rdfs:subClassOf physical-entity:EarthPlace.

human-geography:City
	rdfs:isDefinedBy <http://e-editiones.ch/ontology/human-geography#>;
	a rdfs:Class;
	rdfs:label "city"@en, "Stadt"@de;
	rdfs:comment """Large town."""@en;
	rdfs:subClassOf physical-entity:EarthPlace.

human-geography:District
	rdfs:isDefinedBy <http://e-editiones.ch/ontology/human-geography#>;
	a rdfs:Class;
	rdfs:label "district"@en, "Stadtviertel"@de;
	rdfs:comment """Part of a city with own administration."""@en;
	rdfs:subClassOf physical-entity:EarthPlace.

human-geography:Street
	rdfs:isDefinedBy <http://e-editiones.ch/ontology/human-geography#>;
	a rdfs:Class;
	rdfs:label "street"@en, "Strasse"@de;
	rdfs:comment """."""@en;
	rdfs:subClassOf physical-entity:EarthPlace.

human-geography:StreetPlace
	rdfs:isDefinedBy <http://e-editiones.ch/ontology/human-geography#>;
	a rdfs:Class;
	rdfs:label "street place"@en, "Strassenort"@de;
	rdfs:comment """."""@en;
	rdfs:subClassOf physical-entity:EarthPlace.

human-geography:PostalAddress #° more general? # comprises cidoc:E45_Address and cidoc:E51_Contact_Point: postal box
	rdfs:isDefinedBy <http://e-editiones.ch/ontology/human-geography#>;
	a rdfs:Class;
	rdfs:label "postal address"@en, "Postanschrift"@de;
	rdfs:comment """."""@en;
	rdfs:subClassOf concept:SymbolicEntity.

# domicile

#
# PROPERTIES
#

human-geography:hasDomicile
	rdfs:isDefinedBy <http://e-editiones.ch/ontology/human-geography#>;
	a owl:ObjectProperty;
	rdfs:label "has domicile"@en, "hat Sitz"@de;
	rdfs:comment """Relating a human agent - person or group - to a place of registered staying and contactability."""@en;
	rdfs:domain human:Agent;
	rdfs:range physical-entity:Place;
	rdfs:subPropertyOf physical-entity:hasLocation.

human-geography:hasPostalAddress
	rdfs:isDefinedBy <http://e-editiones.ch/ontology/human-geography#>;
	a owl:ObjectProperty;
	rdfs:label "has postal address"@en, "hat Postanschrift"@de;
	rdfs:comment """Relating someone or something to her/his/its postal address."""@en;
	rdfs:domain rdfs:Resource;
	rdfs:range human-geography:PostalAddress.

human-geography:hasReceiverPostalAddress
	rdfs:isDefinedBy <http://e-editiones.ch/ontology/human-geography#>;
	a owl:ObjectProperty;
	rdfs:label "has receiver postal address"@en, "hat Empfängerpostanschrift"@de;
	rdfs:comment """Relating something being sent to the postal address of the receiver."""@en;
	rdfs:domain physical-entity:Matter;
	rdfs:range human-geography:PostalAddress.

human-geography:hasReturnPostalAddress
	rdfs:isDefinedBy <http://e-editiones.ch/ontology/human-geography#>;
	a owl:ObjectProperty;
	rdfs:label "has return postal address"@en, "hat Absenderpostanschrift"@de;
	rdfs:comment """Relating something being sent to the postal address for return."""@en;
	rdfs:domain physical-entity:Matter;
	rdfs:range human-geography:PostalAddress.

human-geography:addressHasAddresseeNameLiteral
	rdfs:isDefinedBy <http://e-editiones.ch/ontology/human-geography#>;
	a owl:DatatypeProperty;
	rdfs:label "postal address has addressee name literal"@en, "Postanschrift hat Namenliteral des Adressats"@de;
	rdfs:comment """Relating a postal address to an addressee name literal."""@en;
	rdfs:domain human-geography:PostalAddress;
	rdfs:range rdfs:Literal;
	rdfs:subPropertyOf text:hasNameLiteral.

human-geography:addressHasStreetNameLiteral
	rdfs:isDefinedBy <http://e-editiones.ch/ontology/human-geography#>;
	a owl:DatatypeProperty;
	rdfs:label "postal address has street name literal"@en, "Postanschrift hat Strassennamenliteral"@de;
	rdfs:comment """Relating a postal address to the name literal of the street."""@en;
	rdfs:domain human-geography:PostalAddress;
	rdfs:range rdfs:Literal;
	rdfs:subPropertyOf text:hasNameLiteral.

human-geography:addressHasHouseNumberNumeral
	rdfs:isDefinedBy <http://e-editiones.ch/ontology/human-geography#>;
	a owl:DatatypeProperty;
	rdfs:label "postal address has house number numeral"@en, "Postanschrift hat Hausnummernumeral"@de;
	rdfs:comment """Relating a postal address to the nummer numeral of the house."""@en;
	rdfs:domain human-geography:PostalAddress;
	rdfs:range xsd:positiveInteger;
	rdfs:subPropertyOf mathematics:hasOrdinalNumeral.

human-geography:addressHasPostcodeValue
	rdfs:isDefinedBy <http://e-editiones.ch/ontology/human-geography#>;
	a owl:DatatypeProperty;
	rdfs:label "postal address has postcode value"@en, "Postanschrift hat Postleitzahlwert"@de;
#	ling:hasSynonym "has zip code"@en;
	rdfs:comment """Relating a postal address to its postcode value."""@en;
	rdfs:domain human-geography:PostalAddress;
	rdfs:range rdfs:Literal;
	rdfs:subPropertyOf concept:hasLiteral.

human-geography:addressHasTownNameLiteral
	rdfs:isDefinedBy <http://e-editiones.ch/ontology/human-geography#>;
	a owl:DatatypeProperty;
	rdfs:label "postal address has town name literal"@en, "Postanschrift hat Ortsnamenliteral"@de;
	rdfs:comment """Relating a postal address to its town name literal."""@en;
	rdfs:domain human-geography:PostalAddress;
	rdfs:range rdfs:Literal;
	rdfs:subPropertyOf text:hasNameLiteral.

human-geography:addressHasCountryNameLiteral
	rdfs:isDefinedBy <http://e-editiones.ch/ontology/human-geography#>;
	a owl:DatatypeProperty;
	rdfs:label "postal address has country name literal"@en, "Postanschrift hat Ländernamenliteral"@de;
	rdfs:comment """Relating a postal address to its country name literal."""@en;
	rdfs:domain human-geography:PostalAddress;
	rdfs:range rdfs:Literal;
	rdfs:subPropertyOf text:hasNameLiteral.
