@prefix rdfs: <http://www.w3.org/2000/01/rdf-schema#>.
@prefix owl: <http://www.w3.org/2002/07/owl#>.
@prefix xsd: <http://www.w3.org/2001/XMLSchema#>.
@prefix dct: <http://purl.org/dc/terms/>.
@prefix concept: <http://e-editiones.ch/ontology/concept#>.
@prefix language: <http://e-editiones.ch/ontology/language#>.

@base <http://e-editiones.ch/ontology/languages>.
@prefix languages: <http://e-editiones.ch/ontology/languages#>.

<http://e-editiones.ch/ontology/languages>
	a owl:Ontology;
	dct:title "An ontology about languages"@en;
	dct:description """Formal description of human natural languages, referring to the ISO 639 standards."""@en;
	dct:creator "Hans Cools, MD, knowledge engineer, ontologist, software developer, Basel University, Switzerland"@en;
	dct:publisher "Universities of Basel, Bern, and Zürich, Switzerland"@en;
	owl:versionInfo "2020-06-11"^^xsd:date.

#
# LANGUAGE CODING SYSTEM AND DATATYPE INSTANCES
#

languages:iso639System
	rdfs:isDefinedBy <http://e-editiones.ch/ontology/languages#>;
	a rdfs:Class, concept:CodingSystem;
	rdfs:label "ISO 639"@en;
	rdfs:comment """International standard for codes for the representation of names of languages."""@en;
	rdfs:seeAlso <https://www.iso.org/iso-639-language-codes.html>.

languages:iso639-1System
	rdfs:isDefinedBy <http://e-editiones.ch/ontology/languages#>;
	a rdfs:Class, concept:CodingSystem;
	rdfs:label "ISO 639-1"@en;
	rdfs:comment """ISO 639 part 1: alpha-2 (two-letter) codes."""@en;
	rdfs:subClassOf languages:iso639System;
	dct:hasVersion "ISO 639-1:2002";
	concept:codingSystemHasDataType languages:iso639-1;
	rdfs:seeAlso <http://www.infoterm.info/standardization/iso_639_1_2002.php>.

languages:iso639-1
	rdfs:isDefinedBy <http://e-editiones.ch/ontology/languages#>;
	a rdfs:Datatype;
	rdfs:label "ISO 639-1 datatype"@en;
	rdfs:comment """Datatype to type an ISO 639-1 alpha-2 code."""@en;
	rdfs:subClassOf xsd:string.

languages:iso639-2System # B and T codes for 20 languages, T codes favoured
	rdfs:isDefinedBy <http://e-editiones.ch/ontology/languages#>;
	a rdfs:Class, concept:CodingSystem;
	rdfs:label "ISO 639-2"@en;
	rdfs:comment """ISO 639 part 2: alpha-3 (three-letter) codes."""@en;
	rdfs:subClassOf languages:iso639System;
	dct:hasVersion "ISO 639-2:1998";
	concept:codingSystemHasDataType languages:iso639-2;
	rdfs:seeAlso <http://www.loc.gov/standards/iso639-2/>.

languages:iso639-2
	rdfs:isDefinedBy <http://e-editiones.ch/ontology/languages#>;
	a rdfs:Datatype;
	rdfs:label "ISO 639-2 datatype"@en;
	rdfs:comment """Datatype to type an ISO 639-2 alpha-3 code."""@en;
	rdfs:subClassOf xsd:string.

languages:iso639-3System
	rdfs:isDefinedBy <http://e-editiones.ch/ontology/languages#>;
	a rdfs:Class, concept:CodingSystem;
	rdfs:label "ISO 639-3"@en;
	rdfs:comment """ISO 639 part 3: alpha-3 (three-letter) codes for comprehensive coverage of languages."""@en;
	rdfs:subClassOf languages:iso639System;
	dct:hasVersion "ISO 639-3:2007";
	concept:codingSystemHasDataType languages:iso639-3;
	rdfs:seeAlso <http://www-01.sil.org/iso639-3/>.

languages:iso639-3
	rdfs:isDefinedBy <http://e-editiones.ch/ontology/languages#>;
	a rdfs:Datatype;
	rdfs:label "ISO 639-3 datatype"@en;
	rdfs:comment """Datatype to type an ISO 639-3 alpha-3 code."""@en;
	rdfs:subClassOf xsd:string.

#
# LANGUAGE INSTANCES
#

languages:BaselGerman
	rdfs:isDefinedBy <http://e-editiones.ch/ontology/languages#>;
	a rdfs:Class;
	rdfs:label "Basel German"@en, "Baseldeutsch"@de;
	rdfs:comment """Dialect of the city of Basel and its surroundings, Switzerland."""@en;
	rdfs:subClassOf language:SwissGerman.

languages:Dutch
	rdfs:isDefinedBy <http://e-editiones.ch/ontology/languages#>;
	a rdfs:Class;
	rdfs:label "Dutch"@en, "Niederländisch"@de, "Néerlandais"@fr, "olandese"@it, "Nederlands"@nl;
	rdfs:comment """The language developed and spoken in The Netherlands as the official language, and in the Flemish part of Belgium as one of the 3 official languages, and spoken in other parts of the world: in Suriname, Aruba, Curaçao, and Sint Maarten as official language; France, Germany, Indonesia, United States, Canada and Australia. It is also an official language of the European Union."""@en;
	rdfs:subClassOf language:GeneralHumanNaturalLanguage;
	language:hasCode [concept:codeHasSystem languages:iso639-1System; concept:codeHasValue "nl"^^languages:iso639-1];
	language:hasCode [concept:codeHasSystem languages:iso639-2System; concept:codeHasValue "dut"^^languages:iso639-2].

languages:English
	rdfs:isDefinedBy <http://e-editiones.ch/ontology/languages#>;
	a rdfs:Class;
	rdfs:label "English"@en, "Englisch"@de, "Anglais"@fr, "inglese"@it;
	rdfs:comment """The language developed and spoken in the United Kingdom, also an official language in 66 other countries, and spoken in other parts of the world. It is also an official language of the European Union."""@en;
	rdfs:subClassOf language:GeneralHumanNaturalLanguage;
	language:hasCode [concept:codeHasSystem languages:iso639-1System; concept:codeHasValue "en"^^languages:iso639-1];
	language:hasCode [concept:codeHasSystem languages:iso639-2System; concept:codeHasValue "eng"^^languages:iso639-2].

languages:French
	rdfs:isDefinedBy <http://e-editiones.ch/ontology/languages#>;
	a rdfs:Class;
	rdfs:label "French"@en, "Französisch"@de, "Français"@fr, "francese"@it;
	rdfs:comment """The language developed and spoken in France, also an official language in 29 other countries, and spoken in other parts of the world. It is also an official language of the European Union."""@en;
	rdfs:subClassOf language:GeneralHumanNaturalLanguage;
	language:hasCode [concept:codeHasSystem languages:iso639-1System; concept:codeHasValue "fr"^^languages:iso639-1];
	language:hasCode [concept:codeHasSystem languages:iso639-2System; concept:codeHasValue "fre"^^languages:iso639-2, "fra"^^languages:iso639-2].

languages:German
	rdfs:isDefinedBy <http://e-editiones.ch/ontology/languages#>;
	a rdfs:Class;
	rdfs:label "German"@en, "Deutsch"@de, "Allemand"@fr, "tedesco"@it;
	rdfs:comment """The language developed and spoken in Germany and Austria, also an official language in 5 other countries, and spoken in other parts of the world. It is also an official language of the European Union."""@en;
	rdfs:subClassOf language:GeneralHumanNaturalLanguage;
	language:hasCode [concept:codeHasSystem languages:iso639-1System; concept:codeHasValue "de"^^languages:iso639-1];
	language:hasCode [concept:codeHasSystem languages:iso639-2System; concept:codeHasValue "ger"^^languages:iso639-2, "deu"^^languages:iso639-2].

languages:Hungarian
	rdfs:isDefinedBy <http://e-editiones.ch/ontology/languages#>;
	a rdfs:Class;
	rdfs:label "Hungarian"@en, "Ungarisch"@de, "Hongrois"@fr, "ungherese"@it;
	rdfs:comment """The language developed and spoken in Hungary, and parts of several neighbouring countries, and an official language of the European Union."""@en;
	rdfs:subClassOf language:GeneralHumanNaturalLanguage;
	language:hasCode [concept:codeHasSystem languages:iso639-1System; concept:codeHasValue "hu"^^languages:iso639-1];
	language:hasCode [concept:codeHasSystem languages:iso639-2System; concept:codeHasValue "hun"^^languages:iso639-2].

languages:Italian
	rdfs:isDefinedBy <http://e-editiones.ch/ontology/languages#>;
	a rdfs:Class;
	rdfs:label "Italian"@en, "Italienisch"@de, "Italien"@fr, "italiana"@it;
	rdfs:comment """The language developed and spoken in Italy, also an official language in 2 other countries and a state, and spoken in other parts of the world. It is also an official language of the European Union."""@en;
	rdfs:subClassOf language:GeneralHumanNaturalLanguage;
	language:hasCode [concept:codeHasSystem languages:iso639-1System; concept:codeHasValue "it"^^languages:iso639-1];
	language:hasCode [concept:codeHasSystem languages:iso639-2System; concept:codeHasValue "ita"^^languages:iso639-2].

languages:Latin
	rdfs:isDefinedBy <http://e-editiones.ch/ontology/languages#>;
	a rdfs:Class;
	rdfs:label "Latin"@en, "Latein"@de, "Latin"@fr, "latino"@it;
	rdfs:comment """The language developed and spoken originally in Latium (the area around Rome), subsequently in Italy as the dominant language, and in the western Roman Empire. Classical language belonging to the Italic branch of the Indo-European languages. The largest organisation retaining Latin in official and quasi-official contexts is the Catholic Church."""@en;
	rdfs:subClassOf language:GeneralHumanNaturalLanguage;
	language:hasCode [concept:codeHasSystem languages:iso639-1System; concept:codeHasValue "la"^^languages:iso639-1];
	language:hasCode [concept:codeHasSystem languages:iso639-2System; concept:codeHasValue "lat"^^languages:iso639-2].

languages:Polish
	rdfs:isDefinedBy <http://e-editiones.ch/ontology/languages#>;
	a rdfs:Class;
	rdfs:label "Polish"@en, "Polnisch"@de, "polonais"@fr, "Polacco"@it, "Polski"@pl;
	rdfs:comment """The language developed and spoken in Poland. It is also an official language of the European Union."""@en; #°
	rdfs:subClassOf language:GeneralHumanNaturalLanguage;
	language:hasCode [concept:codeHasSystem languages:iso639-1System; concept:codeHasValue "pl"^^languages:iso639-1];
	language:hasCode [concept:codeHasSystem languages:iso639-2System; concept:codeHasValue "pol"^^languages:iso639-2].

languages:Portuguese
	rdfs:isDefinedBy <http://e-editiones.ch/ontology/languages#>;
	a rdfs:Class;
	rdfs:label "Portuguese"@en, "Portugiesisch"@de, "Portugais"@fr, "portoghese"@it;
	rdfs:comment """The language developed and spoken in Portugal. It is also an official language of the European Union."""@en; #°
	rdfs:subClassOf language:GeneralHumanNaturalLanguage;
	language:hasCode [concept:codeHasSystem languages:iso639-1System; concept:codeHasValue "pt"^^languages:iso639-1];
	language:hasCode [concept:codeHasSystem languages:iso639-2System; concept:codeHasValue "por"^^languages:iso639-2].

languages:Russian
	rdfs:isDefinedBy <http://e-editiones.ch/ontology/languages#>;
	a rdfs:Class;
	rdfs:label "Russian"@en, "Russisch"@de, "Russe"@fr, "russo"@it;
	rdfs:comment """The language developed and spoken in Russia."""@en; #°
	rdfs:subClassOf language:GeneralHumanNaturalLanguage;
	language:hasCode [concept:codeHasSystem languages:iso639-1System; concept:codeHasValue "ru"^^languages:iso639-1];
	language:hasCode [concept:codeHasSystem languages:iso639-2System; concept:codeHasValue "rus"^^languages:iso639-2].


languages:Sanskrit
	rdfs:isDefinedBy <http://e-editiones.ch/ontology/languages#>;
	a rdfs:Class;
	rdfs:label "Sanskrit"@en, "Sanskrit"@de, "sanskrit"@fr, "sanscrito"@it;
	rdfs:comment """."""@en;
	rdfs:subClassOf language:GeneralHumanNaturalLanguage;
	language:hasCode [concept:codeHasSystem languages:iso639-1System; concept:codeHasValue "sa"^^languages:iso639-1];
	language:hasCode [concept:codeHasSystem languages:iso639-2System; concept:codeHasValue "san"^^languages:iso639-2].

languages:Spanish
	rdfs:isDefinedBy <http://e-editiones.ch/ontology/languages#>;
	a rdfs:Class;
	rdfs:label "Spanish"@en, "Spanisch"@de, "Espagnol"@fr, "spagnola"@it;
	rdfs:comment """The language developed and spoken in Spain."""@en; #°
	rdfs:subClassOf language:GeneralHumanNaturalLanguage;
	language:hasCode [concept:codeHasSystem languages:iso639-1System; concept:codeHasValue "sa"^^languages:iso639-1];
	language:hasCode [concept:codeHasSystem languages:iso639-2System; concept:codeHasValue "san"^^languages:iso639-2].

languages:SwissGerman
	rdfs:isDefinedBy <http://e-editiones.ch/ontology/languages#>;
	a rdfs:Class;
	rdfs:label "Swiss German"@en, "Schweizerdeutsch"@de;
	rdfs:comment """Any of the Alemannic dialects spoken in the German-speaking part of Switzerland and in some Alpine communities in Northern Italy bordering Switzerland."""@en;
	rdfs:subClassOf language:GeneralHumanNaturalLanguage, [
		a owl:Restriction; owl:onProperty language:isDialectOf; owl:someValuesFrom languages:German].

#
# PROPERTIES
#

