@prefix rdfs: <http://www.w3.org/2000/01/rdf-schema#>.
@prefix owl: <http://www.w3.org/2002/07/owl#>.
@prefix xsd: <http://www.w3.org/2001/XMLSchema#>.
@prefix skos: <http://www.w3.org/2004/02/skos/core#>.
@prefix dct: <http://purl.org/dc/terms/>.
@prefix cidoc: <http://www.cidoc-crm.org/cidoc-crm/>.
@prefix agent: <http://e-editiones.ch/ontology/agent#>.
@prefix human: <http://e-editiones.ch/ontology/human#>.
@prefix creating: <http://e-editiones.ch/ontology/creating#>.
@prefix concept: <http://e-editiones.ch/ontology/concept#>.
@prefix device: <http://e-editiones.ch/ontology/device#>.

@base <http://e-editiones.ch/ontology/language>.
@prefix language: <http://e-editiones.ch/ontology/language#>.

<http://e-editiones.ch/ontology/language>
	a owl:Ontology;
	dct:license <http://creativecommons.org/licenses/by/3.0/>;
	dct:title "An ontology about language"@en;
	dct:description """Formal description of language, general subclasses, related classes and properties."""@en;
	dct:creator "Hans Cools, MD, knowledge engineer, ontologist, software developer, University of Basel, Switzerland"@en;
	dct:contributor "Rebekka Plüss, research assistant and software developer, University of Basel, Switzerland"@en;
	dct:publisher "Universities of Basel, Bern, and Zürich, Switzerland"@en;
	owl:versionInfo "2020-06-11"^^xsd:date.

#
# CLASSES
#

language:Language
	rdfs:isDefinedBy <http://e-editiones.ch/ontology/language#>;
	a rdfs:Class;
	rdfs:label "language"@en, "Sprache"@de;
	rdfs:comment """Dynamic set of sensory carriers, e.g. a sign, symbol, word, including sound and gesture, to express meaning, and used along rules or grammar model, e.g. syntax for serialization."""@en;
	rdfs:subClassOf dct:LinguisticSystem.

language:HumanLanguage
	rdfs:isDefinedBy <http://e-editiones.ch/ontology/language#>;
	a rdfs:Class;
	rdfs:label "human language"@en, "menschliche Sprache"@de;
	rdfs:comment """Language of a human."""@en;
	skos:note """Also formal language, e.g. computer programming language."""@en;
	rdfs:subClassOf language:Language. #*, human:Ability.

language:HumanNaturalLanguage
	rdfs:isDefinedBy <http://e-editiones.ch/ontology/language#>;
	a rdfs:Class;
	rdfs:label "human natural language"@en, "menschliche natürliche Sprache"@de;
	rdfs:comment """Language naturally evolved in humans."""@en;
	skos:note """Excluded is formal language, e.g. computer programming language."""@en;
	rdfs:subClassOf language:HumanLanguage.
#	owl:disjointWith language:FormalLanguage.

language:GeneralHumanNaturalLanguage
	rdfs:isDefinedBy <http://e-editiones.ch/ontology/language#>;
	a rdfs:Class;
	rdfs:label "general human natural language"@en, "allgemeine menschliche natürliche Sprache"@de;
	rdfs:comment """Language naturally evolved in humans and used as official language in one or more countries."""@en; #°
	rdfs:subClassOf language:HumanNaturalLanguage.

language:HumanNaturalLanguageExpression
	rdfs:isDefinedBy <http://e-editiones.ch/ontology/language#>;
	a rdfs:Class;
	rdfs:label "human natural language expression"@en, "menschliche natürliche sprachliche Äusserung"@de;
	rdfs:comment """Expression in a human natural language."""@en;
	skos:note """Expression differs from the FRBRoo based document:Expression."""@en;
	rdfs:subClassOf concept:Information, cidoc:E33_Linguistic_Object.

language:Dialect
	rdfs:isDefinedBy <http://e-editiones.ch/ontology/language#>;
	a rdfs:Class;
	rdfs:label "dialect"@en, "Dialekt"@de;
	rdfs:comment """Regional variant of a standard human natural language."""@en;
	rdfs:subClassOf language:HumanNaturalLanguage.

language:AgentTranslator
	rdfs:isDefinedBy <http://e-editiones.ch/ontology/language#>;
	a rdfs:Class;
	rdfs:label "translator role of agent"@en, "Übersetzerrolle eines Akteurs"@de;
	rdfs:comment """Role of an agent, person or machine, transferring a human natural language expression in another natural language."""@en;
	rdfs:subClassOf agent:Creator.

language:PersonTranslator
	rdfs:isDefinedBy <http://e-editiones.ch/ontology/language#>;
	a rdfs:Class;
	rdfs:label "translator role of person"@en, "Übersetzerrolle einer Person"@de;
	rdfs:comment """Translator as role of a person."""@en;
	rdfs:subClassOf language:AgentTranslator, creating:PersonCreator.

language:MachineTranslator
	rdfs:isDefinedBy <http://e-editiones.ch/ontology/language#>;
	a rdfs:Class;
	rdfs:label "translator role of machine"@en, "Übersetzerrolle einer Maschine"@de;
	rdfs:comment """Translator as role of a machine."""@en;
	rdfs:subClassOf language:AgentTranslator.

language:Translation
	rdfs:isDefinedBy <http://e-editiones.ch/ontology/language#>;
	a rdfs:Class;
	rdfs:label "translation"@en, "Übersetzung"@de, "traduction"@fr, "traduzione"@it;
	rdfs:comment """Human natural language expression transferred from another natural language."""@en;
	skos:note """Can follow the original to a degree, hence differ from another translation; e.g. a free translation gives a general meaning."""@en;
	rdfs:seeAlso <https://www.abc-clio.com/ODLIS/odlis_t.aspx#translation>;
	rdfs:subClassOf language:HumanNaturalLanguageExpression.

language:PersonTranslation
	rdfs:isDefinedBy <http://e-editiones.ch/ontology/language#>;
	a rdfs:Class;
	rdfs:label "person translation"@en, "Übersetzung einer Person"@de;
	rdfs:comment """Translation done by a person."""@en;
	rdfs:subClassOf language:Translation, creating:CreationDerivative.

language:MachineTranslation
	rdfs:isDefinedBy <http://e-editiones.ch/ontology/language#>;
	a rdfs:Class;
	rdfs:label "machine translation"@en, "maschinelle Übersetzung"@de, "traduction automatique"@fr, "traduzione automatica"@it;
	rdfs:comment """Translation done by a digital electronic computer using translation software."""@en;
	rdfs:subClassOf language:Translation.

language:PartialTranslation
	rdfs:isDefinedBy <http://e-editiones.ch/ontology/language#>;
	a rdfs:Class;
	rdfs:label "partial translation"@en, "Teilübersetzung"@de, "traduction partielle"@fr, "traduzione parziale"@it;
	rdfs:comment """Translation being an incomplete transfer from a human natural language expression in another natural language."""@en;
	rdfs:seeAlso <https://www.abc-clio.com/ODLIS/odlis_t.aspx#translation>;
	rdfs:subClassOf language:HumanNaturalLanguageExpression.

language:IdentifierCode
	rdfs:isDefinedBy <http://e-editiones.ch/ontology/language#>;
	a rdfs:Class;
	rdfs:label "language identifier code"@en, "Spracheidentifikatorcode"@de, "code d'indentification de langue"@fr, "codice del identificazione della lingua"@it;
	rdfs:comment """Identifier code in a coding system, attributed to a human natural language, e.g. ISO 639."""@en;
	rdfs:seeAlso <http://e-editiones.ch/ontology/languages#>;
	rdfs:subClassOf concept:IdentifierCode.

#
# PROPERTIES
#

language:hasIdentifierCode
	rdfs:isDefinedBy <http://e-editiones.ch/ontology/language#>;
	a owl:InverseFunctionalProperty;
	rdfs:label "language has identifier code"@en, "Sprache hat Identifikatorcode"@de;
	rdfs:comment """Relating a language to an identifier code representing that language."""@en;
	rdfs:domain language:HumanNaturalLanguage;
	rdfs:range language:IdentifierCode;
	rdfs:subPropertyOf concept:hasIdentifierCode.

language:hasContentLiteral
	rdfs:isDefinedBy <http://e-editiones.ch/ontology/language#>;
	a owl:DatatypeProperty;
	rdfs:label "has content literal"@en, "hat Inhaltliteral"@de;
	rdfs:comment """Relating a human natural language expression to its content."""@en;
	rdfs:domain language:HumanNaturalLanguageExpression;
	rdfs:range rdfs:Literal;
	rdfs:subPropertyOf concept:symbolicEntityHasLiteral.

language:isDialectOf
	rdfs:isDefinedBy <http://e-editiones.ch/ontology/language#>;
	a owl:ObjectProperty;
	rdfs:label "is dialect of"@en, "ist Dialekt von"@de;
	rdfs:comment """Relating a dialect to its human natural language."""@en;
	rdfs:domain language:Dialect;
	rdfs:range language:HumanNaturalLanguage.

language:expressedInNaturalLanguage
	rdfs:isDefinedBy <http://e-editiones.ch/ontology/language#>;
	a owl:ObjectProperty;
	rdfs:label "expressed in natural language"@en, "geäußert in natürlicher Sprache"@de;
	rdfs:comment """Relating a human expression to a natural language wherein it is expressed."""@en;
	rdfs:domain language:HumanNaturalLanguageExpression;
	rdfs:range language:HumanNaturalLanguage;
	rdfs:subPropertyOf cidoc:P72_has_language.

language:expressedInDialect
	rdfs:isDefinedBy <http://e-editiones.ch/ontology/language#>;
	a owl:ObjectProperty;
	rdfs:label "expressed in dialect"@en, "geäußert in Dialekt"@de;
	rdfs:comment """Relating a human expression to a dialect it is expressed in."""@en;
	rdfs:domain language:HumanNaturalLanguageExpression;
	rdfs:range language:Dialect.

language:hasTranslator
	rdfs:isDefinedBy <http://e-editiones.ch/ontology/language#>;
	a owl:ObjectProperty;
	rdfs:label "has translator"@en, "hat Übersetzer"@de;
	rdfs:comment """Relating a natural language expression to an agent that translated it."""@en;
	rdfs:domain language:HumanNaturalLanguageExpression;
	rdfs:range [rdfs:subClassOf agent:Agent, [a owl:Restriction; owl:onProperty agent:hasRole; owl:someValuesFrom language:AgentTranslator]].

language:hasPersonTranslator
	rdfs:isDefinedBy <http://e-editiones.ch/ontology/language#>;
	a owl:ObjectProperty;
	rdfs:label "has person translator"@en, "hat menschlichen Übersetzer"@de;
	rdfs:comment """Relating a natural language expression to a person who translated it."""@en;
	rdfs:domain language:HumanNaturalLanguageExpression;
	rdfs:range [rdfs:subClassOf human:Person, [a owl:Restriction; owl:onProperty human:personHasRole; owl:someValuesFrom language:PersonTranslator]];
	rdfs:subPropertyOf language:hasTranslator.

language:hasMachineTranslator
	rdfs:isDefinedBy <http://e-editiones.ch/ontology/language#>;
	a owl:ObjectProperty;
	rdfs:label "has machine translator"@en, "hat maschinellen Übersetzer"@de;
	rdfs:comment """Relating a natural language expression to a machine that translated it."""@en;
	rdfs:domain language:HumanNaturalLanguageExpression;
	rdfs:range [rdfs:subClassOf device:DigitalElectronicComputer, [a owl:Restriction; owl:onProperty agent:hasRole; owl:someValuesFrom language:MachineTranslator]];
	rdfs:subPropertyOf language:hasTranslator.

language:translationHasTranslator
	rdfs:isDefinedBy <http://e-editiones.ch/ontology/language#>;
	a owl:ObjectProperty;
	rdfs:label "translation has translator"@en, "Übersetzung hat Übersetzer"@de;
	rdfs:comment """Relating a translation to an agent that created it."""@en;
	rdfs:domain language:Translation;
	rdfs:range [rdfs:subClassOf agent:Agent, [a owl:Restriction; owl:onProperty agent:hasRole; owl:someValuesFrom language:AgentTranslator]].

language:translationHasPersonTranslator
	rdfs:isDefinedBy <http://e-editiones.ch/ontology/language#>;
	a owl:ObjectProperty;
	rdfs:label "translation has person translator"@en, "Übersetzung hat menschlichen Übersetzer"@de;
	rdfs:comment """Relating a translation to a person who created it."""@en;
	rdfs:domain language:PersonTranslation;
	rdfs:range [rdfs:subClassOf human:Person, [a owl:Restriction; owl:onProperty human:personHasRole; owl:someValuesFrom language:PersonTranslator]];
	rdfs:subPropertyOf language:translationHasTranslator.

language:translationHasMachineTranslator
	rdfs:isDefinedBy <http://e-editiones.ch/ontology/language#>;
	a owl:ObjectProperty;
	rdfs:label "translation has machine translator"@en, "Übersetzung hat maschinellen Übersetzer"@de;
	rdfs:comment """Relating a translation to a machine that created it."""@en;
	rdfs:domain language:MachineTranslation;
	rdfs:range [rdfs:subClassOf device:DigitalElectronicComputer, [a owl:Restriction; owl:onProperty agent:hasRole; owl:someValuesFrom language:MachineTranslator]];
	rdfs:subPropertyOf language:translationHasTranslator.

language:hasTranslation
	rdfs:isDefinedBy <http://e-editiones.ch/ontology/language#>;
	a owl:ObjectProperty;
	rdfs:label "has translation"@en, "hat Übersetzung"@de;
	rdfs:comment """Relating a human natural language expression to another one in another natural language into which it is translated."""@en;
	rdfs:domain language:HumanNaturalLanguageExpression;
	rdfs:range language:Translation.

language:hasPartialTranslation
	rdfs:isDefinedBy <http://e-editiones.ch/ontology/language#>;
	a owl:ObjectProperty;
	rdfs:label "has partial translation"@en, "hat Teilübersetzung"@de;
	rdfs:comment """Relating a human natural language expression to another one in another natural language into which it is partially translated."""@en;
	rdfs:domain language:HumanNaturalLanguageExpression;
	rdfs:range language:PartialTranslation.

language:isTranslatedInto
	rdfs:isDefinedBy <http://e-editiones.ch/ontology/language#>;
	a owl:ObjectProperty;
	rdfs:label "is translated into"@en, "ist übersetzt in"@de;
	rdfs:comment """Relating a human natural language expression to the language it is translated into."""@en;
	rdfs:domain language:HumanNaturalLanguageExpression;
	rdfs:range language:HumanNaturalLanguage;
	rdfs:subPropertyOf language:expressedInNaturalLanguage;
	owl:propertyChainAxiom (language:hasTranslation language:expressedInNaturalLanguage).
