@prefix rdfs: <http://www.w3.org/2000/01/rdf-schema#>.
@prefix owl: <http://www.w3.org/2002/07/owl#>.
@prefix xsd: <http://www.w3.org/2001/XMLSchema#>.
@prefix dct: <http://purl.org/dc/terms/>.
@prefix frbroo: <http://iflastandards.info/ns/fr/frbr/frbroo/>.
@prefix physical: <http://e-editiones.ch/ontology/physical-entity#>.
@prefix event: <http://e-editiones.ch/ontology/event#>.
@prefix human: <http://e-editiones.ch/ontology/human#>.
@prefix creating: <http://e-editiones.ch/ontology/creating#>.
@prefix text-expression: <http://e-editiones.ch/ontology/text-expression#>.
@prefix text-structure: <http://e-editiones.ch/ontology/text-structure#>.
@prefix infocar: <http://e-editiones.ch/ontology/information-carrier#>.


@base <http://e-editiones.ch/ontology/letter-corresponding>.
@prefix letter-corresponding: <http://e-editiones.ch/ontology/letter-corresponding#>.

<http://e-editiones.ch/ontology/letter-corresponding>
	a owl:Ontology;
	dct:license <http://creativecommons.org/licenses/by/3.0/>;
	dct:title "An ontology about letter corresponding"@en;
	dct:description """Formal description of letter corresponding, related classes, and properties."""@en;
	dct:creator "Hans Cools, MD, knowledge engineer, ontologist, software developer, University of Basel, Switzerland"@en;
	dct:contributor
		"Roberta Padlina, project coordinator and software developer, University of Basel, Switzerland"@en,
		"Reto Baumgartner, tool coordinator and software developer, University of Zürich, Switzerland"@en;
	dct:publisher "Universities of Basel, Bern, and Zürich, Switzerland"@en;
	owl:versionInfo "2020-06-11"^^xsd:date.

#
# CLASSES
#

letter-corresponding:Corresponding
 	rdfs:isDefinedBy <http://e-editiones.ch/ontology/letter-corresponding#>;
	a rdfs:Class;
 	rdfs:label "corresponding"@en,"Korrespondieren"@de, "correspondre"@fr, "corrispondere"@it;
 	rdfs:comment """Communicating by exchanging letters."""@en;
	rdfs:subClassOf human:Procedure.

letter-corresponding:Exchanging
 	rdfs:isDefinedBy <http://e-editiones.ch/ontology/letter-corresponding#>;
	a rdfs:Class;
 	rdfs:label "exchanging"@en,"Auswechselen"@de, "échanger"@fr, "scambiare"@it;
 	rdfs:comment """Sending-receiving cycle in corresponding."""@en;
	rdfs:subClassOf human:Procedure.

letter-corresponding:Compiling
 	rdfs:isDefinedBy <http://e-editiones.ch/ontology/letter-corresponding#>;
	a rdfs:Class;
 	rdfs:label "compiling"@en,"Zusammenstellen"@de, "compiler"@fr, "compilare"@it;
 	rdfs:comment """Preparing a letter for sending, mostly by putting it in an envelope, possibly adding an enclosure."""@en;
	rdfs:subClassOf human:Procedure.

letter-corresponding:Expression
	rdfs:isDefinedBy <http://e-editiones.ch/ontology/letter-corresponding#>;
	a rdfs:Class;
	rdfs:label "letter expression"@en, "Brief-Expression"@de, "expression de lettre"@fr, "espressione letterale"@it;
	rdfs:comment """Text expression with a letter content and possibly structure."""@en;
	rdfs:subClassOf text-expression:IndividualExpression.

letter-corresponding:Structure
	rdfs:isDefinedBy <http://e-editiones.ch/ontology/letter-corresponding#>;
	a rdfs:Class;
	rdfs:label "letter structure"@en, "Briefstruktur"@de, "structure de lettre"@fr, "struttura della lettera"@it;
	rdfs:comment """Text with letter structure."""@en;
	rdfs:subClassOf text-structure:CompositionalContentStructure.

letter-corresponding:Letter
	rdfs:isDefinedBy <http://e-editiones.ch/ontology/letter-corresponding#>;
	a rdfs:Class;
	rdfs:label "letter"@en, "Brief"@de, "lettre"@fr, "lettera"@it;
	rdfs:comment """Written text, e.g. on a leaf, intended to be sent from (a) person(s) or (an) Organization(s) to (an)other one(s), e.g. through a postal system."""@en;
	rdfs:subClassOf infocar:Carrier, frbroo:F4_Manifestation_Singleton.

letter-corresponding:Envelope
	rdfs:isDefinedBy <http://e-editiones.ch/ontology/letter-corresponding#>;
	a rdfs:Class;
	rdfs:label "envelope"@en, "Umschlag"@de, "enveloppe"@fr, "busta"@it;
	rdfs:comment """Flat paper container with a sealable flap for sending something, e.g. a letter, from (a) person(s) or (an) Organization(s) to another one, e.g. through a postal system."""@en;
	rdfs:subClassOf creating:PhysicalCreation.

letter-corresponding:EnclosureExpression
	rdfs:isDefinedBy <http://e-editiones.ch/ontology/letter-corresponding#>;
	a rdfs:Class;
	rdfs:label "letter enclosure text expression"@en, "Briefbeilage-Textexpression"@de, "expression de texte d'une pièce jointe d'une lettre"@fr, "espressione di testo allegato lettera"@it;
	rdfs:comment """Text expression of a letter enclosure."""@en;
	rdfs:subClassOf text-expression:IndividualExpression.

letter-corresponding:Enclosure
	rdfs:isDefinedBy <http://e-editiones.ch/ontology/letter-corresponding#>;
	a rdfs:Class;
	rdfs:label "letter enclosure"@en, "Briefbeilage"@de, "pièce jointe d'une lettre"@fr, "allegato di una lettera"@it;
	rdfs:comment """Something added to a letter being sent, e.g. another information carrier."""@en;
	rdfs:subClassOf creating:PhysicalCreation.

letter-corresponding:InformationEnclosure
	rdfs:isDefinedBy <http://e-editiones.ch/ontology/letter-corresponding#>;
	a rdfs:Class;
	rdfs:label "information letter enclosure"@en, "Information-Briefbeilage"@de, "information annexe à une lettre"@fr, "allegato lettera informativa"@it;
	rdfs:comment """Information carrier as letter enclosure."""@en;
	rdfs:subClassOf letter-corresponding:Enclosure, infocar:Carrier.

#
# PROPERTIES
#

letter-corresponding:isExchangingOf
	rdfs:isDefinedBy <http://e-editiones.ch/ontology/letter-corresponding#>;
	a owl:ObjectProperty;
	rdfs:label "is exchanging of"@en, "ist Auswechselen von"@de, "est un échange de"@fr, "è uno scambio di"@it;
	rdfs:comment """Relating an exchanging to its corresponding it is a suprocedure of."""@en;
	rdfs:domain letter-corresponding:Exchanging;
	rdfs:range letter-corresponding:Corresponding;
	rdfs:subPropertyOf event:isSubProcedureOf.

letter-corresponding:isCompilingOf
	rdfs:isDefinedBy <http://e-editiones.ch/ontology/letter-corresponding#>;
	a owl:ObjectProperty;
	rdfs:label "is compiling of"@en, "ist Zusammenstellen von"@de, "est la compilation de"@fr, "è la compilazione di"@it;
	rdfs:comment """Relating a compiling to its exchanging it is a suprocedure of."""@en;
	rdfs:domain letter-corresponding:Compiling;
	rdfs:range letter-corresponding:Exchanging;
	rdfs:subPropertyOf event:isSubProcedureOf.

letter-corresponding:isInLetter
	rdfs:isDefinedBy <http://e-editiones.ch/ontology/letter-corresponding#>;
	a owl:ObjectProperty;
	rdfs:label "is in letter"@en, "ist in Brief"@de, "est en lettre"@fr, "è nella lettera"@it;
	rdfs:comment """Relating a letter expression to a letter it is in."""@en;
	rdfs:domain letter-corresponding:Expression;
	rdfs:range letter-corresponding:Letter;
	rdfs:subPropertyOf infocar:isOnCarrier.

letter-corresponding:isStructureOfExpression
	rdfs:isDefinedBy <http://e-editiones.ch/ontology/letter-corresponding#>;
	a owl:ObjectProperty;
	rdfs:label "is letter structure of expression"@en, "ist Briefstruktur einer Expression"@de, "est la structure de lettre d'une expression"@fr, "è la struttura delle lettere di un'espressione"@it;
	rdfs:comment """Relating a letter structure to a text expression it is part of."""@en;
	rdfs:domain letter-corresponding:Structure;
	rdfs:range letter-corresponding:Expression;
	rdfs:subPropertyOf text-structure:isPartOfTextExpression.

letter-corresponding:follows
	rdfs:isDefinedBy <http://e-editiones.ch/ontology/letter-corresponding#>;
	a owl:ObjectProperty;
	rdfs:label "letter follows"@en, "Brief folgt"@de, "lettre suivant de"@fr, "lettera successiva a"@it;
	rdfs:comment """Relating a letter to a preceding letter."""@en;
	rdfs:domain letter-corresponding:Letter;
	rdfs:range letter-corresponding:Letter.

letter-corresponding:hasEnvelope
	rdfs:isDefinedBy <http://e-editiones.ch/ontology/letter-corresponding#>;
	a owl:ObjectProperty;
	rdfs:label "letter has envelope"@en, "Brief hat Umschlag"@de, "lettre a une enveloppe"@fr,  "lettera ha una busta"@it;
	rdfs:comment """Relating a letter to an envelope it has."""@en;
	rdfs:domain letter-corresponding:Letter;
	rdfs:range letter-corresponding:Envelope.

letter-corresponding:hasEnvelopeDescription
	rdfs:isDefinedBy <http://e-editiones.ch/ontology/letter-corresponding#>;
	a owl:ObjectProperty;
	rdfs:label "letter has envelope description"@en, "Brief hat Umschlagbeschreibung"@de, "lettre a une description de l'enveloppe"@fr, "lettera ha una descrizione della busta"@it;
	rdfs:comment """Relating a letter to a description of its envelope."""@en;
	rdfs:domain letter-corresponding:Letter;
	rdfs:range rdfs:Literal.

letter-corresponding:hasEnclosure
	rdfs:isDefinedBy <http://e-editiones.ch/ontology/letter-corresponding#>;
	a owl:ObjectProperty;
	rdfs:label "letter has enclosure"@en, "Brief hat Beilage"@de, "lettre a une pièce jointe"@fr, "lettera ha un allegato"@it;
	rdfs:comment """Relating a letter to an enclosure it has."""@en;
	rdfs:domain letter-corresponding:Letter;
	rdfs:range letter-corresponding:Enclosure.

letter-corresponding:isPageOfLetter
	rdfs:isDefinedBy <http://e-editiones.ch/ontology/letter-corresponding#>;
	a owl:ObjectProperty;
	rdfs:label "is page of letter"@en, "ist Seite eines Briefes"@de, "est une page d'une lettre"@fr, "è una pagina di una lettera"@it;
	rdfs:comment """Relating a page to the letter it is part of."""@en;
	rdfs:domain infocar:Page;
	rdfs:range letter-corresponding:Letter;
	rdfs:subPropertyOf physical:isPartOf.

letter-corresponding:isTextInEnclosure
	rdfs:isDefinedBy <http://e-editiones.ch/ontology/letter-corresponding#>;
	a owl:ObjectProperty;
	rdfs:label "is text expression in letter enclosure"@en, "ist Textexpression in Briefbeilage"@de, "est une expression textuelle dans une pièce-jointe à une lettre"@fr, "è un'espressione di testo in un allegato di lettera"@it;
	rdfs:comment """Relating a text expression to a letter information enclosure it is in."""@en;
	rdfs:domain letter-corresponding:EnclosureExpression;
	rdfs:range letter-corresponding:InformationEnclosure;
	rdfs:subPropertyOf infocar:isOnCarrier.