@prefix rdfs: <http://www.w3.org/2000/01/rdf-schema#>.
@prefix owl: <http://www.w3.org/2002/07/owl#>.
@prefix xsd: <http://www.w3.org/2001/XMLSchema#>.
@prefix skos: <http://www.w3.org/2004/02/skos/core#>.
@prefix dct: <http://purl.org/dc/terms/>.
@prefix human: <http://e-editiones.ch/ontology/human#>.
@prefix concept: <http://e-editiones.ch/ontology/concept#>.
@prefix text: <http://e-editiones.ch/ontology/text#>.

@base <http://e-editiones.ch/ontology/mathematics>.
@prefix mathematics: <http://e-editiones.ch/ontology/mathematics#>.

<http://e-editiones.ch/ontology/mathematics>
	a owl:Ontology;
	dct:license <http://creativecommons.org/licenses/by/3.0/>;
	dct:title "An ontology about mathematics"@en;
	dct:description """Formal description of general concepts in mathematics."""@en;
	dct:creator "Hans Cools, MD, knowledge engineer, ontologist, software developer, University of Basel, Switzerland"@en;
	dct:publisher "University of Basel, Switzerland"@en;
	rdfs:seeAlso <http://eulersharp.sourceforge.net/2003/03swap/xsd-rules#>;
	owl:versionInfo "2020-06-11"^^xsd:date.

#
# CLASSES
#

mathematics:MathematicalObject
	rdfs:isDefinedBy <http://e-editiones.ch/ontology/mathematics#>;
	a rdfs:Class;
	rdfs:label "mathematical object"@en, "mathematisches Objekt"@de;
	rdfs:comment """Conceptual entity in mathematics."""@en;
	rdfs:subClassOf concept:ConceptualEntity.

mathematics:Number
	rdfs:isDefinedBy <http://e-editiones.ch/ontology/mathematics#>;
	a rdfs:Class;
	rdfs:label "number"@en, "Zahl"@de;
	rdfs:comment """Mathematical object used for counting, measuring, ordering, labeling, and coding."""@en;
	rdfs:subClassOf mathematics:MathematicalObject, concept:SymbolicEntity.

mathematics:NaturalNumber
	rdfs:isDefinedBy <http://e-editiones.ch/ontology/mathematics#>;
	a rdfs:Class;
	rdfs:label "natural number"@en, "nat√ºrliche Zahl"@de;
	rdfs:comment """Non-negative whole number used for counting and ordering."""@en;
	skos:note """Conform ISO 80000-2:2009."""@en;
	rdfs:subClassOf mathematics:Number, [
		a owl:Restriction; owl:onProperty mathematics:numberHasNumeral; owl:allValuesFrom xsd:nonNegativeInteger].

mathematics:OrdinalSymbol
	rdfs:isDefinedBy <http://e-editiones.ch/ontology/mathematics#>;
	a rdfs:Class;
	rdfs:label "ordinal symbol"@en, "Ordinalsymbol"@de;
	rdfs:comment """Symbol used to order, i.e. denoting the position of something in a sequence, e.g. the letters of an alphabet with literals a to z or A to Z."""@en;
	rdfs:subClassOf concept:Identifier.

mathematics:OrdinalNumber
	rdfs:isDefinedBy <http://e-editiones.ch/ontology/mathematics#>;
	a rdfs:Class;
	rdfs:label "ordinal number"@en, "Ordinalzahl"@de;
	rdfs:comment """Natural number used to order, i.e. denoting the position of something in a sequence."""@en;
	rdfs:subClassOf mathematics:NaturalNumber, mathematics:OrdinalSymbol.

mathematics:Set
	rdfs:isDefinedBy <http://e-editiones.ch/ontology/mathematics#>;
	a rdfs:Class;
	rdfs:label "mathematical set"@en, "mathematische Reihe"@de;
	rdfs:comment """Set of mathematical objects."""@en;
	rdfs:subClassOf concept:Set, mathematics:MathematicalObject.

#
# PROPERTIES
#

mathematics:hasNumber
 	rdfs:isDefinedBy <http://e-editiones.ch/ontology/mathematics#>;
	a owl:ObjectProperty;
	rdfs:label "has number"@en, "hat Zahl"@de;
	rdfs:comment """Relating something to a number."""@en;
	rdfs:domain rdfs:Resource;
	rdfs:range mathematics:Number;
	rdfs:subPropertyOf concept:hasSymbolicEntity.

mathematics:numberHasNumeral
	rdfs:isDefinedBy <http://e-editiones.ch/ontology/mathematics#>;
	a owl:DatatypeProperty;
	rdfs:label "number has numeral"@en, "Nummer hat Numeral"@de;
	rdfs:comment """Relating a number to its representing numeral."""@en;
	rdfs:domain mathematics:Number;
 	rdfs:range xsd:decimal;
 	rdfs:subPropertyOf concept:symbolicEntityHasLiteral.

mathematics:hasNumeral
	rdfs:isDefinedBy <http://e-editiones.ch/ontology/mathematics#>;
	a owl:DatatypeProperty;
	rdfs:label "has numeral"@en, "hat Numeral"@de;
	rdfs:comment """Relating something to a numeral."""@en;
	skos:note """A reification of a numeral, i.e. a number, can always be interposed, see property chain axiom."""@en;
	rdfs:domain rdfs:Resource;
 	rdfs:range xsd:decimal;
	rdfs:subPropertyOf concept:hasLiteral;
 	owl:propertyChainAxiom (mathematics:hasNumber mathematics:numberHasNumeral).

mathematics:hasOrdinalSymbol
 	rdfs:isDefinedBy <http://e-editiones.ch/ontology/mathematics#>;
	a owl:ObjectProperty;
	rdfs:label "has ordinal symbol"@en, "hat Ordinalsymbol"@de;
	rdfs:comment """Relating something to the symbolic entity denoting its position in a sequence."""@en;
	rdfs:domain rdfs:Resource;
	rdfs:range mathematics:OrdinalSymbol;
	rdfs:subPropertyOf concept:hasIdentifier.

mathematics:hasOrdinalNumber
 	rdfs:isDefinedBy <http://e-editiones.ch/ontology/mathematics#>;
	a owl:ObjectProperty;
	rdfs:label "has ordinal number"@en, "hat Ordinalzahl"@de;
	rdfs:comment """Relating something to the number denoting its position in a sequence."""@en;
	rdfs:domain rdfs:Resource;
	rdfs:range mathematics:OrdinalNumber;
	rdfs:subPropertyOf mathematics:hasOrdinalSymbol.

mathematics:hasOrdinalLiteral
	rdfs:isDefinedBy <http://e-editiones.ch/ontology/mathematics#>;
	a owl:DatatypeProperty;
	rdfs:label "has ordinal literal"@en, "hat Ordinalliteral"@de;
	rdfs:comment """Relating something to the literal denoting its position in a sequence."""@en;
	rdfs:domain rdfs:Resource;
	rdfs:range rdfs:Literal;
	rdfs:subPropertyOf concept:hasLiteral;
	owl:propertyChainAxiom (mathematics:hasOrdinalSymbol concept:symbolicEntityHasLiteral).

mathematics:hasOrdinalNumeral
	rdfs:isDefinedBy <http://e-editiones.ch/ontology/mathematics#>;
	a owl:DatatypeProperty;
	rdfs:label "has ordinal numeral"@en, "hat Ordinalnumeral"@de;
	rdfs:comment """Relating something to the numeral denoting its position in a sequence."""@en;
	rdfs:domain rdfs:Resource;
	rdfs:range xsd:nonNegativeInteger;
	rdfs:subPropertyOf mathematics:hasOrdinalLiteral;
 	owl:propertyChainAxiom (mathematics:hasOrdinalNumber mathematics:numberHasNumeral).
