@prefix rdfs: <http://www.w3.org/2000/01/rdf-schema#>.
@prefix owl: <http://www.w3.org/2002/07/owl#>.
@prefix xsd: <http://www.w3.org/2001/XMLSchema#>.
@prefix skos: <http://www.w3.org/2004/02/skos/core#>.
@prefix dct: <http://purl.org/dc/terms/>.
@prefix human: <http://e-editiones.ch/ontology/human#>.
@prefix philo: <http://e-editiones.ch/ontology/philosophy#>.

@base <http://e-editiones.ch/ontology/philosophies>.
@prefix philos: <http://e-editiones.ch/ontology/philosophies#>.

<http://e-editiones.ch/ontology/philosophies>
	a owl:Ontology;
	dct:license <http://creativecommons.org/licenses/by/3.0/>;
	dct:title "An ontology about philosophies"@en;
	dct:description """Formal description of philosophies, general subclasses, related classes, properties, and instances."""@en;
	dct:creator "Hans Cools, MD, knowledge engineer, ontologist, software developer, Basel University, Switzerland"@en;
	dct:contributor
		"Prof. Dr. Ueli Zahnd, Faculty of Theology, University of Basel, Switzerland"@en,
		"Gabriel Müller, Faculty of Theology, University of Basel, Switzerland"@en;
	dct:publisher "Universities of Basel, Bern, and Zürich, Switzerland"@en;
	owl:versionInfo "2020-06-11"^^xsd:date.

#
# INSTANCES
#

philos:Albertism
	rdfs:isDefinedBy <http://e-editiones.ch/ontology/philosophies#>;
	a rdfs:Class;
	#rdfs:isDefinedBy <http://e-editiones.ch/ontology/philosophies#>;
	rdfs:label "Albertism"@en;
	rdfs:comment """Philosophy and theology based on the ideas of Albertus Magnus (before 1200 - 1280-11-15)."""@en;
	rdfs:subClassOf philo:Philosophy. # :Theology

philos:Humanism
	rdfs:isDefinedBy <http://e-editiones.ch/ontology/philosophies#>;
	a rdfs:Class;
	#rdfs:isDefinedBy <http://e-editiones.ch/ontology/philosophies#>;
	rdfs:label "Humanism"@en;
	rdfs:comment """."""@en; #°
	rdfs:subClassOf philo:Philosophy.

philos:Nominalism
	rdfs:isDefinedBy <http://e-editiones.ch/ontology/philosophies#>;
	a rdfs:Class;
	#rdfs:isDefinedBy <http://e-editiones.ch/ontology/philosophies#>;
	rdfs:label "Nominalism"@en;
	rdfs:comment """Philosophy stating that only individual things exist, denying the existence of universals and abstract objects."""@en;
	rdfs:subClassOf philo:Metaphysics.

philos:Scotism
	rdfs:isDefinedBy <http://e-editiones.ch/ontology/philosophies#>;
	a rdfs:Class;
	#rdfs:isDefinedBy <http://e-editiones.ch/ontology/philosophies#>;
	rdfs:label "Scotism"@en;
	rdfs:comment """."""@en; #°
	rdfs:subClassOf philo:Philosophy.

philos:Thomism
	rdfs:isDefinedBy <http://e-editiones.ch/ontology/philosophies#>;
	a rdfs:Class;
	#rdfs:isDefinedBy <http://e-editiones.ch/ontology/philosophies#>;
	rdfs:label "Thomism"@en;
	rdfs:comment """Philosophy based on the work of Thomas Aquinas (1225 - 1274-O3-O7)."""@en;
	rdfs:subClassOf philo:Philosophy. # :Theology

#
# PROPERTIES
#

philos:adheringToThought
	rdfs:isDefinedBy <http://e-editiones.ch/ontology/philosophies#>;
	a owl:ObjectProperty;
	rdfs:label "adhering to philosophy"@en, "ist Anhänger von Philosophie"@de;
	rdfs:comment """Relating a person to a philosophy the person adheres to."""@en;
	rdfs:domain human:Person;
	rdfs:range philo:Philosophy;
	rdfs:subPropertyOf human:adheringToThought.