@prefix rdfs: <http://www.w3.org/2000/01/rdf-schema#>.
@prefix owl: <http://www.w3.org/2002/07/owl#>.
@prefix xsd: <http://www.w3.org/2001/XMLSchema#>.
@prefix skos: <http://www.w3.org/2004/02/skos/core#>.
@prefix geo: <http://www.w3.org/2003/01/geo/wgs84_pos#>.
@prefix dct: <http://purl.org/dc/terms/>.
@prefix cidoc: <http://www.cidoc-crm.org/cidoc-crm/>.
@prefix physical: <http://e-editiones.ch/ontology/physical-entity#>.
@prefix concept: <http://e-editiones.ch/ontology/concept#>.
@prefix text: <http://e-editiones.ch/ontology/text#>.

@base <http://e-editiones.ch/ontology/physical-geography>.
@prefix phygeo: <http://e-editiones.ch/ontology/physical-geography#>.

<http://e-editiones.ch/ontology/physical-geography>
	a owl:Ontology;
	dct:license <http://creativecommons.org/licenses/by/3.0/>;
	dct:title """Physical Geography"""@en;
	dct:description """Formal description of physical geography, general subclasses, related classes, and properties."""@en;
	dct:creator "Hans Cools, MD, knowledge engineer, ontologist, software developer, University of Basel, Switzerland"@en;
	dct:contributor "Dominique Steinbach, tool coordinator and software developer, University of Basel, Switzerland"@en;
	dct:publisher "Universities of Basel, Bern, and Zürich, Switzerland"@en;
	owl:versionInfo "2020-06-11"^^xsd:date;
	rdfs:seeAlso <https://en.wikipedia.org/wiki/World_Geodetic_System>.

#
# CLASSES
#

phygeo:EarthPlace
	rdfs:isDefinedBy <http://e-editiones.ch/ontology/physical-geography#>;
	a rdfs:Class;
	rdfs:label "place on Earth"@en, "Platz auf Erde"@de;
	rdfs:comment """Place on earth, positionable using the World Geodetic System (WGS) standard."""@en;
	rdfs:subClassOf physical:Place.

# cidoc:E48_Place_Name

#
# PROPERTIES
#

phygeo:hasLatitude
	rdfs:isDefinedBy <http://e-editiones.ch/ontology/physical-geography#>;
	a owl:InverseFunctionalProperty, owl:DatatypeProperty;
	rdfs:label "has latitude"@en;
	rdfs:comment """Relating a place of a point or space on the Earth's surface to its geographic coordinate specifying the north–south position of that point, based on the World Geodetic System (WGS) standard. The coordinate is expressed as the angle between the equatorial plane and the normal, for a sphere from the center, to the surface at that point."""@en;
	skos:note """Points with the same latitude lie on a circle around the Earth parallel to its equator. There are different latitudes, depending on the abstracted shape of the earth as spherical or ellipsoid, and other aspects. The decimal value can be converted to a sexagesimal using an N3 rule stating: [decimal degrees - (decimal degrees modulus (%) 1)]° [decimal degrees % 1 x 60 - decimal degrees % 1 x 60 % 1]' + [decimal degrees % 1 * 60 % 1 * 60]''"""@en;
	rdfs:domain phygeo:EarthPlace;
	rdfs:range xsd:decimal;
	rdfs:subPropertyOf geo:lat.

phygeo:hasLongitude
	rdfs:isDefinedBy <http://e-editiones.ch/ontology/physical-geography#>;
	a owl:InverseFunctionalProperty, owl:DatatypeProperty;
	rdfs:label "has longitude"@en;
	rdfs:comment """Relating a place of a point or space on the Earth's surface to its geographic coordinate specifying the east-west position of that point, based on the World Geodetic System (WGS) standard. The coordinate is expressed as the angle in the equatorial plane between a meridian plane containing the surface point and a by convention allocated prime meridian plane at 0 degrees longitude. The IERS Reference Meridian is used here as prime meridian."""@en;
	skos:note """Points with the same longitude lie on a meridian or semi-circle between the poles. There are different longitudes, depending on the abstracted shape of the earth as spherical or ellipsoid, and other aspects. The decimal value can be converted to a sexagesimal using an N3 rule stating: [decimal degrees - (decimal degrees modulus (%) 1)]° [decimal degrees % 1 x 60 - decimal degrees % 1 x 60 % 1]' + [decimal degrees % 1 * 60 % 1 * 60]''"""@en;
	rdfs:domain phygeo:EarthPlace;
	rdfs:range xsd:decimal;
	rdfs:subPropertyOf geo:long.

phygeo:hasElevation #°
	rdfs:isDefinedBy <http://e-editiones.ch/ontology/physical-geography#>;
	a owl:InverseFunctionalProperty, owl:DatatypeProperty;
	rdfs:label "has elevation"@en;
	rdfs:comment """Relating a place of a point or space on the Earth's surface to its height above or below a fixed reference point, most commonly a reference geoid, a mathematical model of the Earth's sea level as an equipotential gravitational surface."""@en;
	rdfs:domain phygeo:EarthPlace;
	rdfs:range xsd:decimal;
	rdfs:subPropertyOf geo:alt.

# SPO cidoc:P87_is_identified_by

phygeo:earthPlaceHasNameLiteral
	rdfs:isDefinedBy <http://e-editiones.ch/ontology/physical-geography#>;
	a owl:DatatypeProperty;
	rdfs:label "earth place has name literal"@en;
	rdfs:comment """Relating a place on Earth to its name literal."""@en;
	rdfs:domain phygeo:EarthPlace;
	rdfs:range rdfs:Literal;
	rdfs:subPropertyOf physical:placeHasNameLiteral.

phygeo:earthPlaceHasIdentifierLiteral
	rdfs:isDefinedBy <http://e-editiones.ch/ontology/physical-geography#>;
	a owl:DatatypeProperty;
	rdfs:label "earth place has identifier literal"@en;
	rdfs:comment """Relating a place on Earth to its identifier literal."""@en;
	rdfs:domain phygeo:EarthPlace;
	rdfs:range rdfs:Literal;
	rdfs:subPropertyOf concept:hasIdentifierLiteral.