@prefix rdf: <http://www.w3.org/1999/02/22-rdf-syntax-ns#>.
@prefix rdfs: <http://www.w3.org/2000/01/rdf-schema#>.
@prefix owl: <http://www.w3.org/2002/07/owl#>.
@prefix xsd: <http://www.w3.org/2001/XMLSchema#>.
@prefix skos: <http://www.w3.org/2004/02/skos/core#>.
@prefix dct: <http://purl.org/dc/terms/>.
@prefix e: <http://www.nie.org/ontology/log-rules#>.
# @prefix tzont: <http://www.w3.org/2006/timezone#>.
@prefix cidoc: <http://www.cidoc-crm.org/cidoc-crm/>.
@prefix event: <http://www.nie.org/ontology/shared/event#>.

# @base <http://www.nie.org/ontology/shared/time>.
@prefix time: <http://www.nie.org/ontology/shared/time#>.

<http://www.nie.org/ontology/shared/time>
	a owl:Ontology;
	dct:title "An ontology about time"@en;
	dct:description """Formal description of time."""@en;
	skos:note """Basic model is a space-time thing, which can be described in different levels of abstraction, mostly with input and output, with a beginning and end, wherein a thing can change and/or act, in a certain way."""@en;
	dct:creator "Hans Cools, MD, knowledge engineer, ontologist, software developer, NIE-INE, Basel University, Switzerland"@en;
	dct:publisher "Basel University, Switzerland"@en;
	dce:format """OWL Full"""@en;
	skos:note """For formal temporal reasoning, using e.g. the Unix Epoch time."""@en;
	skos:note """There are properties with list as range. A list keeps things together in a better way than a blank node and improves reasoning performance. List content is tripled when needed, e.g. to permit SPARQL querying."""@en;
	rdfs:seeAlso
		<http://eulersharp.sourceforge.net/2007/07test/rifP.n3>,
		<http://eulersharp.sourceforge.net/2003/03swap/prolog>,
		<http://eulersharp.sourceforge.net/2007/07test/biP.n3>,
		<http://eulersharp.sourceforge.net/2003/03swap/eventTime_rules>.

#
# PROPERTIES
#

time:hasStartDateTime
	a owl:DatatypeProperty, owl:FunctionalProperty;
	rdfs:isDefinedBy <http://www.nie.org/ontology/time#>;
	skos:definition """Relating an event to its start date time."""@en;
	rdfs:domain event:Event;
	rdfs:range xsd:dateTime.

time:hasEarliestStartDateTime
	a owl:DatatypeProperty, owl:FunctionalProperty;
	rdfs:isDefinedBy <http://www.nie.org/ontology/time#>;
	skos:definition """Relating an event to its rule-calculated earliest possible start date time, based on a set maximum event duration, in absence of the start date time."""@en;
	rdfs:domain event:Event;
	rdfs:range xsd:dateTime.

time:hasStartDate
	a owl:DatatypeProperty, owl:FunctionalProperty;
	rdfs:isDefinedBy <http://www.nie.org/ontology/time#>;
	skos:definition """Relating an event to its start date."""@en;
	rdfs:domain event:Event;
	rdfs:range xsd:date.

time:hasEndDateTime
	a owl:DatatypeProperty, owl:FunctionalProperty;
	rdfs:isDefinedBy <http://www.nie.org/ontology/time#>;
	skos:definition """Relating an event to its end date time."""@en;
	rdfs:domain event:Event;
	rdfs:range xsd:dateTime.

time:hasLatestEndDateTime
	a owl:DatatypeProperty, owl:FunctionalProperty;
	rdfs:isDefinedBy <http://www.nie.org/ontology/time#>;
	skos:definition """Relating an event to its rule-calculated latest possible end date time, based on a set maximum event duration, in absence of the end date time."""@en;
	rdfs:domain event:Event;
	rdfs:range xsd:dateTime.

time:hasEndDate
	a owl:DatatypeProperty, owl:FunctionalProperty;
	rdfs:isDefinedBy <http://www.nie.org/ontology/time#>;
	skos:definition """Relating an event to its end date."""@en;
	rdfs:domain event:Event;
	rdfs:range xsd:date.

time:hasDateTime
	a owl:DatatypeProperty, owl:FunctionalProperty;
	rdfs:isDefinedBy <http://www.nie.org/ontology/time#>;
	skos:definition """Specifying a point in time of something with a date time."""@en;
	rdfs:domain rdfs:Resource;
	rdfs:range xsd:dateTime.

time:hasDate
	a owl:DatatypeProperty, owl:FunctionalProperty;
	rdfs:isDefinedBy <http://www.nie.org/ontology/time#>;
	skos:definition """Specifying a date of something."""@en;
	rdfs:domain rdfs:Resource;
	rdfs:range xsd:date.

time:hasOutputDateTime
	a owl:DatatypeProperty, owl:FunctionalProperty;
	rdfs:isDefinedBy <http://www.nie.org/ontology/time#>;
	skos:definition """Specifying a date time at which a process has an output."""@en;
	rdfs:domain event:Process;
	rdfs:range xsd:dateTime.

time:hasDuration
	a owl:DatatypeProperty, owl:FunctionalProperty;
	rdfs:isDefinedBy <http://www.nie.org/ontology/time#>;
	skos:definition """Specifying a duration of an event."""@en;
	rdfs:domain event:Event;
	rdfs:range xsd:duration.

time:hasMaxDuration
	a owl:DatatypeProperty, owl:FunctionalProperty;
	rdfs:isDefinedBy <http://www.nie.org/ontology/time#>;
	rdfs:label "has maximum duration"@en, "hat maximale Dauer"@de;
	skos:definition """Relating an event to its maximum duration."""@en;
	rdfs:domain event:Event;
	rdfs:range xsd:duration.

time:hasDurationDescription
	a owl:DatatypeProperty, owl:FunctionalProperty;
	rdfs:isDefinedBy <http://www.nie.org/ontology/time#>;
	skos:definition """Specifying a duration description for a temporal entity of something."""@en;
	rdfs:domain rdfs:Resource;
	rdfs:range rdfs:Resource. #any temporal descriptive URI

time:calculatingDuration
	a owl:DatatypeProperty;
	rdfs:isDefinedBy <http://www.nie.org/ontology/time#>;
	skos:definition """Relating an event to its calculated duration."""@en;
	rdfs:comment """Such a triple invokes in an N3 rule a backward N3 rule calculating an event's duration in premise and returning the duration."""@en;
	rdfs:domain event:Event;
	rdfs:range xsd:duration.

time:timeRelatedTo
	a owl:ObjectProperty;
	rdfs:isDefinedBy <http://www.nie.org/ontology/time#>;
	skos:definition """Relating 2 events in time."""@en;
	owl:oneOf (time:beginsBefore time:beginsBeforeEndOf time:hasSameBeginningAs time:beginsDuring time:beginsAfter time:endsBefore time:hasSameEndAs time:endsDuring time:endsAfter time:before time:after time:overlaps time:hasSameTimeAs time:during time:includes time:hasSameDurationAs time:takesLongerThan time:takesLessLongThan);
	rdfs:domain event:Event;
	rdfs:range event:Event.

time:beginsBefore
	a owl:ObjectProperty, owl:TransitiveProperty;
	rdfs:isDefinedBy <http://www.nie.org/ontology/time#>;
	skos:definition """Linking an earlier beginning to a later beginning event."""@en;
	skos:note """Further formalized in an N3 rule by calculation in http://www.nie.org/ontology/eventTime_rules.n3, enabling reasoning with date/time values."""@en;
	rdfs:subPropertyOf time:timeRelatedTo;
	rdfs:domain event:Event;
	rdfs:range event:Event.

time:calculatingBeginsBefore
	a owl:ObjectProperty;
	rdfs:isDefinedBy <http://www.nie.org/ontology/time#>;
	skos:definition """Linking 2 lists with each a beginning and end date time typed literal of an event, and first event begins before second."""@en;
	rdfs:comment """Such a triple invokes in an N3 rule a backward N3 rule checking this time relation for 2 events in premise and returning the triple."""@en;
	rdfs:domain rdf:List;
	rdfs:range rdf:List.

time:beginsBeforeEndOf
	a owl:ObjectProperty;
	rdfs:isDefinedBy <http://www.nie.org/ontology/time#>;
	skos:definition """Linking a beginning event to a later ending of another event."""@en;
	skos:note """Used in an N3 rule conclusion."""@en;
	rdfs:subPropertyOf time:timeRelatedTo;
	owl:propertyChainAxiom (time:beginsDuring time:endsBefore);
	rdfs:domain event:Event;
	rdfs:range event:Event.

time:endsAfterBeginningOf
	a owl:ObjectProperty;
	rdfs:isDefinedBy <http://www.nie.org/ontology/time#>;
	skos:definition """Linking an ending event to an earlier beginning of another event."""@en;
	skos:note """Used in an N3 rule conclusion."""@en;
	rdfs:subPropertyOf time:timeRelatedTo;
	owl:propertyChainAxiom (time:endsDuring time:beginsAfter);
	rdfs:domain event:Event;
	rdfs:range event:Event.

time:hasSameBeginningAs	#	to be varied with accuracy setting, e.g. year, month, weak, day, hour, minute, second
	a owl:SymmetricProperty;
	rdfs:isDefinedBy <http://www.nie.org/ontology/time#>;
	skos:definition """Linking 2 events beginning on the same moment."""@en;
	skos:note """Further formalized in an N3 rule by calculation in http://www.nie.org/ontology/eventTime_rules.n3, enabling reasoning with date/time values."""@en;
	rdfs:subPropertyOf time:timeRelatedTo;
	rdfs:domain event:Event;
	rdfs:range event:Event.

time:calculatingSameBeginning #	to be varied with accuracy setting, e.g. year, month, weak, day, hour, minute, second
	a owl:ObjectProperty;
	rdfs:isDefinedBy <http://www.nie.org/ontology/time#>;
	skos:definition """Linking 2 lists with each a beginning and end date time typed literal of an event, and events beginning at a same time-point."""@en;
	rdfs:comment """Such a triple invokes in an N3 rule a backward N3 rule checking this time relation for 2 events in premise and returning the triple."""@en;
	rdfs:domain rdf:List;
	rdfs:range rdf:List.

time:beginsDuring
	a owl:ObjectProperty, owl:TransitiveProperty;
	rdfs:isDefinedBy <http://www.nie.org/ontology/time#>;
	skos:definition """Specifying an event during which another event begins."""@en;
	rdfs:subPropertyOf time:timeRelatedTo;
	rdfs:domain event:Event;
	rdfs:range event:Event.

time:beginsAfter
	a owl:ObjectProperty, owl:TransitiveProperty;
	rdfs:isDefinedBy <http://www.nie.org/ontology/time#>;
	skos:definition """Linking a later beginning to an earlier beginning event."""@en;
	skos:note """Further formalized in an N3 rule by calculation in http://www.nie.org/ontology/eventTime_rules.n3, enabling reasoning with date/time values."""@en;
	rdfs:subPropertyOf time:timeRelatedTo;
	owl:inverseOf time:beginsBefore;
	rdfs:domain event:Event;
	rdfs:range event:Event.

time:calculatingBeginsAfter
	a owl:ObjectProperty;
	rdfs:isDefinedBy <http://www.nie.org/ontology/time#>;
	skos:definition """Linking 2 lists with each a beginning and end date time typed literal of an event, and first event begins after second."""@en;
	rdfs:comment """Such a triple invokes in an N3 rule a backward N3 rule checking this time relation for 2 events in premise and returning the triple."""@en;
	rdfs:domain rdf:List;
	rdfs:range rdf:List.

time:endsBefore
	a owl:ObjectProperty, owl:TransitiveProperty;
	rdfs:isDefinedBy <http://www.nie.org/ontology/time#>;
	skos:definition """Linking an earlier ending to a later ending event."""@en;
	skos:note """Further formalized in an N3 rule by calculation in http://www.nie.org/ontology/eventTime_rules.n3, enabling reasoning with date/time values."""@en;
	rdfs:subPropertyOf time:timeRelatedTo;
	rdfs:domain event:Event;
	rdfs:range event:Event.

time:calculatingEndsBefore
	a owl:ObjectProperty;
	rdfs:isDefinedBy <http://www.nie.org/ontology/time#>;
	skos:definition """Linking 2 lists with each a beginning and end date time typed literal of an event, and first event ends before second."""@en;
	rdfs:comment """Such a triple invokes in an N3 rule a backward N3 rule checking this time relation for 2 events in premise and returning the triple."""@en;
	rdfs:domain rdf:List;
	rdfs:range rdf:List.

time:hasSameEndAs	#	to be redeclared with accuracy setting, e.g. year, month, weak, day, hour, minute, second
	a owl:SymmetricProperty;
	rdfs:isDefinedBy <http://www.nie.org/ontology/time#>;
	skos:definition """Linking 2 events ending on the same moment."""@en;
	skos:note """Further formalized in an N3 rule by calculation in http://www.nie.org/ontology/eventTime_rules.n3, enabling reasoning with date/time values."""@en;
	rdfs:subPropertyOf time:timeRelatedTo;
	rdfs:domain event:Event;
	rdfs:range event:Event.

time:calculatingSameEnd	
	a owl:ObjectProperty;
	rdfs:isDefinedBy <http://www.nie.org/ontology/time#>;
	skos:definition """Linking 2 lists with each a beginning and end date time typed literal of an event, and events ending at a same time-point."""@en;
	rdfs:comment """Such a triple invokes in an N3 rule a backward N3 rule checking this time relation for 2 events in premise and returning the triple."""@en;
	rdfs:domain rdf:List;
	rdfs:range rdf:List.

time:endsDuring
	a owl:ObjectProperty, owl:TransitiveProperty;
	rdfs:isDefinedBy <http://www.nie.org/ontology/time#>;
	skos:definition """Specifying an event during which another event ends."""@en;
	rdfs:subPropertyOf time:timeRelatedTo;
	rdfs:domain event:Event;
	rdfs:range event:Event.

time:endsAfter
	a owl:ObjectProperty, owl:TransitiveProperty;
	rdfs:isDefinedBy <http://www.nie.org/ontology/time#>;
	skos:definition """Linking a later ending to an earlier ending event."""@en;
	skos:note """Further formalized in an N3 rule by calculation in http://www.nie.org/ontology/eventTime_rules.n3, enabling reasoning with date/time values."""@en;
	rdfs:subPropertyOf time:timeRelatedTo;
	owl:inverseOf time:endsBefore;
	rdfs:domain event:Event;
	rdfs:range event:Event.

time:calculatingEndsAfter
	a owl:ObjectProperty;
	rdfs:isDefinedBy <http://www.nie.org/ontology/time#>;
	skos:definition """Linking 2 lists with each a beginning and end date time typed literal of an event, and first event ends after second."""@en;
	rdfs:comment """Such a triple invokes in an N3 rule a backward N3 rule checking this time relation for 2 events in premise and returning the triple."""@en;
	rdfs:domain rdf:List;
	rdfs:range rdf:List.

time:before
	a owl:ObjectProperty, owl:TransitiveProperty;
	rdfs:isDefinedBy <http://www.nie.org/ontology/time#>;
	skos:definition """Linking an earlier to a later event."""@en;
	skos:note """Further formalized in an N3 rule by calculation in http://www.nie.org/ontology/eventTime_rules.n3, enabling reasoning with date/time values."""@en;
	rdfs:subPropertyOf time:timeRelatedTo;
	rdfs:domain event:Event;
	rdfs:range event:Event.

time:calculatingBefore
	a owl:ObjectProperty;
	rdfs:isDefinedBy <http://www.nie.org/ontology/time#>;
	skos:definition """Linking 2 lists with each a beginning and end date time typed literal of an event, and first event happens before second."""@en;
	rdfs:comment """Such a triple invokes in an N3 rule a backward N3 rule checking this time relation for 2 events in premise and returning the triple."""@en;
	rdfs:domain rdf:List;
	rdfs:range rdf:List.

time:after
	a owl:ObjectProperty, owl:TransitiveProperty;
	rdfs:isDefinedBy <http://www.nie.org/ontology/time#>;
	skos:definition """Linking a later to an earlier event."""@en;
	skos:note """Further formalized in an N3 rule by calculation in http://www.nie.org/ontology/eventTime_rules.n3, enabling reasoning with date/time values."""@en;
	rdfs:subPropertyOf time:timeRelatedTo;
	owl:inverseOf time:before;
	rdfs:domain event:Event;
	rdfs:range event:Event.

time:calculatingAfter
	a owl:ObjectProperty;
	rdfs:isDefinedBy <http://www.nie.org/ontology/time#>;
	skos:definition """Linking 2 lists with each a beginning and end date time typed literal of an event, and first event happens after second."""@en;
	rdfs:comment """Such a triple invokes in an N3 rule a backward N3 rule checking this time relation for 2 events in premise and returning the triple."""@en;
	rdfs:domain rdf:List;
	rdfs:range rdf:List.

time:overlaps
	a owl:SymmetricProperty;
	rdfs:isDefinedBy <http://www.nie.org/ontology/time#>;
	skos:definition """Specifying an event overlapping another event."""@en;
	skos:note """Further formalized in an N3 rule by calculation in http://www.nie.org/ontology/eventTime_rules.n3, enabling reasoning with date/time values."""@en;
	rdfs:subPropertyOf time:timeRelatedTo;
	rdfs:domain event:Event;
	rdfs:range event:Event.

time:calculatingOverlaps
	a owl:ObjectProperty;
	rdfs:isDefinedBy <http://www.nie.org/ontology/time#>;
	skos:definition """Linking 2 lists with each a beginning and end date time typed literal of an event, and events overlap each other."""@en;
	rdfs:comment """Such a triple invokes in an N3 rule a backward N3 rule checking this time relation for 2 events in premise and returning the triple."""@en;
	rdfs:domain rdf:List;
	rdfs:range rdf:List.

time:hasSameTimeAs	#	to be redeclared with accuracy setting, e.g. year, month, weak, day, our, minute, second
	a owl:SymmetricProperty;
	rdfs:isDefinedBy <http://www.nie.org/ontology/time#>;
	skos:definition """Linking 2 events happening at the same time."""@en;
	skos:note """Further formalized in an N3 rule by calculation in http://www.nie.org/ontology/eventTime_rules.n3, enabling reasoning with date/time values."""@en;
	rdfs:subPropertyOf time:timeRelatedTo;
	rdfs:domain event:Event;
	rdfs:range event:Event.

time:calculatingSameTime
	a owl:ObjectProperty;
	rdfs:isDefinedBy <http://www.nie.org/ontology/time#>;
	skos:definition """Linking 2 lists with each a beginning and end date time typed literal of an event, and events happen during same time."""@en;
	rdfs:comment """Such a triple invokes in an N3 rule a backward N3 rule checking this time relation for 2 events in premise and returning the triple."""@en;
	rdfs:domain rdf:List;
	rdfs:range rdf:List.

time:during
	a owl:ObjectProperty, owl:TransitiveProperty;
	rdfs:isDefinedBy <http://www.nie.org/ontology/time#>;
	skos:definition """Specifying an event during which another event happens."""@en;
	skos:note """Further formalized in an N3 rule by calculation in http://www.nie.org/ontology/eventTime_rules.n3, enabling reasoning with date/time values."""@en;
	rdfs:subPropertyOf time:timeRelatedTo;
	rdfs:domain event:Event;
	rdfs:range event:Event.

time:calculatingDuring
	a owl:ObjectProperty;
	rdfs:isDefinedBy <http://www.nie.org/ontology/time#>;
	skos:definition """Linking 2 lists with each a beginning and end date time typed literal of an event, and first event happens during second."""@en;
	rdfs:comment """Such a triple invokes in an N3 rule a backward N3 rule checking this time relation for 2 events in premise and returning the triple."""@en;
	rdfs:domain rdf:List;
	rdfs:range rdf:List.

time:includes
	a owl:ObjectProperty, owl:TransitiveProperty;
	rdfs:isDefinedBy <http://www.nie.org/ontology/time#>;
	skos:definition """Specifying an event happening during another event."""@en;
	skos:note """Further formalized in an N3 rule by calculation in http://www.nie.org/ontology/eventTime_rules.n3, enabling reasoning with date/time values."""@en;
	rdfs:subPropertyOf time:timeRelatedTo;
	owl:inverseOf time:during;
	rdfs:domain event:Event;
	rdfs:range event:Event.

time:calculatingIncludes
	a owl:ObjectProperty;
	rdfs:isDefinedBy <http://www.nie.org/ontology/time#>;
	skos:definition """Linking 2 lists with each a beginning and end date time typed literal of an event, and first event includes second."""@en;
	rdfs:comment """Such a triple invokes in an N3 rule a backward N3 rule checking this time relation for 2 events in premise and returning the triple."""@en;
	rdfs:domain rdf:List;
	rdfs:range rdf:List.

time:hasSameDurationAs # to be redeclared with accuracy setting, e.g. year, month, weak, day, our, minute, second
	a owl:SymmetricProperty;
	rdfs:isDefinedBy <http://www.nie.org/ontology/time#>;
	skos:definition """Linking 2 events having the same duration."""@en;
	skos:note """Further formalized in an N3 rule by calculation in http://www.nie.org/ontology/eventTime_rules.n3, enabling reasoning with date/time values."""@en;
	rdfs:subPropertyOf time:timeRelatedTo;
	rdfs:domain event:Event;
	rdfs:range event:Event.

time:calculatingSameDuration
	a owl:ObjectProperty;
	rdfs:isDefinedBy <http://www.nie.org/ontology/time#>;
	skos:definition """Linking 2 lists with each a beginning and end date time typed literal of an event, and events having same duration."""@en;
	rdfs:comment """Such a triple invokes in an N3 rule a backward N3 rule checking this time relation for 2 events in premise and returning the triple."""@en;
	rdfs:domain rdf:List;
	rdfs:range rdf:List.

time:takesLongerThan
	a owl:ObjectProperty, owl:TransitiveProperty;
	rdfs:isDefinedBy <http://www.nie.org/ontology/time#>;
	skos:definition """Linking a longer to a shorter event."""@en;
	skos:note """Further formalized in an N3 rule by calculation in http://www.nie.org/ontology/eventTime_rules.n3, enabling reasoning with date/time values."""@en;
	rdfs:subPropertyOf time:timeRelatedTo;
	rdfs:domain event:Event;
	rdfs:range event:Event.

time:calculatingTakesLongerThan
	a owl:ObjectProperty;
	rdfs:isDefinedBy <http://www.nie.org/ontology/time#>;
	skos:definition """Linking 2 lists with each a beginning and end date time typed literal of an event, and first event takes longer than second."""@en;
	rdfs:comment """Such a triple invokes in an N3 rule a backward N3 rule checking this time relation for 2 events in premise and returning the triple."""@en;
	rdfs:domain rdf:List;
	rdfs:range rdf:List.

time:takesLessLongThan
	a owl:ObjectProperty, owl:TransitiveProperty;
	rdfs:isDefinedBy <http://www.nie.org/ontology/time#>;
	skos:definition """Linking a shorter to a longer event."""@en;
	skos:note """Further formalized in an N3 rule by calculation in http://www.nie.org/ontology/eventTime_rules.n3, enabling reasoning with date/time values."""@en;
	rdfs:subPropertyOf time:timeRelatedTo;
	owl:inverseOf time:takesLongerThan;
	rdfs:domain event:Event;
	rdfs:range event:Event.

time:calculatingTakesLessLongThan
	a owl:ObjectProperty;
	rdfs:isDefinedBy <http://www.nie.org/ontology/time#>;
	skos:definition """Linking 2 lists with each a beginning and end date time typed literal of an event, and first event takes less long than second."""@en;
	rdfs:comment """Such a triple invokes in an N3 rule a backward N3 rule checking this time relation for 2 events in premise and returning the triple."""@en;
	rdfs:domain rdf:List;
	rdfs:range rdf:List.

time:hasSnapshotDateTime
	a owl:DatatypeProperty, owl:FunctionalProperty;
	rdfs:isDefinedBy <http://www.nie.org/ontology/time#>;
	skos:definition """Specifying a snapshot event's date and time."""@en;
	rdfs:comment """A snapshot is an event with coinciding beginning and end."""@en;
	skos:note """Used in N3 rules calculating with date time and duration using Unix Epoch time."""@en;
	rdfs:domain event:Event;
	rdfs:range xsd:dateTime.

time:hasSnapshotDate
	a owl:DatatypeProperty, owl:FunctionalProperty;
	rdfs:isDefinedBy <http://www.nie.org/ontology/time#>;
	skos:definition """Specifying a snapshot event's date."""@en;
	rdfs:comment """A snapshot is an event with coinciding beginning and end."""@en;
	skos:note """Used in N3 rules calculating with date and duration using Unix Epoch time."""@en;
	rdfs:domain event:Event;
	rdfs:range xsd:date.

time:hasTimeZone
	a owl:DatatypeProperty, owl:FunctionalProperty;
	rdfs:isDefinedBy <http://www.nie.org/ontology/time#>;
	skos:definition """Specifying a time zone of something."""@en;
	rdfs:comment """Time zone extracted from an xsd:date, xsd:dateTime or xsd:time typed literal with rif builtin functions."""@en;
	rdfs:seeAlso <http://eulersharp.sourceforge.net/2006/02swap/rif-plugin.yap>, <http://eulersharp.sourceforge.net/2007/07test/rifP.n3>;
	skos:note """Used in N3 rules calculating with date and duration using Unix Epoch time."""@en;
	rdfs:range xsd:dayTimeDuration.

time:dateLiteralToPeriod
	a owl:ObjectProperty;
	rdfs:isDefinedBy <http://www.nie.org/ontology/time#>;
	skos:definition """Linking a list with 3 literals, resp representing number of years, number of months and number of days, to a list with 2 xsd:dateTime typed literals representing a beginning and an end of a day."""@en;
	rdfs:comment """Used in an N3 rule triple to invoke a backward N3 rule converting a date described by 3 literals to a period described by beginning and end date time, in this way explicitly stating the implicit period of a day margin."""@en;
	rdfs:comment """In N3 rules universally quantified variables are declared to pick up the respective values: (?yearLiteral ?monthLiteral ?dayLiteral) time:dateLiteralToPeriod (?beginning ?end)."""@en;
	rdfs:domain rdf:List;
	rdfs:range rdf:List.
	
time:yearMonthLiteralToPeriod
	a owl:ObjectProperty;
	rdfs:isDefinedBy <http://www.nie.org/ontology/time#>;
	skos:definition """Linking a list with 2 literals, resp representing number of years and number of months, to a list with 2 xsd:dateTime typed literals representing a beginning and an end of a month."""@en;
	rdfs:comment """Used in an N3 rule triple to invoke a backward N3 rule converting 2 literals to a period described by beginning and end date time, in this way explicitly stating the implicit period of a month margin."""@en;
	rdfs:comment """In N3 rules universally quantified variables are declared to pick up the respective values: (?yearLiteral ?monthLiteral) time:yearMonthLiteralToPeriod (?beginning ?end); at runtime this will generate e.g. subject ("2010" "3") and object (."""@en;
	rdfs:domain rdf:List;
	rdfs:range rdf:List.

time:yearLiteralToPeriod
	a owl:ObjectProperty;
	rdfs:isDefinedBy <http://www.nie.org/ontology/time#>;
	skos:definition """Linking a literal representing number of years to a list with 2 xsd:dateTime typed literals representing a beginning and an end of a year."""@en;
	rdfs:comment """Used in a triple to invoke a backward N3 rule converting a literal to a period described by beginning and end date time, in this way explicitly stating the implicit period of a year margin."""@en;
	rdfs:comment """In N3 rules universally quantified variables are declared to pick up the respective values: ?yearLiteral time:yearLiteralToPeriod (?beginning ?end)."""@en;
	rdfs:domain rdfs:Literal;
	rdfs:range rdf:List.

time:dateToPeriod
	a owl:ObjectProperty;
	rdfs:isDefinedBy <http://www.nie.org/ontology/time#>;
	skos:definition """Linking an xsd:date typed literal to a list with 2 xsd:dateTime typed literals representing a beginning and an end of a day."""@en;
	rdfs:comment """Used in a triple to invoke a backward N3 rule converting an xsd:date typed literal to a period described by beginning and end date time, in this way explicitly stating the implicit time period margin."""@en;
	rdfs:comment """In N3 rules universally quantified variables are declared to pick up the respective values: ?date time:dateToPeriod (?beginning ?end)."""@en;
	rdfs:domain xsd:date;
	rdfs:range rdf:List.

time:hasBeginningPeriodMargin
	a owl:ObjectProperty;
	rdfs:isDefinedBy <http://www.nie.org/ontology/time#>;
	skos:definition """Linking an event to a list with 2 xsd:dateTime typed literals representing a beginning and an end of a period wherein it begins."""@en;
	rdfs:domain event:Event;
	rdfs:range rdf:List.

time:hasEndPeriodMargin
	a owl:ObjectProperty;
	rdfs:isDefinedBy <http://www.nie.org/ontology/time#>;
	skos:definition """Linking an event to a list with 2 xsd:dateTime typed literals representing a beginning and an end of a period wherein it ends."""@en;
	rdfs:domain event:Event;
	rdfs:range rdf:List.

time:hasObtainingPeriodMargin
	a owl:ObjectProperty;
	rdfs:isDefinedBy <http://www.nie.org/ontology/time#>;
	skos:definition """Linking something to a list with 2 xsd:dateTime typed literals representing a beginning and an end of a period wherein it is obtained."""@en;
	rdfs:domain rdfs:Resource;
	rdfs:range rdf:List.

time:hasPerformingPeriodMargin
	a owl:ObjectProperty;
	rdfs:isDefinedBy <http://www.nie.org/ontology/time#>;
	skos:definition """Linking an action to a list with 2 xsd:dateTime typed literals representing a beginning and an end of a period wherein the action is performed."""@en;
	rdfs:domain event:Action;
	rdfs:range rdf:List.

time:hasObservingPeriodMargin
	a owl:ObjectProperty;
	rdfs:isDefinedBy <http://www.nie.org/ontology/time#>;
	skos:definition """Linking something to a list with 2 xsd:dateTime typed literals representing a beginning and an end of a period wherein it is observed."""@en;
	rdfs:domain rdfs:Resource;
	rdfs:range rdf:List.

time:hasExaminingPeriodMargin
	a owl:ObjectProperty;
	rdfs:isDefinedBy <http://www.nie.org/ontology/time#>;
	skos:definition """Linking something to a list with 2 xsd:dateTime typed literals representing a beginning and an end of a period wherein it is examined."""@en;
	rdfs:domain rdfs:Resource;
	rdfs:range rdf:List.

time:hasEvaluatingPeriodMargin
	a owl:ObjectProperty;
	rdfs:isDefinedBy <http://www.nie.org/ontology/time#>;
	skos:definition """Linking something to a list with 2 xsd:dateTime typed literals representing a beginning and an end of a period wherein it is evaluated."""@en;
	rdfs:domain rdfs:Resource;
	rdfs:range rdf:List.

time:hasDiagnosingPeriodMargin
	a owl:ObjectProperty;
	rdfs:isDefinedBy <http://www.nie.org/ontology/time#>;
	skos:definition """Linking something to a list with 2 xsd:dateTime typed literals representing a beginning and an end of a period wherein it is diagnosed."""@en;
	rdfs:domain rdfs:Resource;
	rdfs:range rdf:List.

time:hasTreatingPeriodMargin
	a owl:ObjectProperty;
	rdfs:isDefinedBy <http://www.nie.org/ontology/time#>;
	skos:definition """Linking something to a list with 2 xsd:dateTime typed literals representing a beginning and an end of a period wherein it is treated."""@en;
	rdfs:domain rdfs:Resource;
	rdfs:range rdf:List.

time:hasAge
	a owl:FunctionalProperty;
	rdfs:isDefinedBy <http://www.nie.org/ontology/time#>;
	skos:definition """Specifying an age in years of something."""@en;
	rdfs:domain rdfs:Resource;
	rdfs:range e:Number.

time:hasAges
	a owl:FunctionalProperty;
	rdfs:isDefinedBy <http://www.nie.org/ontology/time#>;
	skos:definition """Linking a group of something to a list of its members' ages in years."""@en;
	rdfs:domain rdfs:Class;
	rdfs:range rdf:List.

time:calculatingAge
	a owl:FunctionalProperty;
	rdfs:isDefinedBy <http://www.nie.org/ontology/time#>;
	skos:definition """Specifying a calculated age in years for a list of something and a reference date time."""@en;
	skos:note """Triggering in an N3 rule a backward N3 rule to calculate an age of something depending on a reference date time."""@en;
	rdfs:domain rdf:List;
	rdfs:range e:Number.

time:hasMedianAge
	a owl:DatatypeProperty, owl:FunctionalProperty;
	rdfs:isDefinedBy <http://www.nie.org/ontology/time#>;
	skos:definition """Linking a class to the median age of its members."""@en;
	rdfs:domain rdfs:Class;
	rdfs:range e:Number.

time:endsSameAsBeginningOf
	a owl:ObjectProperty, owl:TransitiveProperty;
	rdfs:isDefinedBy <http://www.nie.org/ontology/time#>;
	skos:definition """Linking an ending event to another event beginning at the same moment."""@en;
	skos:note """Further formalized in an N3 rule by calculation in http://www.nie.org/ontology/eventTime_rules.n3, enabling reasoning with date/time values."""@en;
	rdfs:subPropertyOf time:timeRelatedTo;
	owl:inverseOf time:beginsSameAsEndOf;
	rdfs:domain event:Event;
	rdfs:range event:Event.

time:beginsSameAsEndOf
	a owl:ObjectProperty, owl:TransitiveProperty;
	rdfs:isDefinedBy <http://www.nie.org/ontology/time#>;
	skos:definition """Linking a beginning event to another event ending at the same moment."""@en;
	skos:note """Further formalized in an N3 rule by calculation in http://www.nie.org/ontology/eventTime_rules.n3, enabling reasoning with date/time values."""@en;
	rdfs:subPropertyOf time:timeRelatedTo;
	owl:inverseOf time:endsSameAsBeginningOf;
	rdfs:domain event:Event;
	rdfs:range event:Event.